PREFIX : <https://linked.data.gov.au/def/national-groundwater-information-system/>
PREFIX cs: <https://linked.data.gov.au/def/national-groundwater-information-system>
PREFIX dcterms: <http://purl.org/dc/terms/>
PREFIX owl: <http://www.w3.org/2002/07/owl#>
PREFIX schema: <https://schema.org/>
PREFIX skos: <http://www.w3.org/2004/02/skos/core#>
PREFIX xsd: <http://www.w3.org/2001/XMLSchema#>

:Aquaveo
    a skos:Concept ;
    dcterms:created "2017-11-08"^^xsd:date ;
    dcterms:creator <https://linked.data.gov.au/org/neii> ;
    skos:definition "A software development company based in the United States that builds ArcHydro for groundwater tools"@en ;
    skos:inScheme cs: ;
    skos:prefLabel "Aquaveo"@en ;
    skos:topConceptOf cs: ;
.

:ArcGIS
    a skos:Concept ;
    dcterms:created "2017-11-08"^^xsd:date ;
    dcterms:creator <https://linked.data.gov.au/org/neii> ;
    skos:definition "A range of software programs developed by ESRI for spatial data analysis, processing and storage."@en ;
    skos:inScheme cs: ;
    skos:prefLabel "ArcGIS"@en ;
    skos:topConceptOf cs: ;
.

:ArcHydro-for-Groundwater
    a skos:Concept ;
    dcterms:created "2017-11-08"^^xsd:date ;
    dcterms:creator <https://linked.data.gov.au/org/neii> ;
    skos:definition "A data model published by ESRI and tools developed by Aquaveo for analysis of hydrogeological data."@en ;
    skos:inScheme cs: ;
    skos:prefLabel "ArcHydro for Groundwater"@en ;
    skos:topConceptOf cs: ;
.

:ESRI
    a skos:Concept ;
    dcterms:created "2017-11-08"^^xsd:date ;
    dcterms:creator <https://linked.data.gov.au/org/neii> ;
    skos:definition "A software development company based in the United States that builds ArcGIS."@en ;
    skos:inScheme cs: ;
    skos:prefLabel "ESRI"@en ;
    skos:topConceptOf cs: ;
.

:ESRI-File-Geodatabase
    a skos:Concept ;
    dcterms:created "2017-11-08"^^xsd:date ;
    dcterms:creator <https://linked.data.gov.au/org/neii> ;
    skos:definition "A format for storing GIS data within the ArcGIS software"@en ;
    skos:inScheme cs: ;
    skos:prefLabel "ESRI File Geodatabase"@en ;
    skos:topConceptOf cs: ;
.

:australia-new-zealand-land-information-council
    a skos:Concept ;
    dcterms:created "2017-11-08"^^xsd:date ;
    dcterms:creator <https://linked.data.gov.au/org/neii> ;
    skos:definition "ANZLIC is the Spatial Information Council is the peak intergovernmental organisation providing leadership in the collection, management and use of spatial information in Australia and New Zealand. They have established a widely metadata profile for spatial data in Australia."@en ;
    skos:inScheme cs: ;
    skos:notation "ANZLIC" ;
    skos:prefLabel "australia new zealand land information council"@en ;
    skos:topConceptOf cs: ;
.

:bore
    a skos:Concept ;
    dcterms:created "2017-11-08"^^xsd:date ;
    dcterms:creator <https://linked.data.gov.au/org/neii> ;
    skos:definition "A hole drilled in the ground, a well or any other excavation used to access groundwater. May be used for observation of groundwater (including water level, pressure or quality)."@en ;
    skos:inScheme cs: ;
    skos:prefLabel "bore"@en ;
    skos:topConceptOf cs: ;
.

:bore-feature
    a skos:Concept ;
    dcterms:created "2017-11-08"^^xsd:date ;
    dcterms:creator <https://linked.data.gov.au/org/neii> ;
    skos:definition "Point feature class that represents the location of a bore and associated attributes. Multiple independently screened bore pipes are regarded as separate bore features."@en ;
    skos:inScheme cs: ;
    skos:prefLabel "bore feature"@en ;
    skos:topConceptOf cs: ;
.

:bore-line
    a skos:Concept ;
    dcterms:created "2017-11-08"^^xsd:date ;
    dcterms:creator <https://linked.data.gov.au/org/neii> ;
    skos:definition "A three dimensional line feature class that represents the hydrogeologic units along a borehole."@en ;
    skos:inScheme cs: ;
    skos:prefLabel "bore line"@en ;
    skos:topConceptOf cs: ;
.

:bore-log
    a skos:Concept ;
    dcterms:created "2017-11-08"^^xsd:date ;
    dcterms:creator <https://linked.data.gov.au/org/neii> ;
    skos:altLabel "hydrostratigraphy log"@en ;
    skos:definition "A table with rock or sediment types classified into hydrogeologic units along a borehole."@en ;
    skos:inScheme cs: ;
    skos:prefLabel "bore log"@en ;
    skos:topConceptOf cs: ;
.

:bore-pipe
    a skos:Concept ;
    dcterms:created "2017-11-08"^^xsd:date ;
    dcterms:creator <https://linked.data.gov.au/org/neii> ;
    skos:definition "An independently screened inlet to a bore that can be pumped or monitored separately. A bore can have multiple pipes, each having one or more screens."@en ;
    skos:inScheme cs: ;
    skos:prefLabel "bore pipe"@en ;
    skos:topConceptOf cs: ;
.

:bore-screen
    a skos:Concept ;
    dcterms:created "2017-11-08"^^xsd:date ;
    dcterms:creator <https://linked.data.gov.au/org/neii> ;
    skos:definition "The construction component of a bore that allows groundwater to enter e.g. casing with slots or holes."@en ;
    skos:inScheme cs: ;
    skos:prefLabel "bore screen"@en ;
    skos:topConceptOf cs: ;
.

:casing
    a skos:Concept ;
    dcterms:created "2017-11-08"^^xsd:date ;
    dcterms:creator <https://linked.data.gov.au/org/neii> ;
    skos:definition "The construction component that lines a bore and provides the conduit from the water-producing zone to the surface."@en ;
    skos:inScheme cs: ;
    skos:prefLabel "casing"@en ;
    skos:topConceptOf cs: ;
.

:construction-line
    a skos:Concept ;
    dcterms:created "2017-11-08"^^xsd:date ;
    dcterms:creator <https://linked.data.gov.au/org/neii> ;
    skos:definition "A three dimensional line feature class that represents the construction information (e.g. casing and bore screen) along a borehole"@en ;
    skos:inScheme cs: ;
    skos:prefLabel "construction line"@en ;
    skos:topConceptOf cs: ;
.

:construction-log
    a skos:Concept ;
    dcterms:created "2017-11-08"^^xsd:date ;
    dcterms:creator <https://linked.data.gov.au/org/neii> ;
    skos:definition "A table with bore construction information along a borehole (e.g. casing and bore screen)."@en ;
    skos:inScheme cs: ;
    skos:prefLabel "construction log"@en ;
    skos:topConceptOf cs: ;
.

:creative-commons
    a skos:Concept ;
    dcterms:created "2017-11-08"^^xsd:date ;
    dcterms:creator <https://linked.data.gov.au/org/neii> ;
    dcterms:source "Creative Commons Australia"@en ;
    skos:definition "An international non-profit organisation that provides free licences and tools that copyright owners can use to allow others to share, reuse and remix their material, legally."@en ;
    skos:inScheme cs: ;
    skos:notation "CC" ;
    skos:prefLabel "creative commons"@en ;
    skos:topConceptOf cs: ;
.

:digital-elevation-model
    a skos:Concept ;
    dcterms:created "2017-11-08"^^xsd:date ;
    dcterms:creator <https://linked.data.gov.au/org/neii> ;
    skos:definition "A digital elevation model of the earth's surface."@en ;
    skos:inScheme cs: ;
    skos:notation "DEM" ;
    skos:prefLabel "digital elevation model"@en ;
    skos:topConceptOf cs: ;
.

:feature-class
    a skos:Concept ;
    dcterms:created "2017-11-08"^^xsd:date ;
    dcterms:creator <https://linked.data.gov.au/org/neii> ;
    dcterms:source "ArcGIS 9.2 Desktop Help"@en ;
    skos:definition "Homogeneous collections of common features, each having the same spatial representation, such as points, lines, or polygons, and a common set of attribute columns, for example, a line feature class for representing road centrelines. The four most commonly used feature classes in the geodatabase are points, lines, polygons, and annotation (the geodatabase name for map text)."@en ;
    skos:inScheme cs: ;
    skos:prefLabel "feature class"@en ;
    skos:topConceptOf cs: ;
.

:geographic-information-system
    a skos:Concept ;
    dcterms:created "2017-11-08"^^xsd:date ;
    dcterms:creator <https://linked.data.gov.au/org/neii> ;
    skos:definition "A system used for the design, capture, storage, management and analysis of geographic data. Often referred to as GIS."@en ;
    skos:inScheme cs: ;
    skos:notation "GIS" ;
    skos:prefLabel "geographic information system"@en ;
    skos:topConceptOf cs: ;
.

:georaster
    a skos:Concept ;
    dcterms:created "2017-11-08"^^xsd:date ;
    dcterms:creator <https://linked.data.gov.au/org/neii> ;
    skos:definition "A catalog of raster datasets describing properties of hydrogeologic units (e.g. depth or elevation of hydrogeologic unit's top or base, salinity and groundwater level)."@en ;
    skos:inScheme cs: ;
    skos:prefLabel "georaster"@en ;
    skos:topConceptOf cs: ;
.

:geovolume
    a skos:Concept ;
    dcterms:created "2017-11-08"^^xsd:date ;
    dcterms:creator <https://linked.data.gov.au/org/neii> ;
    skos:definition "A three dimensional multipatch feature class that represents hydrogeologic units as a volume."@en ;
    skos:inScheme cs: ;
    skos:prefLabel "geovolume"@en ;
    skos:topConceptOf cs: ;
.

:hydrostratigraphy-log
    a skos:Concept ;
    dcterms:created "2017-11-08"^^xsd:date ;
    dcterms:creator <https://linked.data.gov.au/org/neii> ;
    skos:altLabel "bore log"@en ;
    skos:definition "A table with rock or sediment types classified into hydrogeologic units along a borehole."@en ;
    skos:inScheme cs: ;
    skos:prefLabel "hydrostratigraphy log"@en ;
    skos:topConceptOf cs: ;
.

:lithology-log
    a skos:Concept ;
    dcterms:created "2017-11-08"^^xsd:date ;
    dcterms:creator <https://linked.data.gov.au/org/neii> ;
    skos:definition "A table with drillers' or geologists' description of rock or sediment types along a borehole."@en ;
    skos:inScheme cs: ;
    skos:prefLabel "lithology log"@en ;
    skos:topConceptOf cs: ;
.

:multipatch-feature-class
    a skos:Concept ;
    dcterms:created "2017-11-08"^^xsd:date ;
    dcterms:creator <https://linked.data.gov.au/org/neii> ;
    dcterms:source "ArcGIS Help 10.1"@en ;
    skos:definition "A GIS object that stores a collection of patches to represent the boundary of a three dimensional object as a single row in a database."@en ;
    skos:inScheme cs: ;
    skos:prefLabel "multipatch feature class"@en ;
    skos:topConceptOf cs: ;
.

:national-groundwater-information-system
    a skos:Concept ;
    dcterms:created "2017-11-08"^^xsd:date ;
    dcterms:creator <https://linked.data.gov.au/org/neii> ;
    skos:definition "A spatially-enabled database for storing and analysing Australian groundwater data."@en ;
    skos:inScheme cs: ;
    skos:notation "NGIS" ;
    skos:prefLabel "national groundwater information system"@en ;
    skos:topConceptOf cs: ;
.

:raster-dataset
    a skos:Concept ;
    dcterms:created "2017-11-08"^^xsd:date ;
    dcterms:creator <https://linked.data.gov.au/org/neii> ;
    skos:definition "Represents geographic features by dividing the world into discrete square or rectangular cells laid out in a grid. Each cell has a value that is used to represent some characteristic of that location."@en ;
    skos:inScheme cs: ;
    skos:prefLabel "raster dataset"@en ;
    skos:topConceptOf cs: ;
.

<https://linked.data.gov.au/org/bom-gu>
    a dcterms:Agent ;
    schema:name "Groundwater Unit, Bureau of Meteorology" ;
    schema:url "http://www.bom.gov.au/water/groundwater/"^^xsd:anyURI ;
.

cs:
    a skos:ConceptScheme ;
    dcterms:contributor <https://linked.data.gov.au/org/bom-gu> ;
    dcterms:created "2017-11-08"^^xsd:date ;
    dcterms:creator <https://linked.data.gov.au/org/bom-gu> ;
    dcterms:issued "2013-05" ;
    dcterms:modified "2024-04-15"^^xsd:date ;
    dcterms:publisher <https://linked.data.gov.au/org/bom-gu> ;
    dcterms:subject "Groundwater"@en ;
    owl:versionInfo "Version 1" ;
    skos:definition "The National Groundwater Information System (NGIS) is a spatial database for GIS specialists that contains a range of groundwater information submitted by States and Territories. The NGIS contains information on more than 870 000 bores and their attributes—such as purpose and date they were drilled. The database also includes logs of their lithology, construction and hydrostratigraphy as well as groundwater management areas and aquifer boundaries. 2.5D and 3D aquifer geometries are also available for some areas. Hydrogeologic units within the NGIS have been standardised for national consistency using the National Aquifer Framework.  http://www.bom.gov.au/water/groundwater/ngis/ "@en ;
    skos:hasTopConcept
        :Aquaveo ,
        :ArcGIS ,
        :ArcHydro-for-Groundwater ,
        :ESRI ,
        :ESRI-File-Geodatabase ,
        :australia-new-zealand-land-information-council ,
        :bore ,
        :bore-feature ,
        :bore-line ,
        :bore-log ,
        :bore-pipe ,
        :bore-screen ,
        :casing ,
        :construction-line ,
        :construction-log ,
        :creative-commons ,
        :digital-elevation-model ,
        :feature-class ,
        :geographic-information-system ,
        :georaster ,
        :geovolume ,
        :hydrostratigraphy-log ,
        :lithology-log ,
        :multipatch-feature-class ,
        :national-groundwater-information-system ,
        :raster-dataset ;
    skos:historyNote "2024-04: IRIs changed from http://www.neii.gov.au/def/voc/GW/national-groundwater-information-system/National-Groundwater-Information-System for the ConceptScheme and http://www.neii.gov.au/def/voc/GW/national-groundwater-information-system/ for the Concept namespace to linked.data.gov.au-based IRIs" ;
    skos:prefLabel "National Groundwater Information System"@en ;
.
