PREFIX : <https://linked.data.gov.au/def/australian-groundwater-insight/>
PREFIX cs: <https://linked.data.gov.au/def/australian-groundwater-insight>
PREFIX dcterms: <http://purl.org/dc/terms/>
PREFIX owl: <http://www.w3.org/2002/07/owl#>
PREFIX schema: <https://schema.org/>
PREFIX skos: <http://www.w3.org/2004/02/skos/core#>
PREFIX xsd: <http://www.w3.org/2001/XMLSchema#>

:aquifer
    a skos:Concept ;
    dcterms:created "2017-11-16"^^xsd:date ;
    dcterms:creator <https://linked.data.gov.au/org/neii> ;
    skos:definition "A geological formation or group of formations; able to receive, store and transmit significant quantities of water."@en ;
    skos:inScheme cs: ;
    skos:prefLabel "aquifer"@en ;
    skos:topConceptOf cs: ;
.

:bedrock
    a skos:Concept ;
    dcterms:created "2017-11-16"^^xsd:date ;
    dcterms:creator <https://linked.data.gov.au/org/neii> ;
    skos:definition "A consolidated rock that underlies geological basins. Above the bedrock is usually an area of weathered and unconsolidated rock which can from aquifers."@en ;
    skos:inScheme cs: ;
    skos:prefLabel "bedrock"@en ;
    skos:topConceptOf cs: ;
.

:bore
    a skos:Concept ;
    dcterms:created "2017-11-16"^^xsd:date ;
    dcterms:creator <https://linked.data.gov.au/org/neii> ;
    skos:definition "A hole drilled in the ground, a well or any other excavation used to access groundwater. May be used for observation of groundwater (including water level, pressure or water quality)."@en ;
    skos:inScheme cs: ;
    skos:prefLabel "bore"@en ;
    skos:topConceptOf cs: ;
.

:bore-density
    a skos:Concept ;
    dcterms:created "2017-11-16"^^xsd:date ;
    dcterms:creator <https://linked.data.gov.au/org/neii> ;
    skos:definition "The number of bores per unit area of land."@en ;
    skos:inScheme cs: ;
    skos:prefLabel "bore density"@en ;
    skos:topConceptOf cs: ;
.

:confined-aquifer
    a skos:Concept ;
    dcterms:created "2017-11-16"^^xsd:date ;
    dcterms:creator <https://linked.data.gov.au/org/neii> ;
    skos:definition "An aquifer whose upper surface is confined by an overlaying geological formation. Groundwater in a confined aquifer is typically under pressure."@en ;
    skos:inScheme cs: ;
    skos:prefLabel "confined aquifer"@en ;
    skos:topConceptOf cs: ;
.

:groundwater-entitlement-limit
    a skos:Concept ;
    dcterms:created "2017-11-16"^^xsd:date ;
    dcterms:creator <https://linked.data.gov.au/org/neii> ;
    skos:definition "The theoretical maximum volume of water that may be issued as entitlement within a Groundwater Management Area."@en ;
    skos:inScheme cs: ;
    skos:prefLabel "groundwater entitlement limit"@en ;
    skos:topConceptOf cs: ;
.

:groundwater-level
    a skos:Concept ;
    dcterms:created "2017-11-16"^^xsd:date ;
    dcterms:creator <https://linked.data.gov.au/org/neii> ;
    skos:definition "Groundwater levels, as measured in a bore."@en ;
    skos:inScheme cs: ;
    skos:prefLabel "groundwater level"@en ;
    skos:topConceptOf cs: ;
.

:groundwater-management-area
    a skos:Concept ;
    dcterms:created "2017-11-16"^^xsd:date ;
    dcterms:creator <https://linked.data.gov.au/org/neii> ;
    skos:altLabel "GMA"@en ;
    skos:definition "An area of land that is appointed as an area within which there are rules for managing groundwater."@en ;
    skos:inScheme cs: ;
    skos:notation "GMA" ;
    skos:prefLabel "groundwater management area"@en ;
    skos:topConceptOf cs: ;
.

:hydrogeology
    a skos:Concept ;
    dcterms:created "2017-11-16"^^xsd:date ;
    dcterms:creator <https://linked.data.gov.au/org/neii> ;
    skos:definition "The hydrological and geological science concerned with the occurrence, distribution, quality and movement of groundwater, especially relating to the distribution of aquifers, groundwater flow and groundwater quality."@en ;
    skos:inScheme cs: ;
    skos:prefLabel "hydrogeology"@en ;
    skos:topConceptOf cs: ;
.

:licensed-groundwater-entitlement
    a skos:Concept ;
    dcterms:created "2017-11-16"^^xsd:date ;
    dcterms:creator <https://linked.data.gov.au/org/neii> ;
    skos:definition "A specific volume of water licensed to an individual or business for extraction in a given period (typically annually), according to rules established in the relevant groundwater plan."@en ;
    skos:inScheme cs: ;
    skos:prefLabel "licensed groundwater entitlement"@en ;
    skos:topConceptOf cs: ;
.

:not-available
    a skos:Concept ;
    dcterms:created "2017-11-21"^^xsd:date ;
    dcterms:creator <https://linked.data.gov.au/org/neii> ;
    dcterms:modified "2017-11-21"^^xsd:date ;
    skos:altLabel "NA"@en ;
    skos:definition "No data is currently available."@en ;
    skos:inScheme cs: ;
    skos:notation "NA" ;
    skos:prefLabel "not available"@en ;
    skos:topConceptOf cs: ;
.

:salinity
    a skos:Concept ;
    dcterms:created "2017-11-16"^^xsd:date ;
    dcterms:creator <https://linked.data.gov.au/org/neii> ;
    skos:definition "The concentration of soluble salts in a solution, soil or other medium."@en ;
    skos:inScheme cs: ;
    skos:prefLabel "salinity"@en ;
    skos:topConceptOf cs: ;
.

:stock-and-domestic-bores
    a skos:Concept ;
    dcterms:created "2017-11-16"^^xsd:date ;
    dcterms:creator <https://linked.data.gov.au/org/neii> ;
    skos:definition "Bores drilled for extracting groundwater for the purpose of watering stock or to use domestically. Groundwater extracted for these purposes does not require a licence in most regions."@en ;
    skos:inScheme cs: ;
    skos:prefLabel "stock and domestic bores"@en ;
    skos:topConceptOf cs: ;
.

:sustainable-diversion-limit
    a skos:Concept ;
    dcterms:created "2017-11-16"^^xsd:date ;
    dcterms:creator <https://linked.data.gov.au/org/neii> ;
    skos:altLabel "SDL"@en ;
    skos:definition "The Sustainable Diversion Limit specifies how much water can be sustainably taken from a catchment, aquifer or basin as a long term annual extraction volume. Each SDL is defined in the Murray Darling Basin Plan."@en ;
    skos:inScheme cs: ;
    skos:notation "SDL" ;
    skos:prefLabel "sustainable diversion limit"@en ;
    skos:topConceptOf cs: ;
.

:unconfined-aquifer
    a skos:Concept ;
    dcterms:created "2017-11-16"^^xsd:date ;
    dcterms:creator <https://linked.data.gov.au/org/neii> ;
    skos:definition "An aquifer whose upper surface is a water table free to fluctuate in equilibrium with atmospheric pressure."@en ;
    skos:inScheme cs: ;
    skos:prefLabel "unconfined aquifer"@en ;
    skos:topConceptOf cs: ;
.

:watertable
    a skos:Concept ;
    dcterms:created "2017-11-16"^^xsd:date ;
    dcterms:creator <https://linked.data.gov.au/org/neii> ;
    skos:definition "The surface in an unconfined aquifer or confining bed below which the ground is saturated with water."@en ;
    skos:inScheme cs: ;
    skos:prefLabel "watertable"@en ;
    skos:topConceptOf cs: ;
.

<https://linked.data.gov.au/org/bom-gu>
    a dcterms:Agent ;
    schema:name "Groundwater Unit, Bureau of Meteorology" ;
    schema:url "http://www.bom.gov.au/water/groundwater/"^^xsd:anyURI ;
.

cs:
    a skos:ConceptScheme ;
    dcterms:created "2017-11-16"^^xsd:date ;
    dcterms:creator <https://linked.data.gov.au/org/bom-gu> ;
    dcterms:issued "2015-11" ;
    dcterms:modified "2024-04-15"^^xsd:date ;
    dcterms:publisher <https://linked.data.gov.au/org/bom-gu> ;
    dcterms:subject "Groundwater"@en ;
    owl:versionInfo "Version 1" ;
    skos:definition "The Australian Groundwater Insight is a user-friendly web mapping application designed for non-experts in government, policy development and the general public.  The Insight shows hydrogeological information alongside information about licences, entitlements, bore density, groundwater management areas and salinity. The Insight also presents trends in groundwater levels over time and recent groundwater levels compared to the long-term average. "@en ;
    skos:hasTopConcept
        :aquifer ,
        :bedrock ,
        :bore ,
        :bore-density ,
        :confined-aquifer ,
        :groundwater-entitlement-limit ,
        :groundwater-level ,
        :groundwater-management-area ,
        :hydrogeology ,
        :licensed-groundwater-entitlement ,
        :not-available ,
        :salinity ,
        :stock-and-domestic-bores ,
        :sustainable-diversion-limit ,
        :unconfined-aquifer ,
        :watertable ;
    skos:historyNote "2024-04: IRIs changed from http://www.neii.gov.au/def/voc/GW/australian-groundwater-insight/Australian-Groundwater-Insight for the ConceptScheme and http://www.neii.gov.au/def/voc/GW/australian-groundwater-insight/ for the Concept namespace to linked.data.gov.au-based IRIs" ;
    skos:prefLabel "Australian Groundwater Insight"@en ;
.
