PREFIX : <https://linked.data.gov.au/def/neii-observation-method/>
PREFIX cs: <https://linked.data.gov.au/def/neii-observation-method>
PREFIX dcterms: <http://purl.org/dc/terms/>
PREFIX owl: <http://www.w3.org/2002/07/owl#>
PREFIX rdfs: <http://www.w3.org/2000/01/rdf-schema#>
PREFIX schema: <https://schema.org/>
PREFIX skos: <http://www.w3.org/2004/02/skos/core#>
PREFIX xsd: <http://www.w3.org/2001/XMLSchema#>

:NEII-Observation-method
    a rdfs:Resource ;
    owl:deprecated true ;
    skos:prefLabel "NEII Observation method"@en ;
.

:aircraftOrAirborne
    a skos:Concept ;
    dcterms:created "2017-08-10"^^xsd:date ;
    dcterms:creator <https://linked.data.gov.au/org/neii> ;
    owl:deprecated true ;
    skos:definition "The network uses aircraft, balloons, rockets or other airborne instrumentation"@en ;
    skos:inScheme cs: ;
    skos:prefLabel "aircraftOrAirborne"@en ;
    skos:topConceptOf cs: ;
.

:earthObservationSatellites
    a skos:Concept ;
    dcterms:created "2017-08-10"^^xsd:date ;
    dcterms:creator <https://linked.data.gov.au/org/neii> ;
    owl:deprecated true ;
    skos:definition "The network uses earth observation satellites (for example, LANDSAT, MODIS)"@en ;
    skos:inScheme cs: ;
    skos:prefLabel "earthObservationSatellites"@en ;
    skos:topConceptOf cs: ;
.

:humanAssessment
    a skos:Concept ;
    dcterms:created "2017-08-10"^^xsd:date ;
    dcterms:creator <https://linked.data.gov.au/org/neii> ;
    owl:deprecated true ;
    skos:definition "The network uses human assessments or surveys (for example species counts and vegetation canopy cover estimates completed by a botanist, human observation of animal movement)."@en ;
    skos:inScheme cs: ;
    skos:prefLabel "humanAssessment"@en ;
    skos:topConceptOf cs: ;
.

:inSituHydroBasedPlatforms
    a skos:Concept ;
    dcterms:created "2017-08-10"^^xsd:date ;
    dcterms:creator <https://linked.data.gov.au/org/neii> ;
    owl:deprecated true ;
    skos:definition "The network uses in-situ hydrological-based platforms (for example, streamflow gauges, water quality sensors)."@en ;
    skos:inScheme cs: ;
    skos:prefLabel "inSituHydroBasedPlatforms"@en ;
    skos:topConceptOf cs: ;
.

:inSituLandBasedPlatforms
    a skos:Concept ;
    dcterms:created "2017-08-10"^^xsd:date ;
    dcterms:creator <https://linked.data.gov.au/org/neii> ;
    owl:deprecated true ;
    skos:definition "The network uses in-situ land-based platforms (for example, weather stations, air monitoring stations, or seismological stations)."@en ;
    skos:inScheme cs: ;
    skos:prefLabel "inSituLandBasedPlatforms"@en ;
    skos:topConceptOf cs: ;
.

:inSituOceanBasedPlatforms
    a skos:Concept ;
    dcterms:created "2017-08-10"^^xsd:date ;
    dcterms:creator <https://linked.data.gov.au/org/neii> ;
    owl:deprecated true ;
    skos:definition "The network uses in-situ ocean-based platforms (for example, ships, buoys, or moorings)."@en ;
    skos:inScheme cs: ;
    skos:prefLabel "inSituOceanBasedPlatforms"@en ;
    skos:topConceptOf cs: ;
.

:modelsOrAnalysis
    a skos:Concept ;
    dcterms:created "2017-08-10"^^xsd:date ;
    dcterms:creator <https://linked.data.gov.au/org/neii> ;
    owl:deprecated true ;
    skos:definition "The network uses models or data analysis (for example, climate models, soil models, or land surface models)."@en ;
    skos:inScheme cs: ;
    skos:prefLabel "modelsOrAnalysis"@en ;
    skos:topConceptOf cs: ;
.

:navigationPlatforms
    a skos:Concept ;
    dcterms:created "2017-08-10"^^xsd:date ;
    dcterms:creator <https://linked.data.gov.au/org/neii> ;
    owl:deprecated true ;
    skos:definition "The network uses navigation platforms (for example, Global Positioning System, NAVSTAR, or GLONASS)."@en ;
    skos:inScheme cs: ;
    skos:prefLabel "navigationPlatforms"@en ;
    skos:topConceptOf cs: ;
.

<https://linked.data.gov.au/org/neii>
    a
        dcterms:Agent ,
        schema:Organization ;
    dcterms:modified "2017-08-09"^^xsd:date ;
    schema:name "National Environmental Information Infrastructure (NEII)" ;
    schema:url "http://www.bom.gov.au/environment/transition.shtml"^^xsd:anyURI ;
.

cs:
    a skos:ConceptScheme ;
    dcterms:created "2017-08-10"^^xsd:date ;
    dcterms:creator <https://linked.data.gov.au/org/neii> ;
    dcterms:issued "2016-09-01" ;
    dcterms:modified "2024-04-15"^^xsd:date ;
    dcterms:publisher <https://linked.data.gov.au/org/neii> ;
    dcterms:subject "NEII"@en ;
    owl:versionInfo "Version 1" ;
    skos:definition "Observation method is a high-level classification of the method used to make environmental observations. The initial list of methods is based on a subset of NASA's Global Change Master Directory (GCMD) Platforms keyword list (http://gcmd.nasa.gov/learn/keyword_list.html)."@en ;
    skos:hasTopConcept
        :aircraftOrAirborne ,
        :earthObservationSatellites ,
        :humanAssessment ,
        :inSituHydroBasedPlatforms ,
        :inSituLandBasedPlatforms ,
        :inSituOceanBasedPlatforms ,
        :modelsOrAnalysis ,
        :navigationPlatforms ;
    skos:historyNote "2024-04: IRIs changed from http://www.neii.gov.au/def/voc/NEII/neii-observation-method/NEII-Observation-Method for the ConceptScheme and http://www.neii.gov.au/def/voc/NEII/neii-observation-method/ for the Concept namespace to linked.data.gov.au-based IRIs" ;
    skos:prefLabel "NEII Observation Method"@en ;
.
