PREFIX dcterms: <http://purl.org/dc/terms/>
PREFIX foaf: <http://xmlns.com/foaf/0.1/>
PREFIX owl: <http://www.w3.org/2002/07/owl#>
PREFIX rdf: <http://www.w3.org/1999/02/22-rdf-syntax-ns#>
PREFIX rdfs: <http://www.w3.org/2000/01/rdf-schema#>
PREFIX schema: <https://schema.org/>
PREFIX skos: <http://www.w3.org/2004/02/skos/core#>
PREFIX xsd: <http://www.w3.org/2001/XMLSchema#>

<http://editor.vocabs.ands.org.au/user/Water-Program,-Bureau-of-Meteorology>
    a dcterms:Agent ;
    foaf:name "Water Program, Bureau of Meteorology" ;
.

<http://www.neii.gov.au/def/voc/waterprogram/water-regulations-2008-water-information-terms>
    a rdfs:Resource ;
    dcterms:contributor <https://linked.data.gov.au/org/neii> ;
.

<http://www.neii.gov.au/def/voc/waterprogram/water-regulations-2008-water-information-terms/Australian-water-access-entitlement>
    a skos:Concept ;
    dcterms:contributor <https://linked.data.gov.au/org/neii> ;
    dcterms:created "2020-05-18"^^xsd:date ;
    dcterms:creator <https://linked.data.gov.au/org/neii> ;
    dcterms:modified "2020-05-18"^^xsd:date ;
    skos:definition """A perpetual or ongoing entitlement, by or under a law of a State, to exclusive access to a share of the water resources of a water resource plan area or other water management area.
Source: Water Regulations 2008 (https://www.legislation.gov.au/Series/F2008L02170) Schedule 3 Part 1."""@en ;
    skos:notation "1" ;
    skos:prefLabel "Australian water access entitlement"@en ;
    skos:topConceptOf <http://www.neii.gov.au/def/voc/waterprogram/water-regulations-2008-water-information-terms/Water-Regulations-2008-water-information-terms> ;
.

<http://www.neii.gov.au/def/voc/waterprogram/water-regulations-2008-water-information-terms/Australian-water-allocation>
    a skos:Concept ;
    dcterms:contributor <https://linked.data.gov.au/org/neii> ;
    dcterms:created "2020-05-18"^^xsd:date ;
    dcterms:creator <https://linked.data.gov.au/org/neii> ;
    dcterms:modified "2020-05-18"^^xsd:date ;
    skos:definition """The specific volume of water allocated to an Australian water access entitlement in a given water accounting period.
Source: Water Regulations 2008 (https://www.legislation.gov.au/Series/F2008L02170) Schedule 3 Part 1."""@en ;
    skos:notation "2" ;
    skos:prefLabel "Australian water allocation"@en ;
    skos:topConceptOf <http://www.neii.gov.au/def/voc/waterprogram/water-regulations-2008-water-information-terms/Water-Regulations-2008-water-information-terms> ;
.

<http://www.neii.gov.au/def/voc/waterprogram/water-regulations-2008-water-information-terms/Category>
    a skos:Concept ;
    dcterms:contributor <https://linked.data.gov.au/org/neii> ;
    dcterms:created "2020-05-18"^^xsd:date ;
    dcterms:creator <https://linked.data.gov.au/org/neii> ;
    dcterms:modified "2020-05-18"^^xsd:date ;
    skos:definition "In relation to water information, means a category of water information specified in regulation 7.03."@en ;
    skos:notation "7" ;
    skos:prefLabel "Category"@en ;
    skos:topConceptOf <http://www.neii.gov.au/def/voc/waterprogram/water-regulations-2008-water-information-terms/Water-Regulations-2008-water-information-terms> ;
.

<http://www.neii.gov.au/def/voc/waterprogram/water-regulations-2008-water-information-terms/Category-A-person>
    a skos:Concept ;
    dcterms:contributor <https://linked.data.gov.au/org/neii> ;
    dcterms:created "2020-05-18"^^xsd:date ;
    dcterms:creator <https://linked.data.gov.au/org/neii> ;
    dcterms:modified "2020-05-18"^^xsd:date ;
    skos:definition """A person specified as a Category A person in the document titled Persons and Classes of Persons (http://www.bom.gov.au/water/regulations/schedules/classesOfPerson.shtml)
Source: Water Regulations 2008 (https://www.legislation.gov.au/Series/F2008L02170) Regulation 1.03."""@en ;
    skos:notation "18" ;
    skos:prefLabel "Category A person"@en ;
    skos:topConceptOf <http://www.neii.gov.au/def/voc/waterprogram/water-regulations-2008-water-information-terms/Water-Regulations-2008-water-information-terms> ;
.

<http://www.neii.gov.au/def/voc/waterprogram/water-regulations-2008-water-information-terms/Category-B-person>
    a skos:Concept ;
    dcterms:contributor <https://linked.data.gov.au/org/neii> ;
    dcterms:created "2020-05-18"^^xsd:date ;
    dcterms:creator <https://linked.data.gov.au/org/neii> ;
    dcterms:modified "2020-05-18"^^xsd:date ;
    skos:definition """A person specified as a Category B person in the document titled Persons and Classes of Persons (http://www.bom.gov.au/water/regulations/schedules/classesOfPerson.shtml)
Source: Water Regulations 2008 (https://www.legislation.gov.au/Series/F2008L02170) Regulation 1.03."""@en ;
    skos:notation "19" ;
    skos:prefLabel "Category B person"@en ;
    skos:topConceptOf <http://www.neii.gov.au/def/voc/waterprogram/water-regulations-2008-water-information-terms/Water-Regulations-2008-water-information-terms> ;
.

<http://www.neii.gov.au/def/voc/waterprogram/water-regulations-2008-water-information-terms/Category-C-person>
    a skos:Concept ;
    dcterms:contributor <https://linked.data.gov.au/org/neii> ;
    dcterms:created "2020-05-18"^^xsd:date ;
    dcterms:creator <https://linked.data.gov.au/org/neii> ;
    dcterms:modified "2020-05-18"^^xsd:date ;
    skos:definition """A person specified as a Category C person in the document titled Persons and Classes of Persons (http://www.bom.gov.au/water/regulations/schedules/classesOfPerson.shtml)
Source: Water Regulations 2008 (https://www.legislation.gov.au/Series/F2008L02170) Regulation 1.03."""@en ;
    skos:notation "20" ;
    skos:prefLabel "Category C person"@en ;
    skos:topConceptOf <http://www.neii.gov.au/def/voc/waterprogram/water-regulations-2008-water-information-terms/Water-Regulations-2008-water-information-terms> ;
.

<http://www.neii.gov.au/def/voc/waterprogram/water-regulations-2008-water-information-terms/Category-D-person>
    a skos:Concept ;
    dcterms:contributor <https://linked.data.gov.au/org/neii> ;
    dcterms:created "2020-05-18"^^xsd:date ;
    dcterms:creator <https://linked.data.gov.au/org/neii> ;
    dcterms:modified "2020-05-18"^^xsd:date ;
    skos:definition """A person specified as a Category D person in the document titled Persons and Classes of Persons (http://www.bom.gov.au/water/regulations/schedules/classesOfPerson.shtml)
Source: Water Regulations 2008 (https://www.legislation.gov.au/Series/F2008L02170) Regulation 1.03."""@en ;
    skos:notation "21" ;
    skos:prefLabel "Category D person"@en ;
    skos:topConceptOf <http://www.neii.gov.au/def/voc/waterprogram/water-regulations-2008-water-information-terms/Water-Regulations-2008-water-information-terms> ;
.

<http://www.neii.gov.au/def/voc/waterprogram/water-regulations-2008-water-information-terms/Category-E-person>
    a skos:Concept ;
    dcterms:contributor <https://linked.data.gov.au/org/neii> ;
    dcterms:created "2020-05-18"^^xsd:date ;
    dcterms:creator <https://linked.data.gov.au/org/neii> ;
    dcterms:modified "2020-05-18"^^xsd:date ;
    skos:definition """A person specified as a Category E person in the document titled Persons and Classes of Persons (http://www.bom.gov.au/water/regulations/schedules/classesOfPerson.shtml)
Source: Water Regulations 2008 (https://www.legislation.gov.au/Series/F2008L02170) Regulation 1.03."""@en ;
    skos:notation "22" ;
    skos:prefLabel "Category E person"@en ;
    skos:topConceptOf <http://www.neii.gov.au/def/voc/waterprogram/water-regulations-2008-water-information-terms/Water-Regulations-2008-water-information-terms> ;
.

<http://www.neii.gov.au/def/voc/waterprogram/water-regulations-2008-water-information-terms/Category-F-person>
    a skos:Concept ;
    dcterms:contributor <https://linked.data.gov.au/org/neii> ;
    dcterms:created "2020-05-18"^^xsd:date ;
    dcterms:creator <https://linked.data.gov.au/org/neii> ;
    dcterms:modified "2020-05-18"^^xsd:date ;
    skos:definition """A person specified as a Category F person in the document titled Persons and Classes of Persons (http://www.bom.gov.au/water/regulations/schedules/classesOfPerson.shtml)
Source: Water Regulations 2008 (https://www.legislation.gov.au/Series/F2008L02170) Regulation 1.03."""@en ;
    skos:notation "23" ;
    skos:prefLabel "Category F person"@en ;
    skos:topConceptOf <http://www.neii.gov.au/def/voc/waterprogram/water-regulations-2008-water-information-terms/Water-Regulations-2008-water-information-terms> ;
.

<http://www.neii.gov.au/def/voc/waterprogram/water-regulations-2008-water-information-terms/Category-G-person>
    a skos:Concept ;
    dcterms:contributor <https://linked.data.gov.au/org/neii> ;
    dcterms:created "2020-05-18"^^xsd:date ;
    dcterms:creator <https://linked.data.gov.au/org/neii> ;
    dcterms:modified "2020-05-18"^^xsd:date ;
    skos:definition """A person specified as a Category G person in the document titled Persons and Classes of Persons (http://www.bom.gov.au/water/regulations/schedules/classesOfPerson.shtml)
Source: Water Regulations 2008 (https://www.legislation.gov.au/Series/F2008L02170) Regulation 1.03."""@en ;
    skos:notation "24" ;
    skos:prefLabel "Category G person"@en ;
    skos:topConceptOf <http://www.neii.gov.au/def/voc/waterprogram/water-regulations-2008-water-information-terms/Water-Regulations-2008-water-information-terms> ;
.

<http://www.neii.gov.au/def/voc/waterprogram/water-regulations-2008-water-information-terms/Category-H-person>
    a skos:Concept ;
    dcterms:contributor <https://linked.data.gov.au/org/neii> ;
    dcterms:created "2020-05-18"^^xsd:date ;
    dcterms:creator <https://linked.data.gov.au/org/neii> ;
    dcterms:modified "2020-05-18"^^xsd:date ;
    skos:definition """A person specified as a Category H person in the document titled Persons and Classes of Persons (http://www.bom.gov.au/water/regulations/schedules/classesOfPerson.shtml)
Source: Water Regulations 2008 (https://www.legislation.gov.au/Series/F2008L02170) Regulation 1.03."""@en ;
    skos:notation "25" ;
    skos:prefLabel "Category H person"@en ;
    skos:topConceptOf <http://www.neii.gov.au/def/voc/waterprogram/water-regulations-2008-water-information-terms/Water-Regulations-2008-water-information-terms> ;
.

<http://www.neii.gov.au/def/voc/waterprogram/water-regulations-2008-water-information-terms/Category-K-person>
    a skos:Concept ;
    dcterms:contributor <https://linked.data.gov.au/org/neii> ;
    dcterms:created "2020-05-18"^^xsd:date ;
    dcterms:creator <https://linked.data.gov.au/org/neii> ;
    dcterms:modified "2020-05-18"^^xsd:date ;
    skos:definition """A person specified as a Category K person in the document titled Persons and Classes of Persons (http://www.bom.gov.au/water/regulations/schedules/classesOfPerson.shtml)
Source: Water Regulations 2008 (https://www.legislation.gov.au/Series/F2008L02170) Regulation 1.03."""@en ;
    skos:notation "26" ;
    skos:prefLabel "Category K person"@en ;
    skos:topConceptOf <http://www.neii.gov.au/def/voc/waterprogram/water-regulations-2008-water-information-terms/Water-Regulations-2008-water-information-terms> ;
.

<http://www.neii.gov.au/def/voc/waterprogram/water-regulations-2008-water-information-terms/Category-L-person>
    a skos:Concept ;
    dcterms:contributor <https://linked.data.gov.au/org/neii> ;
    dcterms:created "2020-05-18"^^xsd:date ;
    dcterms:creator <https://linked.data.gov.au/org/neii> ;
    dcterms:modified "2020-05-18"^^xsd:date ;
    skos:definition """A person specified as a Category L person in the document titled Persons and Classes of Persons (http://www.bom.gov.au/water/regulations/schedules/classesOfPerson.shtml)
Source: Water Regulations 2008 (https://www.legislation.gov.au/Series/F2008L02170) Regulation 1.03(1)."""@en ;
    skos:notation "27" ;
    skos:prefLabel "Category L person"@en ;
    skos:topConceptOf <http://www.neii.gov.au/def/voc/waterprogram/water-regulations-2008-water-information-terms/Water-Regulations-2008-water-information-terms> ;
.

<http://www.neii.gov.au/def/voc/waterprogram/water-regulations-2008-water-information-terms/Category-M-person>
    a skos:Concept ;
    dcterms:contributor <https://linked.data.gov.au/org/neii> ;
    dcterms:created "2020-05-18"^^xsd:date ;
    dcterms:creator <https://linked.data.gov.au/org/neii> ;
    dcterms:modified "2020-05-18"^^xsd:date ;
    skos:definition """A person specified as a Category M person in the document titled Persons and Classes of Persons (http://www.bom.gov.au/water/regulations/schedules/classesOfPerson.shtml)
Source: Water Regulations 2008 (https://www.legislation.gov.au/Series/F2008L02170) Regulation 1.03(1)."""@en ;
    skos:notation "28" ;
    skos:prefLabel "Category M person"@en ;
    skos:topConceptOf <http://www.neii.gov.au/def/voc/waterprogram/water-regulations-2008-water-information-terms/Water-Regulations-2008-water-information-terms> ;
.

<http://www.neii.gov.au/def/voc/waterprogram/water-regulations-2008-water-information-terms/Irrigation-water-scheme>
    a skos:Concept ;
    dcterms:contributor <https://linked.data.gov.au/org/neii> ;
    dcterms:created "2020-05-18"^^xsd:date ;
    dcterms:creator <https://linked.data.gov.au/org/neii> ;
    dcterms:modified "2020-05-18"^^xsd:date ;
    skos:definition "The water service infrastructure for delivering water for the primary purpose of being used for irrigation."@en ;
    skos:notation "46" ;
    skos:prefLabel "Irrigation water scheme"@en ;
    skos:topConceptOf <http://www.neii.gov.au/def/voc/waterprogram/water-regulations-2008-water-information-terms/Water-Regulations-2008-water-information-terms> ;
.

<http://www.neii.gov.au/def/voc/waterprogram/water-regulations-2008-water-information-terms/Major-storage>
    a skos:Concept ;
    dcterms:contributor <https://linked.data.gov.au/org/neii> ;
    dcterms:created "2020-05-18"^^xsd:date ;
    dcterms:creator <https://linked.data.gov.au/org/neii> ;
    dcterms:modified "2020-05-18"^^xsd:date ;
    skos:definition """Any water storage that has a total storage capacity of 1000 million litres or more.
Source: Water Regulations 2008 (https://www.legislation.gov.au/Series/F2008L02170) Schedule 3 Part 1."""@en ;
    skos:notation "47" ;
    skos:prefLabel "Major storage"@en ;
    skos:topConceptOf <http://www.neii.gov.au/def/voc/waterprogram/water-regulations-2008-water-information-terms/Water-Regulations-2008-water-information-terms> ;
.

<http://www.neii.gov.au/def/voc/waterprogram/water-regulations-2008-water-information-terms/Minor-storage>
    a skos:Concept ;
    dcterms:contributor <https://linked.data.gov.au/org/neii> ;
    dcterms:created "2020-05-18"^^xsd:date ;
    dcterms:creator <https://linked.data.gov.au/org/neii> ;
    dcterms:modified "2020-05-18"^^xsd:date ;
    skos:definition """Any water storage in which water is stored for taking and that meets the following  criteria: (a) it is not a major storage; (b) it has a storage capacity of 100 million litres or more; (c) it is not used primarily for the precipitation of ash; (d) it is not a mine tailings dam; (e) it is not managed by an urban infrastructure operator primarily for the purpose of flood management or pollution abatement.
Source: Water Regulations 2008 (https://www.legislation.gov.au/Series/F2008L02170) Schedule 3 Part 1."""@en ;
    skos:notation "48" ;
    skos:prefLabel "Minor storage"@en ;
    skos:topConceptOf <http://www.neii.gov.au/def/voc/waterprogram/water-regulations-2008-water-information-terms/Water-Regulations-2008-water-information-terms> ;
.

<http://www.neii.gov.au/def/voc/waterprogram/water-regulations-2008-water-information-terms/State-NGIS-information>
    a skos:Concept ;
    dcterms:contributor <https://linked.data.gov.au/org/neii> ;
    dcterms:created "2020-05-18"^^xsd:date ;
    dcterms:creator <https://linked.data.gov.au/org/neii> ;
    dcterms:modified "2020-05-18"^^xsd:date ;
    skos:definition """Any water information in a State's National Groundwater Information System (NGIS) database.
Source: Water Regulations 2008 (https://www.legislation.gov.au/Series/F2008L02170) Schedule 3 Part 1."""@en ;
    skos:notation "61" ;
    skos:prefLabel "State NGIS information"@en ;
    skos:topConceptOf <http://www.neii.gov.au/def/voc/waterprogram/water-regulations-2008-water-information-terms/Water-Regulations-2008-water-information-terms> ;
.

<http://www.neii.gov.au/def/voc/waterprogram/water-regulations-2008-water-information-terms/State-aquifer-framework-information>
    a skos:Concept ;
    dcterms:contributor <https://linked.data.gov.au/org/neii> ;
    dcterms:created "2020-05-18"^^xsd:date ;
    dcterms:creator <https://linked.data.gov.au/org/neii> ;
    dcterms:modified "2020-05-18"^^xsd:date ;
    skos:definition """Any water information in the aquifer framework used by a State.
Source: Water Regulations 2008 (https://www.legislation.gov.au/Series/F2008L02170) Schedule 3 Part 1."""@en ;
    skos:notation "60" ;
    skos:prefLabel "State aquifer framework information"@en ;
    skos:topConceptOf <http://www.neii.gov.au/def/voc/waterprogram/water-regulations-2008-water-information-terms/Water-Regulations-2008-water-information-terms> ;
.

<http://www.neii.gov.au/def/voc/waterprogram/water-regulations-2008-water-information-terms/U-code>
    a skos:Concept ;
    dcterms:contributor <https://linked.data.gov.au/org/neii> ;
    dcterms:created "2020-05-18"^^xsd:date ;
    dcterms:creator <https://linked.data.gov.au/org/neii> ;
    dcterms:modified "2020-05-19"^^xsd:date ;
    skos:definition """A detailed component water volumes describing the availability, movement and use of water within urban water systems.  Typically, U code volumes are at the plant or transfer party scale and provide a detailed breakdown of W indicator volumes.
Source: Category 7 Reporting Handbook"""@en ;
    skos:notation "126" ;
    skos:prefLabel "U code"@en ;
    skos:topConceptOf <http://www.neii.gov.au/def/voc/waterprogram/water-regulations-2008-water-information-terms/Water-Regulations-2008-water-information-terms> ;
.

<http://www.neii.gov.au/def/voc/waterprogram/water-regulations-2008-water-information-terms/W-indicator>
    a skos:Concept ;
    dcterms:contributor <https://linked.data.gov.au/org/neii> ;
    dcterms:created "2020-05-18"^^xsd:date ;
    dcterms:creator <https://linked.data.gov.au/org/neii> ;
    dcterms:modified "2020-05-19"^^xsd:date ;
    skos:definition """A component water volumes describing the availability, movement and use of water within urban water systems. W indicators are the water resources indicators used to compile the urban National Performance Report.  W indicator volumes are at the scale of the urban National Performance Reporting regions.
Source: Category 7 Reporting Handbook"""@en ;
    skos:notation "146" ;
    skos:prefLabel "W indicator"@en ;
    skos:topConceptOf <http://www.neii.gov.au/def/voc/waterprogram/water-regulations-2008-water-information-terms/Water-Regulations-2008-water-information-terms> ;
.

<http://www.neii.gov.au/def/voc/waterprogram/water-regulations-2008-water-information-terms/bulk-water-charge>
    a skos:Concept ;
    dcterms:contributor <https://linked.data.gov.au/org/neii> ;
    dcterms:created "2020-05-18"^^xsd:date ;
    dcterms:creator <https://linked.data.gov.au/org/neii> ;
    dcterms:modified "2020-05-18"^^xsd:date ;
    skos:definition """A charge payable for the storage of water for, and the delivery of water to, any of the following:
(a) infrastructure operators;
(b) other operators of reticulated water systems;
(c) other persons prescribed by the regulations for the purposes of this paragraph.
In the Regulation 1.05A, a person is prescribed for the above paragraph (c) if:
(a) the person diverts water directly from a watercourse for the person's use, including for one of the following purposes:
(i) agricultural purposes;
(ii) industrial purposes;
(iii) irrigation;
(iv) stock and domestic water use; and
(b) the water is made available through a bulk water service.
Source: Derived from Water Act 2007 (https://www.legislation.gov.au/Details/C2018C00505) Part 1 Section 4 and Water Regulations 2008 (https://www.legislation.gov.au/Series/F2008L02170) Regulation 1.05A, at 8 February 2019."""@en ;
    skos:notation "3" ;
    skos:prefLabel "bulk water charge"@en ;
    skos:topConceptOf <http://www.neii.gov.au/def/voc/waterprogram/water-regulations-2008-water-information-terms/Water-Regulations-2008-water-information-terms> ;
.

<http://www.neii.gov.au/def/voc/waterprogram/water-regulations-2008-water-information-terms/bulk-water-service>
    a skos:Concept ;
    dcterms:contributor <https://linked.data.gov.au/org/neii> ;
    dcterms:created "2020-05-18"^^xsd:date ;
    dcterms:creator <https://linked.data.gov.au/org/neii> ;
    dcterms:modified "2020-05-18"^^xsd:date ;
    skos:definition """Means one or more of the following:
(a) a service that is provided for the storage of water that is primarily stored on-river;
(b) a service that is provided for the storage of water that is primarily delivered on-river."""@en ;
    skos:notation "4" ;
    skos:prefLabel "bulk water service"@en ;
    skos:topConceptOf <http://www.neii.gov.au/def/voc/waterprogram/water-regulations-2008-water-information-terms/Water-Regulations-2008-water-information-terms> ;
.

<http://www.neii.gov.au/def/voc/waterprogram/water-regulations-2008-water-information-terms/bulk-water-supplier>
    a skos:Concept ;
    dcterms:contributor <https://linked.data.gov.au/org/neii> ;
    dcterms:created "2020-05-18"^^xsd:date ;
    dcterms:creator <https://linked.data.gov.au/org/neii> ;
    dcterms:modified "2020-05-18"^^xsd:date ;
    skos:definition """An entity who imposes a bulk water charge for a bulk water service.
Source: Water Regulations 2008 (https://www.legislation.gov.au/Series/F2008L02170) Regulation 4.01A."""@en ;
    skos:notation "5" ;
    skos:prefLabel "bulk water supplier"@en ;
    skos:topConceptOf <http://www.neii.gov.au/def/voc/waterprogram/water-regulations-2008-water-information-terms/Water-Regulations-2008-water-information-terms> ;
.

<http://www.neii.gov.au/def/voc/waterprogram/water-regulations-2008-water-information-terms/calendar-month>
    a skos:Concept ;
    dcterms:contributor <https://linked.data.gov.au/org/neii> ;
    dcterms:created "2020-05-18"^^xsd:date ;
    dcterms:creator <https://linked.data.gov.au/org/neii> ;
    dcterms:modified "2020-05-18"^^xsd:date ;
    skos:definition """A period commencing at the beginning of a day of one of the 12 months of the year and ending immediately before the beginning of the corresponding day of the next month or, if there is no such corresponding day, ending at the expiration of the next month.
Source: Acts Interpretation Act 1901 (http://www.comlaw.gov.au/Details/C2009C00554) Part V 22"""@en ;
    skos:notation "6" ;
    skos:prefLabel "calendar month"@en ;
    skos:topConceptOf <http://www.neii.gov.au/def/voc/waterprogram/water-regulations-2008-water-information-terms/Water-Regulations-2008-water-information-terms> ;
.

<http://www.neii.gov.au/def/voc/waterprogram/water-regulations-2008-water-information-terms/data-management-system>
    a skos:Concept ;
    dcterms:contributor <https://linked.data.gov.au/org/neii> ;
    dcterms:created "2020-05-18"^^xsd:date ;
    dcterms:creator <https://linked.data.gov.au/org/neii> ;
    dcterms:modified "2020-05-18"^^xsd:date ;
    skos:definition """The software and hardware used to manage the storage of and access to information held in a set of related files.
Source: Water Regulations 2008 (https://www.legislation.gov.au/Series/F2008L02170) Regulation 1.03."""@en ;
    skos:notation "29" ;
    skos:prefLabel "data management system"@en ;
    skos:topConceptOf <http://www.neii.gov.au/def/voc/waterprogram/water-regulations-2008-water-information-terms/Water-Regulations-2008-water-information-terms> ;
.

<http://www.neii.gov.au/def/voc/waterprogram/water-regulations-2008-water-information-terms/day>
    a skos:Concept ;
    dcterms:contributor <https://linked.data.gov.au/org/neii> ;
    dcterms:created "2020-05-18"^^xsd:date ;
    dcterms:creator <https://linked.data.gov.au/org/neii> ;
    dcterms:modified "2020-05-18"^^xsd:date ;
    skos:definition """A period of 24 hours starting at 12:00 midnight.
Source: Water Regulations 2008 (https://www.legislation.gov.au/Series/F2008L02170) Regulation 1.04."""@en ;
    skos:notation "30" ;
    skos:prefLabel "day"@en ;
    skos:topConceptOf <http://www.neii.gov.au/def/voc/waterprogram/water-regulations-2008-water-information-terms/Water-Regulations-2008-water-information-terms> ;
.

<http://www.neii.gov.au/def/voc/waterprogram/water-regulations-2008-water-information-terms/dewpoint-temperature>
    a skos:Concept ;
    dcterms:contributor <https://linked.data.gov.au/org/neii> ;
    dcterms:created "2020-05-18"^^xsd:date ;
    dcterms:creator <https://linked.data.gov.au/org/neii> ;
    dcterms:modified "2020-05-18"^^xsd:date ;
    skos:definition """The temperature to which air must be cooled, at constant pressure and constant moisture content, to reach saturation.
Source: Water Regulations 2008 (https://www.legislation.gov.au/Series/F2008L02170) Schedule 3 Part 1."""@en ;
    skos:notation "31" ;
    skos:prefLabel "dewpoint temperature"@en ;
    skos:topConceptOf <http://www.neii.gov.au/def/voc/waterprogram/water-regulations-2008-water-information-terms/Water-Regulations-2008-water-information-terms> ;
.

<http://www.neii.gov.au/def/voc/waterprogram/water-regulations-2008-water-information-terms/downward-longwave-exposure>
    a skos:Concept ;
    dcterms:contributor <https://linked.data.gov.au/org/neii> ;
    dcterms:created "2020-05-18"^^xsd:date ;
    dcterms:creator <https://linked.data.gov.au/org/neii> ;
    dcterms:modified "2020-05-18"^^xsd:date ;
    skos:definition """The total amount of terrestrial electromagnetic energy that falls on a specified unit horizontal surface.
Source: Water Regulations 2008 (https://www.legislation.gov.au/Series/F2008L02170) Schedule 3 Part 1."""@en ;
    skos:notation "32" ;
    skos:prefLabel "downward longwave exposure"@en ;
    skos:topConceptOf <http://www.neii.gov.au/def/voc/waterprogram/water-regulations-2008-water-information-terms/Water-Regulations-2008-water-information-terms> ;
.

<http://www.neii.gov.au/def/voc/waterprogram/water-regulations-2008-water-information-terms/downward-longwave-irradiance>
    a skos:Concept ;
    dcterms:contributor <https://linked.data.gov.au/org/neii> ;
    dcterms:created "2020-05-18"^^xsd:date ;
    dcterms:creator <https://linked.data.gov.au/org/neii> ;
    dcterms:modified "2020-05-18"^^xsd:date ;
    skos:definition """The longwave irradiance emitted from the sky that falls on a specified unit horizontal surface.
Source: Water Regulations 2008 (https://www.legislation.gov.au/Series/F2008L02170) Schedule 3 Part 1."""@en ;
    skos:notation "33" ;
    skos:prefLabel "downward longwave irradiance"@en ;
    skos:topConceptOf <http://www.neii.gov.au/def/voc/waterprogram/water-regulations-2008-water-information-terms/Water-Regulations-2008-water-information-terms> ;
.

<http://www.neii.gov.au/def/voc/waterprogram/water-regulations-2008-water-information-terms/dry-bulb-air-temperature>
    a skos:Concept ;
    dcterms:contributor <https://linked.data.gov.au/org/neii> ;
    dcterms:created "2020-05-18"^^xsd:date ;
    dcterms:creator <https://linked.data.gov.au/org/neii> ;
    dcterms:modified "2020-05-18"^^xsd:date ;
    skos:definition """The temperature of air, measured by a thermometer freely exposed to the air but shielded from radiation and moisture.
Source: Water Regulations 2008 (https://www.legislation.gov.au/Series/F2008L02170) Schedule 3 Part 1."""@en ;
    skos:notation "34" ;
    skos:prefLabel "dry bulb air temperature"@en ;
    skos:topConceptOf <http://www.neii.gov.au/def/voc/waterprogram/water-regulations-2008-water-information-terms/Water-Regulations-2008-water-information-terms> ;
.

<http://www.neii.gov.au/def/voc/waterprogram/water-regulations-2008-water-information-terms/electrical-conductivity>
    a skos:Concept ;
    dcterms:contributor <https://linked.data.gov.au/org/neii> ;
    dcterms:created "2020-05-18"^^xsd:date ;
    dcterms:creator <https://linked.data.gov.au/org/neii> ;
    dcterms:modified "2020-05-18"^^xsd:date ;
    skos:definition """In relation to water, means the capacity of the water to transmit a flow of electricity, and is a common measure of the salinity of the water.
Source: Water Regulations 2008 (https://www.legislation.gov.au/Series/F2008L02170) Schedule 3 Part 1."""@en ;
    skos:notation "35" ;
    skos:prefLabel "electrical conductivity"@en ;
    skos:topConceptOf <http://www.neii.gov.au/def/voc/waterprogram/water-regulations-2008-water-information-terms/Water-Regulations-2008-water-information-terms> ;
.

<http://www.neii.gov.au/def/voc/waterprogram/water-regulations-2008-water-information-terms/electronic-format>
    a skos:Concept ;
    dcterms:contributor <https://linked.data.gov.au/org/neii> ;
    dcterms:created "2020-05-18"^^xsd:date ;
    dcterms:creator <https://linked.data.gov.au/org/neii> ;
    dcterms:modified "2020-05-18"^^xsd:date ;
    skos:definition """A format that is machine readable, but does not include scanned documents.
Source: Water Regulations 2008 (https://www.legislation.gov.au/Series/F2008L02170) Regulation 1.03."""@en ;
    skos:notation "36" ;
    skos:prefLabel "electronic format"@en ;
    skos:topConceptOf <http://www.neii.gov.au/def/voc/waterprogram/water-regulations-2008-water-information-terms/Water-Regulations-2008-water-information-terms> ;
.

<http://www.neii.gov.au/def/voc/waterprogram/water-regulations-2008-water-information-terms/exposure>
    a skos:Concept ;
    dcterms:contributor <https://linked.data.gov.au/org/neii> ;
    dcterms:created "2020-05-18"^^xsd:date ;
    dcterms:creator <https://linked.data.gov.au/org/neii> ;
    dcterms:modified "2020-05-18"^^xsd:date ;
    skos:definition """The measure of the energy received per unit area.
Source: Water Regulations 2008 (https://www.legislation.gov.au/Series/F2008L02170) Schedule 3 Part 1."""@en ;
    skos:notation "37" ;
    skos:prefLabel "exposure"@en ;
    skos:topConceptOf <http://www.neii.gov.au/def/voc/waterprogram/water-regulations-2008-water-information-terms/Water-Regulations-2008-water-information-terms> ;
.

<http://www.neii.gov.au/def/voc/waterprogram/water-regulations-2008-water-information-terms/global-solar-exposure>
    a skos:Concept ;
    dcterms:contributor <https://linked.data.gov.au/org/neii> ;
    dcterms:created "2020-05-18"^^xsd:date ;
    dcterms:creator <https://linked.data.gov.au/org/neii> ;
    dcterms:modified "2020-05-18"^^xsd:date ;
    skos:definition """The total amount of electromagnetic energy emitted from the sun that falls on a specified unit horizontal surface.
Source: Water Regulations 2008 (https://www.legislation.gov.au/Series/F2008L02170) Schedule 3 Part 1."""@en ;
    skos:notation "38" ;
    skos:prefLabel "global solar exposure"@en ;
    skos:topConceptOf <http://www.neii.gov.au/def/voc/waterprogram/water-regulations-2008-water-information-terms/Water-Regulations-2008-water-information-terms> ;
.

<http://www.neii.gov.au/def/voc/waterprogram/water-regulations-2008-water-information-terms/global-solar-irradiance>
    a skos:Concept ;
    dcterms:contributor <https://linked.data.gov.au/org/neii> ;
    dcterms:created "2020-05-18"^^xsd:date ;
    dcterms:creator <https://linked.data.gov.au/org/neii> ;
    dcterms:modified "2020-05-18"^^xsd:date ;
    skos:definition """The irradiance emitted from the sun that falls on a specified unit horizontal surface.
Source: Water Regulations 2008 (https://www.legislation.gov.au/Series/F2008L02170) Schedule 3 Part 1."""@en ;
    skos:notation "39" ;
    skos:prefLabel "global solar irradiance"@en ;
    skos:topConceptOf <http://www.neii.gov.au/def/voc/waterprogram/water-regulations-2008-water-information-terms/Water-Regulations-2008-water-information-terms> ;
.

<http://www.neii.gov.au/def/voc/waterprogram/water-regulations-2008-water-information-terms/grace-period>
    a skos:Concept ;
    dcterms:contributor <https://linked.data.gov.au/org/neii> ;
    dcterms:created "2020-05-18"^^xsd:date ;
    dcterms:creator <https://linked.data.gov.au/org/neii> ;
    dcterms:modified "2020-05-18"^^xsd:date ;
    skos:definition """The period beginning on the day the person is specified in the new category and ending 3 months after that day.
Source: Water Regulations 2008 (https://www.legislation.gov.au/Series/F2008L02170) Subregulation 7.04(1A)."""@en ;
    skos:notation "40" ;
    skos:prefLabel "grace period"@en ;
    skos:topConceptOf <http://www.neii.gov.au/def/voc/waterprogram/water-regulations-2008-water-information-terms/Water-Regulations-2008-water-information-terms> ;
.

<http://www.neii.gov.au/def/voc/waterprogram/water-regulations-2008-water-information-terms/groundwater>
    a skos:Concept ;
    dcterms:contributor <https://linked.data.gov.au/org/neii> ;
    dcterms:created "2020-05-18"^^xsd:date ;
    dcterms:creator <https://linked.data.gov.au/org/neii> ;
    dcterms:modified "2020-05-18"^^xsd:date ;
    skos:definition """(a) water occurring naturally below ground level (whether in an aquifer or otherwise) or (b) water occurring at a place below ground that has been pumped, diverted or released to that place for the purpose of being stored there.  It does not include water held in underground tanks, pipes or other works.
Source: Water Act 2007 (https://www.legislation.gov.au/Details/C2018C00505) Part 1 Section 4 at 8 February 2019."""@en ;
    skos:notation "41" ;
    skos:prefLabel "groundwater"@en ;
    skos:topConceptOf <http://www.neii.gov.au/def/voc/waterprogram/water-regulations-2008-water-information-terms/Water-Regulations-2008-water-information-terms> ;
.

<http://www.neii.gov.au/def/voc/waterprogram/water-regulations-2008-water-information-terms/hour>
    a skos:Concept ;
    dcterms:contributor <https://linked.data.gov.au/org/neii> ;
    dcterms:created "2020-05-18"^^xsd:date ;
    dcterms:creator <https://linked.data.gov.au/org/neii> ;
    dcterms:modified "2020-05-18"^^xsd:date ;
    skos:definition """A period of 60 minutes starting on the hour (e.g. 12:00).
Source: Water Regulations 2008 (https://www.legislation.gov.au/Series/F2008L02170) Regulation 1.04."""@en ;
    skos:notation "42" ;
    skos:prefLabel "hour"@en ;
    skos:topConceptOf <http://www.neii.gov.au/def/voc/waterprogram/water-regulations-2008-water-information-terms/Water-Regulations-2008-water-information-terms> ;
.

<http://www.neii.gov.au/def/voc/waterprogram/water-regulations-2008-water-information-terms/irradiance>
    a skos:Concept ;
    dcterms:contributor <https://linked.data.gov.au/org/neii> ;
    dcterms:created "2020-05-18"^^xsd:date ;
    dcterms:creator <https://linked.data.gov.au/org/neii> ;
    dcterms:modified "2020-05-18"^^xsd:date ;
    skos:definition """The measure of the rate of electromagnetic energy received per unit area.
Source: Water Regulations 2008 (https://www.legislation.gov.au/Series/F2008L02170) Schedule 3 Part 1."""@en ;
    skos:notation "43" ;
    skos:prefLabel "irradiance"@en ;
    skos:topConceptOf <http://www.neii.gov.au/def/voc/waterprogram/water-regulations-2008-water-information-terms/Water-Regulations-2008-water-information-terms> ;
.

<http://www.neii.gov.au/def/voc/waterprogram/water-regulations-2008-water-information-terms/irrigation-network>
    a skos:Concept ;
    dcterms:contributor <https://linked.data.gov.au/org/neii> ;
    dcterms:created "2020-05-18"^^xsd:date ;
    dcterms:creator <https://linked.data.gov.au/org/neii> ;
    dcterms:modified "2020-05-18"^^xsd:date ;
    skos:definition """The water service infrastructure for delivering water for the primary purpose of being used for irrigation.
Source: Derived from Water Act 2007 (https://www.legislation.gov.au/Details/C2018C00505) Part 1 Section 7 at 8 February 2019."""@en ;
    skos:notation "44" ;
    skos:prefLabel "irrigation network"@en ;
    skos:topConceptOf <http://www.neii.gov.au/def/voc/waterprogram/water-regulations-2008-water-information-terms/Water-Regulations-2008-water-information-terms> ;
.

<http://www.neii.gov.au/def/voc/waterprogram/water-regulations-2008-water-information-terms/irrigation-right>
    a skos:Concept ;
    dcterms:contributor <https://linked.data.gov.au/org/neii> ;
    dcterms:created "2020-05-18"^^xsd:date ;
    dcterms:creator <https://linked.data.gov.au/org/neii> ;
    dcterms:modified "2020-05-18"^^xsd:date ;
    skos:definition """A right that: (a) a person has against an irrigation infrastructure operator to receive water and (b) is not a water access right or a water delivery right.
Source: Water Act 2007 (https://www.legislation.gov.au/Details/C2018C00505) Part 1 Section 4 at 8 February 2019."""@en ;
    skos:notation "45" ;
    skos:prefLabel "irrigation right"@en ;
    skos:topConceptOf <http://www.neii.gov.au/def/voc/waterprogram/water-regulations-2008-water-information-terms/Water-Regulations-2008-water-information-terms> ;
.

<http://www.neii.gov.au/def/voc/waterprogram/water-regulations-2008-water-information-terms/month>
    a skos:Concept ;
    dcterms:contributor <https://linked.data.gov.au/org/neii> ;
    dcterms:created "2020-05-18"^^xsd:date ;
    dcterms:creator <https://linked.data.gov.au/org/neii> ;
    dcterms:modified "2020-05-18"^^xsd:date ;
    skos:definition """One of the 12 months of the calendar year (e.g. January).
Source: Water Regulations 2008 (https://www.legislation.gov.au/Series/F2008L02170) Regulation 1.04."""@en ;
    skos:notation "49" ;
    skos:prefLabel "month"@en ;
    skos:topConceptOf <http://www.neii.gov.au/def/voc/waterprogram/water-regulations-2008-water-information-terms/Water-Regulations-2008-water-information-terms> ;
.

<http://www.neii.gov.au/def/voc/waterprogram/water-regulations-2008-water-information-terms/net-exposure>
    a skos:Concept ;
    dcterms:contributor <https://linked.data.gov.au/org/neii> ;
    dcterms:created "2020-05-18"^^xsd:date ;
    dcterms:creator <https://linked.data.gov.au/org/neii> ;
    dcterms:modified "2020-05-18"^^xsd:date ;
    skos:definition """The net global solar exposure plus the net longwave exposure.
Source: Water Regulations 2008 (https://www.legislation.gov.au/Series/F2008L02170) Schedule 3 Part 1."""@en ;
    skos:notation "50" ;
    skos:prefLabel "net exposure"@en ;
    skos:topConceptOf <http://www.neii.gov.au/def/voc/waterprogram/water-regulations-2008-water-information-terms/Water-Regulations-2008-water-information-terms> ;
.

<http://www.neii.gov.au/def/voc/waterprogram/water-regulations-2008-water-information-terms/net-global-solar-exposure>
    a skos:Concept ;
    dcterms:contributor <https://linked.data.gov.au/org/neii> ;
    dcterms:created "2020-05-18"^^xsd:date ;
    dcterms:creator <https://linked.data.gov.au/org/neii> ;
    dcterms:modified "2020-05-18"^^xsd:date ;
    skos:definition """The global solar exposure less the reflected global solar exposure.
Source: Water Regulations 2008 (https://www.legislation.gov.au/Series/F2008L02170) Schedule 3 Part 1."""@en ;
    skos:notation "51" ;
    skos:prefLabel "net global solar exposure"@en ;
    skos:topConceptOf <http://www.neii.gov.au/def/voc/waterprogram/water-regulations-2008-water-information-terms/Water-Regulations-2008-water-information-terms> ;
.

<http://www.neii.gov.au/def/voc/waterprogram/water-regulations-2008-water-information-terms/net-global-solar-irradiance>
    a skos:Concept ;
    dcterms:contributor <https://linked.data.gov.au/org/neii> ;
    dcterms:created "2020-05-18"^^xsd:date ;
    dcterms:creator <https://linked.data.gov.au/org/neii> ;
    dcterms:modified "2020-05-18"^^xsd:date ;
    skos:definition """The global solar irradiance less the reflected global solar irradiance.
Source: Water Regulations 2008 (https://www.legislation.gov.au/Series/F2008L02170) Schedule 3 Part 1."""@en ;
    skos:notation "52" ;
    skos:prefLabel "net global solar irradiance"@en ;
    skos:topConceptOf <http://www.neii.gov.au/def/voc/waterprogram/water-regulations-2008-water-information-terms/Water-Regulations-2008-water-information-terms> ;
.

<http://www.neii.gov.au/def/voc/waterprogram/water-regulations-2008-water-information-terms/net-irradiance>
    a skos:Concept ;
    dcterms:contributor <https://linked.data.gov.au/org/neii> ;
    dcterms:created "2020-05-18"^^xsd:date ;
    dcterms:creator <https://linked.data.gov.au/org/neii> ;
    dcterms:modified "2020-05-18"^^xsd:date ;
    skos:definition """The net global solar irradiance plus the net longwave irradiance.
Source: Water Regulations 2008 (https://www.legislation.gov.au/Series/F2008L02170) Schedule 3 Part 1."""@en ;
    skos:notation "53" ;
    skos:prefLabel "net irradiance"@en ;
    skos:topConceptOf <http://www.neii.gov.au/def/voc/waterprogram/water-regulations-2008-water-information-terms/Water-Regulations-2008-water-information-terms> ;
.

<http://www.neii.gov.au/def/voc/waterprogram/water-regulations-2008-water-information-terms/net-longwave-exposure>
    a skos:Concept ;
    dcterms:contributor <https://linked.data.gov.au/org/neii> ;
    dcterms:created "2020-05-18"^^xsd:date ;
    dcterms:creator <https://linked.data.gov.au/org/neii> ;
    dcterms:modified "2020-05-18"^^xsd:date ;
    skos:definition """The downward longwave exposure less the upward longwave exposure.
Source: Water Regulations 2008 (https://www.legislation.gov.au/Series/F2008L02170) Schedule 3 Part 1."""@en ;
    skos:notation "54" ;
    skos:prefLabel "net longwave exposure"@en ;
    skos:topConceptOf <http://www.neii.gov.au/def/voc/waterprogram/water-regulations-2008-water-information-terms/Water-Regulations-2008-water-information-terms> ;
.

<http://www.neii.gov.au/def/voc/waterprogram/water-regulations-2008-water-information-terms/net-longwave-irradiance>
    a skos:Concept ;
    dcterms:contributor <https://linked.data.gov.au/org/neii> ;
    dcterms:created "2020-05-18"^^xsd:date ;
    dcterms:creator <https://linked.data.gov.au/org/neii> ;
    dcterms:modified "2020-05-18"^^xsd:date ;
    skos:definition """The downward longwave irradiance less the upward longwave exposure.
Source: Water Regulations 2008 (https://www.legislation.gov.au/Series/F2008L02170) Schedule 3 Part 1."""@en ;
    skos:notation "55" ;
    skos:prefLabel "net longwave irradiance"@en ;
    skos:topConceptOf <http://www.neii.gov.au/def/voc/waterprogram/water-regulations-2008-water-information-terms/Water-Regulations-2008-water-information-terms> ;
.

<http://www.neii.gov.au/def/voc/waterprogram/water-regulations-2008-water-information-terms/plant>
    a skos:Concept ;
    dcterms:contributor <https://linked.data.gov.au/org/neii> ;
    dcterms:created "2020-05-18"^^xsd:date ;
    dcterms:creator <https://linked.data.gov.au/org/neii> ;
    dcterms:modified "2020-05-18"^^xsd:date ;
    skos:definition """A treatment plant, relevant to the particular urban water system, of the reporting organisation.  It includes water treatment plants (WTP), wastewater treatment plants (WWTP) and water reclamation plants (WRP).
Source: Category 7 Reporting Handbook"""@en ;
    skos:notation "56" ;
    skos:prefLabel "plant"@en ;
    skos:topConceptOf <http://www.neii.gov.au/def/voc/waterprogram/water-regulations-2008-water-information-terms/Water-Regulations-2008-water-information-terms> ;
.

<http://www.neii.gov.au/def/voc/waterprogram/water-regulations-2008-water-information-terms/reflected-global-solar-exposure>
    a skos:Concept ;
    dcterms:contributor <https://linked.data.gov.au/org/neii> ;
    dcterms:created "2020-05-18"^^xsd:date ;
    dcterms:creator <https://linked.data.gov.au/org/neii> ;
    dcterms:modified "2020-05-18"^^xsd:date ;
    skos:definition """The total amount of electromagnetic energy emitted from the sun that is reflected from the ground and irradiates a specified unit horizontal surface from underneath.
Source: Water Regulations 2008 (https://www.legislation.gov.au/Series/F2008L02170) Schedule 3 Part 1."""@en ;
    skos:notation "57" ;
    skos:prefLabel "reflected global solar exposure"@en ;
    skos:topConceptOf <http://www.neii.gov.au/def/voc/waterprogram/water-regulations-2008-water-information-terms/Water-Regulations-2008-water-information-terms> ;
.

<http://www.neii.gov.au/def/voc/waterprogram/water-regulations-2008-water-information-terms/reflected-global-solar-irradiance>
    a skos:Concept ;
    dcterms:contributor <https://linked.data.gov.au/org/neii> ;
    dcterms:created "2020-05-18"^^xsd:date ;
    dcterms:creator <https://linked.data.gov.au/org/neii> ;
    dcterms:modified "2020-05-18"^^xsd:date ;
    skos:definition """The irradiance emitted from the sun that is reflected from the ground and irradiates a specified unit horizontal surface from underneath.
Source: Water Regulations 2008 (https://www.legislation.gov.au/Series/F2008L02170) Schedule 3 Part 1."""@en ;
    skos:notation "58" ;
    skos:prefLabel "reflected global solar irradiance"@en ;
    skos:topConceptOf <http://www.neii.gov.au/def/voc/waterprogram/water-regulations-2008-water-information-terms/Water-Regulations-2008-water-information-terms> ;
.

<http://www.neii.gov.au/def/voc/waterprogram/water-regulations-2008-water-information-terms/self-extract>
    a skos:Concept ;
    dcterms:contributor <https://linked.data.gov.au/org/neii> ;
    dcterms:created "2020-05-18"^^xsd:date ;
    dcterms:creator <https://linked.data.gov.au/org/neii> ;
    dcterms:modified "2020-05-18"^^xsd:date ;
    skos:definition """To take water directly from a water resource for the use of the person who takes water, but does not include taking water: (a) to provide it to another person, (b) under a stock and domestic right or (c) from an infrastructure operator.
Source: Water Regulations 2008 (https://www.legislation.gov.au/Series/F2008L02170) Schedule 3 Part 1."""@en ;
    skos:notation "59" ;
    skos:prefLabel "self extract"@en ;
    skos:topConceptOf <http://www.neii.gov.au/def/voc/waterprogram/water-regulations-2008-water-information-terms/Water-Regulations-2008-water-information-terms> ;
.

<http://www.neii.gov.au/def/voc/waterprogram/water-regulations-2008-water-information-terms/subcategory>
    a skos:Concept ;
    dcterms:contributor <https://linked.data.gov.au/org/neii> ;
    dcterms:created "2020-05-18"^^xsd:date ;
    dcterms:creator <https://linked.data.gov.au/org/neii> ;
    dcterms:modified "2020-05-18"^^xsd:date ;
    skos:definition "In relation to water information, means a subcategory of water information sepcified in regulation 7.03 and Schedule 3."@en ;
    skos:notation "62" ;
    skos:prefLabel "subcategory"@en ;
    skos:topConceptOf <http://www.neii.gov.au/def/voc/waterprogram/water-regulations-2008-water-information-terms/Water-Regulations-2008-water-information-terms> ;
.

<http://www.neii.gov.au/def/voc/waterprogram/water-regulations-2008-water-information-terms/surface-water>
    a skos:Concept ;
    dcterms:contributor <https://linked.data.gov.au/org/neii> ;
    dcterms:created "2020-05-18"^^xsd:date ;
    dcterms:creator <https://linked.data.gov.au/org/neii> ;
    dcterms:modified "2020-05-18"^^xsd:date ;
    skos:definition """Includes: (a) water in a watercourse, lake or wetland and (b) any water flowing over or lying on land: (i) after having precipitated naturally or (ii) after having risen to the surface naturally from underground.
Source: Water Act 2007 (https://www.legislation.gov.au/Details/C2018C00505) Part 1 Section 4, at 8 February 2019."""@en ;
    skos:notation "118" ;
    skos:prefLabel "surface water"@en ;
    skos:topConceptOf <http://www.neii.gov.au/def/voc/waterprogram/water-regulations-2008-water-information-terms/Water-Regulations-2008-water-information-terms> ;
.

<http://www.neii.gov.au/def/voc/waterprogram/water-regulations-2008-water-information-terms/take>
    a skos:Concept ;
    dcterms:contributor <https://linked.data.gov.au/org/neii> ;
    dcterms:created "2020-05-18"^^xsd:date ;
    dcterms:creator <https://linked.data.gov.au/org/neii> ;
    dcterms:modified "2020-05-18"^^xsd:date ;
    skos:definition """Take water from a water resource means to remove water from, or to reduce the flow of water in or into, the water resource including by any of the following means:
(a) pumping or siphoning water from the water resource;
(b) stopping, impeding or diverting the flow of water in or into the water resource;
(c) releasing water from the water resource if the water resource is a wetland or lake;
(d) permitting water to flow from the water resource if the water resource is a well or watercourse;
and includes storing water as part of, or in a way that is ancillary to, any of the processes or activities referred to in paragraphs (a) to (d).
Source: Water Act 2007 (https://www.legislation.gov.au/Details/C2018C00505) Part 1 Section 4, at 8 February 2019."""@en ;
    skos:notation "119" ;
    skos:prefLabel "take"@en ;
    skos:topConceptOf <http://www.neii.gov.au/def/voc/waterprogram/water-regulations-2008-water-information-terms/Water-Regulations-2008-water-information-terms> ;
.

<http://www.neii.gov.au/def/voc/waterprogram/water-regulations-2008-water-information-terms/tidal-limit>
    a skos:Concept ;
    dcterms:contributor <https://linked.data.gov.au/org/neii> ;
    dcterms:created "2020-05-18"^^xsd:date ;
    dcterms:creator <https://linked.data.gov.au/org/neii> ;
    dcterms:modified "2020-05-18"^^xsd:date ;
    skos:definition """In relation to a watercourse, the maximum upstream location on that watercourse at which a tidal variation in water-level is observed.
Source: Water Regulations 2008 (https://www.legislation.gov.au/Series/F2008L02170) Schedule 3 Part 1."""@en ;
    skos:notation "120" ;
    skos:prefLabel "tidal limit"@en ;
    skos:topConceptOf <http://www.neii.gov.au/def/voc/waterprogram/water-regulations-2008-water-information-terms/Water-Regulations-2008-water-information-terms> ;
.

<http://www.neii.gov.au/def/voc/waterprogram/water-regulations-2008-water-information-terms/total-nitrogen-concentration>
    a skos:Concept ;
    dcterms:contributor <https://linked.data.gov.au/org/neii> ;
    dcterms:created "2020-05-18"^^xsd:date ;
    dcterms:creator <https://linked.data.gov.au/org/neii> ;
    dcterms:modified "2020-05-19"^^xsd:date ;
    skos:definition """In relation to a water sample, the total concentration of all forms of nitrogen found in the water sample, including nitrate, nitrite, ammonia-N and organic forms of nitrogen.
Source: Water Regulations 2008 (https://www.legislation.gov.au/Series/F2008L02170) Schedule 3 Part 1."""@en ;
    skos:notation "121" ;
    skos:prefLabel "total nitrogen concentration"@en ;
    skos:topConceptOf <http://www.neii.gov.au/def/voc/waterprogram/water-regulations-2008-water-information-terms/Water-Regulations-2008-water-information-terms> ;
.

<http://www.neii.gov.au/def/voc/waterprogram/water-regulations-2008-water-information-terms/total-phosphorus-concentration>
    a skos:Concept ;
    dcterms:contributor <https://linked.data.gov.au/org/neii> ;
    dcterms:created "2020-05-18"^^xsd:date ;
    dcterms:creator <https://linked.data.gov.au/org/neii> ;
    dcterms:modified "2020-05-19"^^xsd:date ;
    skos:definition """In relation to a water sample, the total concentration of all forms of phosphorus found in the water sample.
Source: Water Regulations 2008 (https://www.legislation.gov.au/Series/F2008L02170) Schedule 3 Part 1."""@en ;
    skos:notation "122" ;
    skos:prefLabel "total phosphorus concentration"@en ;
    skos:topConceptOf <http://www.neii.gov.au/def/voc/waterprogram/water-regulations-2008-water-information-terms/Water-Regulations-2008-water-information-terms> ;
.

<http://www.neii.gov.au/def/voc/waterprogram/water-regulations-2008-water-information-terms/total-suspended-solids>
    a skos:Concept ;
    dcterms:contributor <https://linked.data.gov.au/org/neii> ;
    dcterms:created "2020-05-18"^^xsd:date ;
    dcterms:creator <https://linked.data.gov.au/org/neii> ;
    dcterms:modified "2020-05-19"^^xsd:date ;
    skos:definition """In relation to a water sample, the measure of the particles mixed in the water sample.
Source: Water Regulations 2008 (https://www.legislation.gov.au/Series/F2008L02170) Schedule 3 Part 1."""@en ;
    skos:notation "123" ;
    skos:prefLabel "total suspended solids"@en ;
    skos:topConceptOf <http://www.neii.gov.au/def/voc/waterprogram/water-regulations-2008-water-information-terms/Water-Regulations-2008-water-information-terms> ;
.

<http://www.neii.gov.au/def/voc/waterprogram/water-regulations-2008-water-information-terms/transfer-party>
    a skos:Concept ;
    dcterms:contributor <https://linked.data.gov.au/org/neii> ;
    dcterms:created "2020-05-18"^^xsd:date ;
    dcterms:creator <https://linked.data.gov.au/org/neii> ;
    dcterms:modified "2020-05-19"^^xsd:date ;
    skos:definition """Another service provider or other operational area within one's own operation.
Transfer party includes: (i) water utility; (ii) defined operational area of a utility; and (iii) private water manager.
Source: Category 7 Reporting Handbook"""@en ;
    skos:notation "124" ;
    skos:prefLabel "transfer party"@en ;
    skos:topConceptOf <http://www.neii.gov.au/def/voc/waterprogram/water-regulations-2008-water-information-terms/Water-Regulations-2008-water-information-terms> ;
.

<http://www.neii.gov.au/def/voc/waterprogram/water-regulations-2008-water-information-terms/turbidity>
    a skos:Concept ;
    dcterms:contributor <https://linked.data.gov.au/org/neii> ;
    dcterms:created "2020-05-18"^^xsd:date ;
    dcterms:creator <https://linked.data.gov.au/org/neii> ;
    dcterms:modified "2020-05-19"^^xsd:date ;
    skos:definition """Means the measure of the light scattering properties of water, and is an indicator of the presence of suspended solids.
Source: Water Regulations 2008 (https://www.legislation.gov.au/Series/F2008L02170) Schedule 3 Part 1."""@en ;
    skos:notation "125" ;
    skos:prefLabel "turbidity"@en ;
    skos:topConceptOf <http://www.neii.gov.au/def/voc/waterprogram/water-regulations-2008-water-information-terms/Water-Regulations-2008-water-information-terms> ;
.

<http://www.neii.gov.au/def/voc/waterprogram/water-regulations-2008-water-information-terms/upward-longwave-exposure>
    a skos:Concept ;
    dcterms:contributor <https://linked.data.gov.au/org/neii> ;
    dcterms:created "2020-05-18"^^xsd:date ;
    dcterms:creator <https://linked.data.gov.au/org/neii> ;
    dcterms:modified "2020-05-19"^^xsd:date ;
    skos:definition """The total amount of terrestrial electromagnetic energy emitted from the Earth's surface that irradiates a specified unit horizontal surface from underneath.
Source: Water Regulations 2008 (https://www.legislation.gov.au/Series/F2008L02170) Schedule 3 Part 1."""@en ;
    skos:notation "127" ;
    skos:prefLabel "upward longwave exposure"@en ;
    skos:topConceptOf <http://www.neii.gov.au/def/voc/waterprogram/water-regulations-2008-water-information-terms/Water-Regulations-2008-water-information-terms> ;
.

<http://www.neii.gov.au/def/voc/waterprogram/water-regulations-2008-water-information-terms/upward-longwave-irradiance>
    a skos:Concept ;
    dcterms:contributor <https://linked.data.gov.au/org/neii> ;
    dcterms:created "2020-05-18"^^xsd:date ;
    dcterms:creator <https://linked.data.gov.au/org/neii> ;
    dcterms:modified "2020-05-19"^^xsd:date ;
    skos:definition """The longwave irradiance emitted from the Earth's surface that irradiates a specified unit horizontal surface from underneath.
Source: Water Regulations 2008 (https://www.legislation.gov.au/Series/F2008L02170) Schedule 3 Part 1."""@en ;
    skos:notation "128" ;
    skos:prefLabel "upward longwave irradiance"@en ;
    skos:topConceptOf <http://www.neii.gov.au/def/voc/waterprogram/water-regulations-2008-water-information-terms/Water-Regulations-2008-water-information-terms> ;
.

<http://www.neii.gov.au/def/voc/waterprogram/water-regulations-2008-water-information-terms/urban-recycled-water-information>
    a skos:Concept ;
    dcterms:contributor <https://linked.data.gov.au/org/neii> ;
    dcterms:created "2020-05-18"^^xsd:date ;
    dcterms:creator <https://linked.data.gov.au/org/neii> ;
    dcterms:modified "2020-05-19"^^xsd:date ;
    skos:definition """Information about the treatment and reuse of urban wastewater.
Source: Water Regulations 2008 (https://www.legislation.gov.au/Series/F2008L02170) Schedule 3 Part 1."""@en ;
    skos:notation "129" ;
    skos:prefLabel "urban recycled water information"@en ;
    skos:topConceptOf <http://www.neii.gov.au/def/voc/waterprogram/water-regulations-2008-water-information-terms/Water-Regulations-2008-water-information-terms> ;
.

<http://www.neii.gov.au/def/voc/waterprogram/water-regulations-2008-water-information-terms/urban-stormwater-information>
    a skos:Concept ;
    dcterms:contributor <https://linked.data.gov.au/org/neii> ;
    dcterms:created "2020-05-18"^^xsd:date ;
    dcterms:creator <https://linked.data.gov.au/org/neii> ;
    dcterms:modified "2020-05-19"^^xsd:date ;
    skos:definition """Information about water in the urban water stormwater drainage system.
Source: Water Regulations 2008 (https://www.legislation.gov.au/Series/F2008L02170) Schedule 3 Part 1."""@en ;
    skos:notation "130" ;
    skos:prefLabel "urban stormwater information"@en ;
    skos:topConceptOf <http://www.neii.gov.au/def/voc/waterprogram/water-regulations-2008-water-information-terms/Water-Regulations-2008-water-information-terms> ;
.

<http://www.neii.gov.au/def/voc/waterprogram/water-regulations-2008-water-information-terms/urban-wastewater-information>
    a skos:Concept ;
    dcterms:contributor <https://linked.data.gov.au/org/neii> ;
    dcterms:created "2020-05-18"^^xsd:date ;
    dcterms:creator <https://linked.data.gov.au/org/neii> ;
    dcterms:modified "2020-05-19"^^xsd:date ;
    skos:definition """Information about wastewater that is disposed of through a sewerage system.
Source: Water Regulations 2008 (https://www.legislation.gov.au/Series/F2008L02170) Schedule 3 Part 1."""@en ;
    skos:notation "131" ;
    skos:prefLabel "urban wastewater information"@en ;
    skos:topConceptOf <http://www.neii.gov.au/def/voc/waterprogram/water-regulations-2008-water-information-terms/Water-Regulations-2008-water-information-terms> ;
.

<http://www.neii.gov.au/def/voc/waterprogram/water-regulations-2008-water-information-terms/urban-water-supply-information>
    a skos:Concept ;
    dcterms:contributor <https://linked.data.gov.au/org/neii> ;
    dcterms:created "2020-05-18"^^xsd:date ;
    dcterms:creator <https://linked.data.gov.au/org/neii> ;
    dcterms:modified "2020-05-19"^^xsd:date ;
    skos:definition """Information about water supplied by urban water utilities.
Source: Water Regulations 2008 (https://www.legislation.gov.au/Series/F2008L02170) Schedule 3 Part 1."""@en ;
    skos:notation "132" ;
    skos:prefLabel "urban water supply information"@en ;
    skos:topConceptOf <http://www.neii.gov.au/def/voc/waterprogram/water-regulations-2008-water-information-terms/Water-Regulations-2008-water-information-terms> ;
.

<http://www.neii.gov.au/def/voc/waterprogram/water-regulations-2008-water-information-terms/vapour-pressure-deficit>
    a skos:Concept ;
    dcterms:contributor <https://linked.data.gov.au/org/neii> ;
    dcterms:created "2020-05-18"^^xsd:date ;
    dcterms:creator <https://linked.data.gov.au/org/neii> ;
    dcterms:modified "2020-05-19"^^xsd:date ;
    skos:definition """The difference between the amount of moisture in the air and how much moisture the air can hold when it is saturated.
Source: Water Regulations 2008 (https://www.legislation.gov.au/Series/F2008L02170) Schedule 3 Part 1."""@en ;
    skos:notation "133" ;
    skos:prefLabel "vapour pressure deficit"@en ;
    skos:topConceptOf <http://www.neii.gov.au/def/voc/waterprogram/water-regulations-2008-water-information-terms/Water-Regulations-2008-water-information-terms> ;
.

<http://www.neii.gov.au/def/voc/waterprogram/water-regulations-2008-water-information-terms/wastewater-treatment-plant-WWTP>
    a skos:Concept ;
    dcterms:contributor <https://linked.data.gov.au/org/neii> ;
    dcterms:created "2020-05-18"^^xsd:date ;
    dcterms:creator <https://linked.data.gov.au/org/neii> ;
    dcterms:modified "2020-05-19"^^xsd:date ;
    skos:definition """The general name given to a plant used to treat wastewater collected through the urban wastewater system to meet quality requirements for effluent discharge to receiving waterways or land based re-use.
Source: Category 7 Reporting Handbook"""@en ;
    skos:notation "134" ;
    skos:prefLabel "wastewater treatment plant (WWTP)"@en ;
    skos:topConceptOf <http://www.neii.gov.au/def/voc/waterprogram/water-regulations-2008-water-information-terms/Water-Regulations-2008-water-information-terms> ;
.

<http://www.neii.gov.au/def/voc/waterprogram/water-regulations-2008-water-information-terms/water-connection>
    a skos:Concept ;
    dcterms:contributor <https://linked.data.gov.au/org/neii> ;
    dcterms:created "2020-05-18"^^xsd:date ;
    dcterms:creator <https://linked.data.gov.au/org/neii> ;
    dcterms:modified "2020-05-19"^^xsd:date ;
    skos:definition "A distribution point for a water service provided to an end user."@en ;
    skos:notation "135" ;
    skos:prefLabel "water connection"@en ;
    skos:topConceptOf <http://www.neii.gov.au/def/voc/waterprogram/water-regulations-2008-water-information-terms/Water-Regulations-2008-water-information-terms> ;
.

<http://www.neii.gov.au/def/voc/waterprogram/water-regulations-2008-water-information-terms/water-equivalent-precipitation>
    a skos:Concept ;
    dcterms:contributor <https://linked.data.gov.au/org/neii> ;
    dcterms:created "2020-05-18"^^xsd:date ;
    dcterms:creator <https://linked.data.gov.au/org/neii> ;
    dcterms:modified "2020-05-19"^^xsd:date ;
    skos:definition """The depth of water that would result if solid precipitation were melted.
Source: Water Regulations 2008 (https://www.legislation.gov.au/Series/F2008L02170) Schedule 3 Part 1."""@en ;
    skos:notation "137" ;
    skos:prefLabel "water-equivalent precipitation"@en ;
    skos:topConceptOf <http://www.neii.gov.au/def/voc/waterprogram/water-regulations-2008-water-information-terms/Water-Regulations-2008-water-information-terms> ;
.

<http://www.neii.gov.au/def/voc/waterprogram/water-regulations-2008-water-information-terms/water-information>
    a skos:Concept ;
    dcterms:contributor <https://linked.data.gov.au/org/neii> ;
    dcterms:created "2020-05-18"^^xsd:date ;
    dcterms:creator <https://linked.data.gov.au/org/neii> ;
    dcterms:modified "2020-05-19"^^xsd:date ;
    skos:definition """(a) any raw data, or any value added information product, that relates to:
(i) the availability, distribution, quantity, quality, use, trading or cost of water; or
(ii) water access rights, water delivery rights or irrigation rights; or
(b) any metadata relating to data of a kind referred to in paragraph (a);
and includes contextual information relating to water (such as land use information, geological information and ecological information).
Source: Water Act 2007 (https://www.legislation.gov.au/Details/C2018C00505) Part 7 Section 125, at 8 February 2019."""@en ;
    skos:notation "138" ;
    skos:prefLabel "water information"@en ;
    skos:topConceptOf <http://www.neii.gov.au/def/voc/waterprogram/water-regulations-2008-water-information-terms/Water-Regulations-2008-water-information-terms> ;
.

<http://www.neii.gov.au/def/voc/waterprogram/water-regulations-2008-water-information-terms/water-management-area>
    a skos:Concept ;
    dcterms:contributor <https://linked.data.gov.au/org/neii> ;
    dcterms:created "2020-05-18"^^xsd:date ;
    dcterms:creator <https://linked.data.gov.au/org/neii> ;
    dcterms:modified "2020-05-19"^^xsd:date ;
    skos:definition """An area (however described) used by an agency of the Commonwealth or an agency of a State for the purpose of managing surface water or ground water.
Note: The following are examples of water management areas:
(a) river basins;
(b) catchments;
(c) aquifers;
(d) water sources;
(e) sustainable diversion limit resource units.
Source: Water Regulations 2008 (https://www.legislation.gov.au/Series/F2008L02170) Schedule 3 Part 1."""@en ;
    skos:notation "139" ;
    skos:prefLabel "water management area"@en ;
    skos:topConceptOf <http://www.neii.gov.au/def/voc/waterprogram/water-regulations-2008-water-information-terms/Water-Regulations-2008-water-information-terms> ;
.

<http://www.neii.gov.au/def/voc/waterprogram/water-regulations-2008-water-information-terms/water-reclamation-plant-WRP>
    a skos:Concept ;
    dcterms:contributor <https://linked.data.gov.au/org/neii> ;
    dcterms:created "2020-05-18"^^xsd:date ;
    dcterms:creator <https://linked.data.gov.au/org/neii> ;
    dcterms:modified "2020-05-19"^^xsd:date ;
    skos:definition """The general name given to a plant used to treated wastewater treatment plant effluent for recycling.
Source: Category 7 Reporting Handbook"""@en ;
    skos:notation "140" ;
    skos:prefLabel "water reclamation plant (WRP)"@en ;
    skos:topConceptOf <http://www.neii.gov.au/def/voc/waterprogram/water-regulations-2008-water-information-terms/Water-Regulations-2008-water-information-terms> ;
.

<http://www.neii.gov.au/def/voc/waterprogram/water-regulations-2008-water-information-terms/water-storage>
    a skos:Concept ;
    dcterms:contributor <https://linked.data.gov.au/org/neii> ;
    dcterms:created "2020-05-18"^^xsd:date ;
    dcterms:creator <https://linked.data.gov.au/org/neii> ;
    dcterms:modified "2020-05-19"^^xsd:date ;
    skos:definition """A body of water that is naturally occurring, is impounded by a constructed barrier or is within an excavation, and includes ponds, swamps, lakes, wetlands, weirs, dams, basins, reservoirs and open pits.
Source: Water Regulations 2008 (https://www.legislation.gov.au/Series/F2008L02170) Schedule 3 Part 1."""@en ;
    skos:notation "141" ;
    skos:prefLabel "water storage"@en ;
    skos:topConceptOf <http://www.neii.gov.au/def/voc/waterprogram/water-regulations-2008-water-information-terms/Water-Regulations-2008-water-information-terms> ;
.

<http://www.neii.gov.au/def/voc/waterprogram/water-regulations-2008-water-information-terms/water-treatment-plant-WTP>
    a skos:Concept ;
    dcterms:contributor <https://linked.data.gov.au/org/neii> ;
    dcterms:created "2020-05-18"^^xsd:date ;
    dcterms:creator <https://linked.data.gov.au/org/neii> ;
    dcterms:modified "2020-05-19"^^xsd:date ;
    skos:definition """The general name given to a plant typically used to treat water sourced from surface or groundwater for supply into the urban water system.
Source: Category 7 Reporting Handbook"""@en ;
    skos:notation "142" ;
    skos:prefLabel "water treatment plant (WTP)"@en ;
    skos:topConceptOf <http://www.neii.gov.au/def/voc/waterprogram/water-regulations-2008-water-information-terms/Water-Regulations-2008-water-information-terms> ;
.

<http://www.neii.gov.au/def/voc/waterprogram/water-regulations-2008-water-information-terms/watercourse>
    a skos:Concept ;
    dcterms:contributor <https://linked.data.gov.au/org/neii> ;
    dcterms:created "2020-05-18"^^xsd:date ;
    dcterms:creator <https://linked.data.gov.au/org/neii> ;
    dcterms:modified "2020-05-19"^^xsd:date ;
    skos:definition """A river, creek or other natural watercourse (whether modified or not) in which water is contained or flows (whether permanently or from time to time); and includes:
(i) a dam or reservoir that collects water flowing in a watercourse;
(ii) a lake or wetland through which water flows;
(iii) a channel into which the water of a watercourse has been diverted;
(iv) part of a watercourse; and
(v) an estuary through which water flows
Source: Based on content from the Federal Register of Legislation (https://www.legislation.gov.au/Details/C2018C00505), at 8 February 2019."""@en ;
    skos:notation "136" ;
    skos:prefLabel "watercourse"@en ;
    skos:topConceptOf <http://www.neii.gov.au/def/voc/waterprogram/water-regulations-2008-water-information-terms/Water-Regulations-2008-water-information-terms> ;
.

<http://www.neii.gov.au/def/voc/waterprogram/water-regulations-2008-water-information-terms/web-service>
    a skos:Concept ;
    dcterms:contributor <https://linked.data.gov.au/org/neii> ;
    dcterms:created "2020-05-18"^^xsd:date ;
    dcterms:creator <https://linked.data.gov.au/org/neii> ;
    dcterms:modified "2020-05-19"^^xsd:date ;
    skos:definition """A software system designed to support machine-to-machine interaction, in which the machines are capable of being used or operated reciprocally over a network of computers.
Source: Water Regulations 2008 (https://www.legislation.gov.au/Series/F2008L02170) Regulation 1.03."""@en ;
    skos:notation "143" ;
    skos:prefLabel "web service"@en ;
    skos:topConceptOf <http://www.neii.gov.au/def/voc/waterprogram/water-regulations-2008-water-information-terms/Water-Regulations-2008-water-information-terms> ;
.

<http://www.neii.gov.au/def/voc/waterprogram/water-regulations-2008-water-information-terms/week>
    a skos:Concept ;
    dcterms:contributor <https://linked.data.gov.au/org/neii> ;
    dcterms:created "2020-05-18"^^xsd:date ;
    dcterms:creator <https://linked.data.gov.au/org/neii> ;
    dcterms:modified "2020-05-19"^^xsd:date ;
    skos:definition """A period of seven consecutive days starting on the first moment of a Monday and finishing at the end of the following Sunday.
Source: Water Regulations 2008 (https://www.legislation.gov.au/Series/F2008L02170) Regulation 1.04."""@en ;
    skos:notation "144" ;
    skos:prefLabel "week"@en ;
    skos:topConceptOf <http://www.neii.gov.au/def/voc/waterprogram/water-regulations-2008-water-information-terms/Water-Regulations-2008-water-information-terms> ;
.

<http://www.neii.gov.au/def/voc/waterprogram/water-regulations-2008-water-information-terms/wet-bulb-air-temperature>
    a skos:Concept ;
    dcterms:contributor <https://linked.data.gov.au/org/neii> ;
    dcterms:created "2020-05-18"^^xsd:date ;
    dcterms:creator <https://linked.data.gov.au/org/neii> ;
    dcterms:modified "2020-05-19"^^xsd:date ;
    skos:definition """The temperature of air measured by a thermometer that has its bulb wrapped in wet muslin.
Source: Water Regulations 2008 (https://www.legislation.gov.au/Series/F2008L02170) Schedule 3 Part 1."""@en ;
    skos:notation "145" ;
    skos:prefLabel "wet bulb air temperature"@en ;
    skos:topConceptOf <http://www.neii.gov.au/def/voc/waterprogram/water-regulations-2008-water-information-terms/Water-Regulations-2008-water-information-terms> ;
.

<http://www.neii.gov.au/def/voc/waterprogram/water-regulations-2008-water-information-terms/wind-run>
    a skos:Concept ;
    dcterms:contributor <https://linked.data.gov.au/org/neii> ;
    dcterms:created "2020-05-18"^^xsd:date ;
    dcterms:creator <https://linked.data.gov.au/org/neii> ;
    dcterms:modified "2020-05-19"^^xsd:date ;
    skos:definition """The product of the average wind speed and the period over which that average speed was measured.
Source: Water Regulations 2008 (https://www.legislation.gov.au/Series/F2008L02170) Schedule 3 Part 1."""@en ;
    skos:notation "147" ;
    skos:prefLabel "wind run"@en ;
    skos:topConceptOf <http://www.neii.gov.au/def/voc/waterprogram/water-regulations-2008-water-information-terms/Water-Regulations-2008-water-information-terms> ;
.

<http://www.neii.gov.au/def/voc/waterprogram/water-regulations-2008-water-information-terms/year>
    a skos:Concept ;
    dcterms:contributor <https://linked.data.gov.au/org/neii> ;
    dcterms:created "2020-05-18"^^xsd:date ;
    dcterms:creator <https://linked.data.gov.au/org/neii> ;
    dcterms:modified "2020-05-19"^^xsd:date ;
    skos:definition """The financial year.
Source: Water Regulations 2008 (https://www.legislation.gov.au/Series/F2008L02170) Regulation 1.04."""@en ;
    skos:notation "148" ;
    skos:prefLabel "year"@en ;
    skos:topConceptOf <http://www.neii.gov.au/def/voc/waterprogram/water-regulations-2008-water-information-terms/Water-Regulations-2008-water-information-terms> ;
.

skos:related
    a
        rdf:Property ,
        rdfs:Resource ;
    rdfs:subPropertyOf skos:related ;
.

<http://www.neii.gov.au/def/voc/waterprogram/water-regulations-2008-water-information-terms/Category-8-water-information>
    a skos:Concept ;
    dcterms:contributor <https://linked.data.gov.au/org/neii> ;
    dcterms:created "2020-05-18"^^xsd:date ;
    dcterms:creator <https://linked.data.gov.au/org/neii> ;
    dcterms:modified "2020-05-18"^^xsd:date ;
    skos:definition """Information about water restrictions
Source: Water Regulations 2008 (https://www.legislation.gov.au/Series/F2008L02170) Schedule 3 Part 9."""@en ;
    skos:notation "15" ;
    skos:prefLabel "Category 8 water information"@en ;
    skos:related <http://www.neii.gov.au/def/voc/waterprogram/water-regulations-2008-water-information-terms/subcategory-8a-water-information> ;
    skos:topConceptOf <http://www.neii.gov.au/def/voc/waterprogram/water-regulations-2008-water-information-terms/Water-Regulations-2008-water-information-terms> ;
.

<http://www.neii.gov.au/def/voc/waterprogram/water-regulations-2008-water-information-terms/subcategory-11a-water-information>
    a skos:Concept ;
    dcterms:contributor <https://linked.data.gov.au/org/neii> ;
    dcterms:created "2020-05-18"^^xsd:date ;
    dcterms:creator <https://linked.data.gov.au/org/neii> ;
    dcterms:modified "2020-05-18"^^xsd:date ;
    skos:definition """Level of a watercourse, expressed in metres.
Source: Water Regulations 2008 (https://www.legislation.gov.au/Series/F2008L02170) Schedule 3 Part 11."""@en ;
    skos:notation "115" ;
    skos:prefLabel "subcategory 11a water information"@en ;
    skos:related <http://www.neii.gov.au/def/voc/waterprogram/water-regulations-2008-water-information-terms/Category-11-water-information> ;
    skos:topConceptOf <http://www.neii.gov.au/def/voc/waterprogram/water-regulations-2008-water-information-terms/Water-Regulations-2008-water-information-terms> ;
.

<http://www.neii.gov.au/def/voc/waterprogram/water-regulations-2008-water-information-terms/subcategory-11b-water-information>
    a skos:Concept ;
    dcterms:contributor <https://linked.data.gov.au/org/neii> ;
    dcterms:created "2020-05-18"^^xsd:date ;
    dcterms:creator <https://linked.data.gov.au/org/neii> ;
    dcterms:modified "2020-05-18"^^xsd:date ;
    skos:definition """Discharge of a watercourse, expressed in cumecs.
Source: Water Regulations 2008 (https://www.legislation.gov.au/Series/F2008L02170) Schedule 3 Part 11."""@en ;
    skos:notation "116" ;
    skos:prefLabel "subcategory 11b water information"@en ;
    skos:related <http://www.neii.gov.au/def/voc/waterprogram/water-regulations-2008-water-information-terms/Category-11-water-information> ;
    skos:topConceptOf <http://www.neii.gov.au/def/voc/waterprogram/water-regulations-2008-water-information-terms/Water-Regulations-2008-water-information-terms> ;
.

<http://www.neii.gov.au/def/voc/waterprogram/water-regulations-2008-water-information-terms/subcategory-11c-water-information>
    a skos:Concept ;
    dcterms:contributor <https://linked.data.gov.au/org/neii> ;
    dcterms:created "2020-05-18"^^xsd:date ;
    dcterms:creator <https://linked.data.gov.au/org/neii> ;
    dcterms:modified "2020-05-18"^^xsd:date ;
    skos:definition """Accumulated precipitation depth, including water-equivalent precipitation depth, expressed in millimetres.
Source: Water Regulations 2008 (https://www.legislation.gov.au/Series/F2008L02170) Schedule 3 Part 11."""@en ;
    skos:notation "117" ;
    skos:prefLabel "subcategory 11c water information"@en ;
    skos:related <http://www.neii.gov.au/def/voc/waterprogram/water-regulations-2008-water-information-terms/Category-11-water-information> ;
    skos:topConceptOf <http://www.neii.gov.au/def/voc/waterprogram/water-regulations-2008-water-information-terms/Water-Regulations-2008-water-information-terms> ;
.

<http://www.neii.gov.au/def/voc/waterprogram/water-regulations-2008-water-information-terms/subcategory-1a-water-information>
    a skos:Concept ;
    dcterms:contributor <https://linked.data.gov.au/org/neii> ;
    dcterms:created "2020-05-18"^^xsd:date ;
    dcterms:creator <https://linked.data.gov.au/org/neii> ;
    dcterms:modified "2020-05-18"^^xsd:date ;
    skos:definition """Level of a watercourse (other than a water storage), expressed in metres.
Source: Water Regulations 2008 (https://www.legislation.gov.au/Series/F2008L02170) Schedule 3 Part 2."""@en ;
    skos:notation "63" ;
    skos:prefLabel "subcategory 1a water information"@en ;
    skos:related <http://www.neii.gov.au/def/voc/waterprogram/water-regulations-2008-water-information-terms/Category-1-water-information> ;
    skos:topConceptOf <http://www.neii.gov.au/def/voc/waterprogram/water-regulations-2008-water-information-terms/Water-Regulations-2008-water-information-terms> ;
.

<http://www.neii.gov.au/def/voc/waterprogram/water-regulations-2008-water-information-terms/subcategory-1b-water-information>
    a skos:Concept ;
    dcterms:contributor <https://linked.data.gov.au/org/neii> ;
    dcterms:created "2020-05-18"^^xsd:date ;
    dcterms:creator <https://linked.data.gov.au/org/neii> ;
    dcterms:modified "2020-05-18"^^xsd:date ;
    skos:definition """Discharge of a watercourse (other than a water storage), expressed in cumecs.
Source: Water Regulations 2008 (https://www.legislation.gov.au/Series/F2008L02170) Schedule 3 Part 2."""@en ;
    skos:notation "64" ;
    skos:prefLabel "subcategory 1b water information"@en ;
    skos:related <http://www.neii.gov.au/def/voc/waterprogram/water-regulations-2008-water-information-terms/Category-1-water-information> ;
    skos:topConceptOf <http://www.neii.gov.au/def/voc/waterprogram/water-regulations-2008-water-information-terms/Water-Regulations-2008-water-information-terms> ;
.

<http://www.neii.gov.au/def/voc/waterprogram/water-regulations-2008-water-information-terms/subcategory-2a-water-information>
    a skos:Concept ;
    dcterms:contributor <https://linked.data.gov.au/org/neii> ;
    dcterms:created "2020-05-18"^^xsd:date ;
    dcterms:creator <https://linked.data.gov.au/org/neii> ;
    dcterms:modified "2020-05-18"^^xsd:date ;
    skos:definition """Ground water level, expressed in metres.
Source: Water Regulations 2008 (https://www.legislation.gov.au/Series/F2008L02170) Schedule 3 Part 3."""@en ;
    skos:notation "65" ;
    skos:prefLabel "subcategory 2a water information"@en ;
    skos:related <http://www.neii.gov.au/def/voc/waterprogram/water-regulations-2008-water-information-terms/Category-2-water-information> ;
    skos:topConceptOf <http://www.neii.gov.au/def/voc/waterprogram/water-regulations-2008-water-information-terms/Water-Regulations-2008-water-information-terms> ;
.

<http://www.neii.gov.au/def/voc/waterprogram/water-regulations-2008-water-information-terms/subcategory-2b-water-information>
    a skos:Concept ;
    dcterms:contributor <https://linked.data.gov.au/org/neii> ;
    dcterms:created "2020-05-18"^^xsd:date ;
    dcterms:creator <https://linked.data.gov.au/org/neii> ;
    dcterms:modified "2020-05-18"^^xsd:date ;
    skos:definition """Ground water pressure, expressed in kilopascals.
Source: Water Regulations 2008 (https://www.legislation.gov.au/Series/F2008L02170) Schedule 3 Part 3."""@en ;
    skos:notation "66" ;
    skos:prefLabel "subcategory 2b water information"@en ;
    skos:related <http://www.neii.gov.au/def/voc/waterprogram/water-regulations-2008-water-information-terms/Category-2-water-information> ;
    skos:topConceptOf <http://www.neii.gov.au/def/voc/waterprogram/water-regulations-2008-water-information-terms/Water-Regulations-2008-water-information-terms> ;
.

<http://www.neii.gov.au/def/voc/waterprogram/water-regulations-2008-water-information-terms/subcategory-2d-water-information>
    a skos:Concept ;
    dcterms:contributor <https://linked.data.gov.au/org/neii> ;
    dcterms:created "2020-05-18"^^xsd:date ;
    dcterms:creator <https://linked.data.gov.au/org/neii> ;
    dcterms:modified "2020-05-18"^^xsd:date ;
    skos:definition """State aquifer framework information
Source: Water Regulations 2008 (https://www.legislation.gov.au/Series/F2008L02170) Schedule 3 Part 3."""@en ;
    skos:notation "67" ;
    skos:prefLabel "subcategory 2d water information"@en ;
    skos:related <http://www.neii.gov.au/def/voc/waterprogram/water-regulations-2008-water-information-terms/Category-2-water-information> ;
    skos:topConceptOf <http://www.neii.gov.au/def/voc/waterprogram/water-regulations-2008-water-information-terms/Water-Regulations-2008-water-information-terms> ;
.

<http://www.neii.gov.au/def/voc/waterprogram/water-regulations-2008-water-information-terms/subcategory-2e-water-information>
    a skos:Concept ;
    dcterms:contributor <https://linked.data.gov.au/org/neii> ;
    dcterms:created "2020-05-18"^^xsd:date ;
    dcterms:creator <https://linked.data.gov.au/org/neii> ;
    dcterms:modified "2020-05-18"^^xsd:date ;
    skos:definition """State NGIS information
Source: Water Regulations 2008 (https://www.legislation.gov.au/Series/F2008L02170) Schedule 3 Part 3."""@en ;
    skos:notation "68" ;
    skos:prefLabel "subcategory 2e water information"@en ;
    skos:related <http://www.neii.gov.au/def/voc/waterprogram/water-regulations-2008-water-information-terms/Category-2-water-information> ;
    skos:topConceptOf <http://www.neii.gov.au/def/voc/waterprogram/water-regulations-2008-water-information-terms/Water-Regulations-2008-water-information-terms> ;
.

<http://www.neii.gov.au/def/voc/waterprogram/water-regulations-2008-water-information-terms/subcategory-3a-water-information>
    a skos:Concept ;
    dcterms:contributor <https://linked.data.gov.au/org/neii> ;
    dcterms:created "2020-05-18"^^xsd:date ;
    dcterms:creator <https://linked.data.gov.au/org/neii> ;
    dcterms:modified "2020-05-18"^^xsd:date ;
    skos:definition """Level of water in a major storage, expressed in metres.
Source: Water Regulations 2008 (https://www.legislation.gov.au/Series/F2008L02170) Schedule 3 Part 4."""@en ;
    skos:notation "69" ;
    skos:prefLabel "subcategory 3a water information"@en ;
    skos:related <http://www.neii.gov.au/def/voc/waterprogram/water-regulations-2008-water-information-terms/Category-3-water-information> ;
    skos:topConceptOf <http://www.neii.gov.au/def/voc/waterprogram/water-regulations-2008-water-information-terms/Water-Regulations-2008-water-information-terms> ;
.

<http://www.neii.gov.au/def/voc/waterprogram/water-regulations-2008-water-information-terms/subcategory-3b-water-information>
    a skos:Concept ;
    dcterms:contributor <https://linked.data.gov.au/org/neii> ;
    dcterms:created "2020-05-18"^^xsd:date ;
    dcterms:creator <https://linked.data.gov.au/org/neii> ;
    dcterms:modified "2020-05-18"^^xsd:date ;
    skos:definition """Volume of water in a major storage, expressed in megalitres.
Source: Water Regulations 2008 (https://www.legislation.gov.au/Series/F2008L02170) Schedule 3 Part 4."""@en ;
    skos:notation "70" ;
    skos:prefLabel "subcategory 3b water information"@en ;
    skos:related <http://www.neii.gov.au/def/voc/waterprogram/water-regulations-2008-water-information-terms/Category-3-water-information> ;
    skos:topConceptOf <http://www.neii.gov.au/def/voc/waterprogram/water-regulations-2008-water-information-terms/Water-Regulations-2008-water-information-terms> ;
.

<http://www.neii.gov.au/def/voc/waterprogram/water-regulations-2008-water-information-terms/subcategory-3c-water-information>
    a skos:Concept ;
    dcterms:contributor <https://linked.data.gov.au/org/neii> ;
    dcterms:created "2020-05-18"^^xsd:date ;
    dcterms:creator <https://linked.data.gov.au/org/neii> ;
    dcterms:modified "2020-05-18"^^xsd:date ;
    skos:definition """Volume of water released from a major storage, expressed in megalitres.
Source: Water Regulations 2008 (https://www.legislation.gov.au/Series/F2008L02170) Schedule 3 Part 4."""@en ;
    skos:notation "71" ;
    skos:prefLabel "subcategory 3c water information"@en ;
    skos:related <http://www.neii.gov.au/def/voc/waterprogram/water-regulations-2008-water-information-terms/Category-3-water-information> ;
    skos:topConceptOf <http://www.neii.gov.au/def/voc/waterprogram/water-regulations-2008-water-information-terms/Water-Regulations-2008-water-information-terms> ;
.

<http://www.neii.gov.au/def/voc/waterprogram/water-regulations-2008-water-information-terms/subcategory-3d-water-information>
    a skos:Concept ;
    dcterms:contributor <https://linked.data.gov.au/org/neii> ;
    dcterms:created "2020-05-18"^^xsd:date ;
    dcterms:creator <https://linked.data.gov.au/org/neii> ;
    dcterms:modified "2020-05-19"^^xsd:date ;
    skos:definition """Total volume of water delivered to a major storage, expressed in megalitres.
Source: Water Regulations 2008 (https://www.legislation.gov.au/Series/F2008L02170) Schedule 3 Part 4."""@en ;
    skos:notation "72" ;
    skos:prefLabel "subcategory 3d water information"@en ;
    skos:related <http://www.neii.gov.au/def/voc/waterprogram/water-regulations-2008-water-information-terms/Category-3-water-information> ;
    skos:topConceptOf <http://www.neii.gov.au/def/voc/waterprogram/water-regulations-2008-water-information-terms/Water-Regulations-2008-water-information-terms> ;
.

<http://www.neii.gov.au/def/voc/waterprogram/water-regulations-2008-water-information-terms/subcategory-3da-water-information>
    a skos:Concept ;
    dcterms:contributor <https://linked.data.gov.au/org/neii> ;
    dcterms:created "2020-05-18"^^xsd:date ;
    dcterms:creator <https://linked.data.gov.au/org/neii> ;
    dcterms:modified "2020-05-19"^^xsd:date ;
    skos:definition """Volume of water delivered to a major storage from each water source, expressed in megalitres.
Source: Water Regulations 2008 (https://www.legislation.gov.au/Series/F2008L02170) Schedule 3 Part 4."""@en ;
    skos:notation "73" ;
    skos:prefLabel "subcategory 3da water information"@en ;
    skos:related <http://www.neii.gov.au/def/voc/waterprogram/water-regulations-2008-water-information-terms/Category-3-water-information> ;
    skos:topConceptOf <http://www.neii.gov.au/def/voc/waterprogram/water-regulations-2008-water-information-terms/Water-Regulations-2008-water-information-terms> ;
.

<http://www.neii.gov.au/def/voc/waterprogram/water-regulations-2008-water-information-terms/subcategory-3e-water-information>
    a skos:Concept ;
    dcterms:contributor <https://linked.data.gov.au/org/neii> ;
    dcterms:created "2020-05-18"^^xsd:date ;
    dcterms:creator <https://linked.data.gov.au/org/neii> ;
    dcterms:modified "2020-05-18"^^xsd:date ;
    skos:definition """Volume of water in a minor storage, expressed in megalitres.
Source: Water Regulations 2008 (https://www.legislation.gov.au/Series/F2008L02170) Schedule 3 Part 4."""@en ;
    skos:notation "74" ;
    skos:prefLabel "subcategory 3e water information"@en ;
    skos:related <http://www.neii.gov.au/def/voc/waterprogram/water-regulations-2008-water-information-terms/Category-3-water-information> ;
    skos:topConceptOf <http://www.neii.gov.au/def/voc/waterprogram/water-regulations-2008-water-information-terms/Water-Regulations-2008-water-information-terms> ;
.

<http://www.neii.gov.au/def/voc/waterprogram/water-regulations-2008-water-information-terms/subcategory-3f-water-information>
    a skos:Concept ;
    dcterms:contributor <https://linked.data.gov.au/org/neii> ;
    dcterms:created "2020-05-18"^^xsd:date ;
    dcterms:creator <https://linked.data.gov.au/org/neii> ;
    dcterms:modified "2020-05-18"^^xsd:date ;
    skos:definition """A list of major storages owned, operated or regulated by the person required to give the information.
Source: Water Regulations 2008 (https://www.legislation.gov.au/Series/F2008L02170) Schedule 3 Part 4."""@en ;
    skos:notation "75" ;
    skos:prefLabel "subcategory 3f water information"@en ;
    skos:related <http://www.neii.gov.au/def/voc/waterprogram/water-regulations-2008-water-information-terms/Category-3-water-information> ;
    skos:topConceptOf <http://www.neii.gov.au/def/voc/waterprogram/water-regulations-2008-water-information-terms/Water-Regulations-2008-water-information-terms> ;
.

<http://www.neii.gov.au/def/voc/waterprogram/water-regulations-2008-water-information-terms/subcategory-4a-water-information>
    a skos:Concept ;
    dcterms:contributor <https://linked.data.gov.au/org/neii> ;
    dcterms:created "2020-05-18"^^xsd:date ;
    dcterms:creator <https://linked.data.gov.au/org/neii> ;
    dcterms:modified "2020-05-18"^^xsd:date ;
    skos:definition """Accumulated precipitation depth, including the water-equivalent precipitation depth, expressed in millimetres.
Source: Water Regulations 2008 (https://www.legislation.gov.au/Series/F2008L02170) Schedule 3 Part 5."""@en ;
    skos:notation "76" ;
    skos:prefLabel "subcategory 4a water information"@en ;
    skos:related <http://www.neii.gov.au/def/voc/waterprogram/water-regulations-2008-water-information-terms/Category-4-water-information> ;
    skos:topConceptOf <http://www.neii.gov.au/def/voc/waterprogram/water-regulations-2008-water-information-terms/Water-Regulations-2008-water-information-terms> ;
.

<http://www.neii.gov.au/def/voc/waterprogram/water-regulations-2008-water-information-terms/subcategory-4b-water-information>
    a skos:Concept ;
    dcterms:contributor <https://linked.data.gov.au/org/neii> ;
    dcterms:created "2020-05-18"^^xsd:date ;
    dcterms:creator <https://linked.data.gov.au/org/neii> ;
    dcterms:modified "2020-05-18"^^xsd:date ;
    skos:definition """Wind speed (expressed in metres per second), wind direction and wind run (expressed in kilometres over a specified period).
Source: Water Regulations 2008 (https://www.legislation.gov.au/Series/F2008L02170) Schedule 3 Part 5."""@en ;
    skos:notation "77" ;
    skos:prefLabel "subcategory 4b water information"@en ;
    skos:related <http://www.neii.gov.au/def/voc/waterprogram/water-regulations-2008-water-information-terms/Category-4-water-information> ;
    skos:topConceptOf <http://www.neii.gov.au/def/voc/waterprogram/water-regulations-2008-water-information-terms/Water-Regulations-2008-water-information-terms> ;
.

<http://www.neii.gov.au/def/voc/waterprogram/water-regulations-2008-water-information-terms/subcategory-4c-water-information>
    a skos:Concept ;
    dcterms:contributor <https://linked.data.gov.au/org/neii> ;
    dcterms:created "2020-05-18"^^xsd:date ;
    dcterms:creator <https://linked.data.gov.au/org/neii> ;
    dcterms:modified "2020-05-18"^^xsd:date ;
    skos:definition """Evaporation, expressed in millimetres per day.
Source: Water Regulations 2008 (https://www.legislation.gov.au/Series/F2008L02170) Schedule 3 Part 5."""@en ;
    skos:notation "78" ;
    skos:prefLabel "subcategory 4c water information"@en ;
    skos:related <http://www.neii.gov.au/def/voc/waterprogram/water-regulations-2008-water-information-terms/Category-4-water-information> ;
    skos:topConceptOf <http://www.neii.gov.au/def/voc/waterprogram/water-regulations-2008-water-information-terms/Water-Regulations-2008-water-information-terms> ;
.

<http://www.neii.gov.au/def/voc/waterprogram/water-regulations-2008-water-information-terms/subcategory-4d-water-information>
    a skos:Concept ;
    dcterms:contributor <https://linked.data.gov.au/org/neii> ;
    dcterms:created "2020-05-18"^^xsd:date ;
    dcterms:creator <https://linked.data.gov.au/org/neii> ;
    dcterms:modified "2020-05-18"^^xsd:date ;
    skos:definition """Global solar exposure, reflected global solar exposure, downward longwave exposure, upward longwave exposure and net exposure, each expressed in joules per square metre.
Source: Water Regulations 2008 (https://www.legislation.gov.au/Series/F2008L02170) Schedule 3 Part 5."""@en ;
    skos:notation "79" ;
    skos:prefLabel "subcategory 4d water information"@en ;
    skos:related <http://www.neii.gov.au/def/voc/waterprogram/water-regulations-2008-water-information-terms/Category-4-water-information> ;
    skos:topConceptOf <http://www.neii.gov.au/def/voc/waterprogram/water-regulations-2008-water-information-terms/Water-Regulations-2008-water-information-terms> ;
.

<http://www.neii.gov.au/def/voc/waterprogram/water-regulations-2008-water-information-terms/subcategory-4e-water-information>
    a skos:Concept ;
    dcterms:contributor <https://linked.data.gov.au/org/neii> ;
    dcterms:created "2020-05-18"^^xsd:date ;
    dcterms:creator <https://linked.data.gov.au/org/neii> ;
    dcterms:modified "2020-05-18"^^xsd:date ;
    skos:definition """Global solar irradiance, reflected global solar irradiance, downward longwave irradiance, upward longwave irradiance and net irradiance, each expressed in watts per square metre.
Source: Water Regulations 2008 (https://www.legislation.gov.au/Series/F2008L02170) Schedule 3 Part 5."""@en ;
    skos:notation "80" ;
    skos:prefLabel "subcategory 4e water information"@en ;
    skos:related <http://www.neii.gov.au/def/voc/waterprogram/water-regulations-2008-water-information-terms/Category-4-water-information> ;
    skos:topConceptOf <http://www.neii.gov.au/def/voc/waterprogram/water-regulations-2008-water-information-terms/Water-Regulations-2008-water-information-terms> ;
.

<http://www.neii.gov.au/def/voc/waterprogram/water-regulations-2008-water-information-terms/subcategory-4f-water-information>
    a skos:Concept ;
    dcterms:contributor <https://linked.data.gov.au/org/neii> ;
    dcterms:created "2020-05-18"^^xsd:date ;
    dcterms:creator <https://linked.data.gov.au/org/neii> ;
    dcterms:modified "2020-05-18"^^xsd:date ;
    skos:definition """Dry-bulb air temperature, expressed in degrees Celsius.
Source: Water Regulations 2008 (https://www.legislation.gov.au/Series/F2008L02170) Schedule 3 Part 5."""@en ;
    skos:notation "81" ;
    skos:prefLabel "subcategory 4f water information"@en ;
    skos:related <http://www.neii.gov.au/def/voc/waterprogram/water-regulations-2008-water-information-terms/Category-4-water-information> ;
    skos:topConceptOf <http://www.neii.gov.au/def/voc/waterprogram/water-regulations-2008-water-information-terms/Water-Regulations-2008-water-information-terms> ;
.

<http://www.neii.gov.au/def/voc/waterprogram/water-regulations-2008-water-information-terms/subcategory-4g-water-information>
    a skos:Concept ;
    dcterms:contributor <https://linked.data.gov.au/org/neii> ;
    dcterms:created "2020-05-18"^^xsd:date ;
    dcterms:creator <https://linked.data.gov.au/org/neii> ;
    dcterms:modified "2020-05-18"^^xsd:date ;
    skos:definition """Wet-bulb air temperature, expressed in degrees Celsius.
Source: Water Regulations 2008 (https://www.legislation.gov.au/Series/F2008L02170) Schedule 3 Part 5."""@en ;
    skos:notation "82" ;
    skos:prefLabel "subcategory 4g water information"@en ;
    skos:related <http://www.neii.gov.au/def/voc/waterprogram/water-regulations-2008-water-information-terms/Category-4-water-information> ;
    skos:topConceptOf <http://www.neii.gov.au/def/voc/waterprogram/water-regulations-2008-water-information-terms/Water-Regulations-2008-water-information-terms> ;
.

<http://www.neii.gov.au/def/voc/waterprogram/water-regulations-2008-water-information-terms/subcategory-4h-water-information>
    a skos:Concept ;
    dcterms:contributor <https://linked.data.gov.au/org/neii> ;
    dcterms:created "2020-05-18"^^xsd:date ;
    dcterms:creator <https://linked.data.gov.au/org/neii> ;
    dcterms:modified "2020-05-18"^^xsd:date ;
    skos:definition """Relative humidity, expressed as a percentage.
Source: Water Regulations 2008 (https://www.legislation.gov.au/Series/F2008L02170) Schedule 3 Part 5."""@en ;
    skos:notation "83" ;
    skos:prefLabel "subcategory 4h water information"@en ;
    skos:related <http://www.neii.gov.au/def/voc/waterprogram/water-regulations-2008-water-information-terms/Category-4-water-information> ;
    skos:topConceptOf <http://www.neii.gov.au/def/voc/waterprogram/water-regulations-2008-water-information-terms/Water-Regulations-2008-water-information-terms> ;
.

<http://www.neii.gov.au/def/voc/waterprogram/water-regulations-2008-water-information-terms/subcategory-4i-water-information>
    a skos:Concept ;
    dcterms:contributor <https://linked.data.gov.au/org/neii> ;
    dcterms:created "2020-05-18"^^xsd:date ;
    dcterms:creator <https://linked.data.gov.au/org/neii> ;
    dcterms:modified "2020-05-18"^^xsd:date ;
    skos:definition """Vapour pressure deficit, expressed in millibars.
Source: Water Regulations 2008 (https://www.legislation.gov.au/Series/F2008L02170) Schedule 3 Part 5."""@en ;
    skos:notation "84" ;
    skos:prefLabel "subcategory 4i water information"@en ;
    skos:related <http://www.neii.gov.au/def/voc/waterprogram/water-regulations-2008-water-information-terms/Category-4-water-information> ;
    skos:topConceptOf <http://www.neii.gov.au/def/voc/waterprogram/water-regulations-2008-water-information-terms/Water-Regulations-2008-water-information-terms> ;
.

<http://www.neii.gov.au/def/voc/waterprogram/water-regulations-2008-water-information-terms/subcategory-4j-water-information>
    a skos:Concept ;
    dcterms:contributor <https://linked.data.gov.au/org/neii> ;
    dcterms:created "2020-05-18"^^xsd:date ;
    dcterms:creator <https://linked.data.gov.au/org/neii> ;
    dcterms:modified "2020-05-18"^^xsd:date ;
    skos:definition """Dewpoint temperature, expressed in degrees Celsius.
Source: Water Regulations 2008 (https://www.legislation.gov.au/Series/F2008L02170) Schedule 3 Part 5."""@en ;
    skos:notation "85" ;
    skos:prefLabel "subcategory 4j water information"@en ;
    skos:related <http://www.neii.gov.au/def/voc/waterprogram/water-regulations-2008-water-information-terms/Category-4-water-information> ;
    skos:topConceptOf <http://www.neii.gov.au/def/voc/waterprogram/water-regulations-2008-water-information-terms/Water-Regulations-2008-water-information-terms> ;
.

<http://www.neii.gov.au/def/voc/waterprogram/water-regulations-2008-water-information-terms/subcategory-5a-water-information>
    a skos:Concept ;
    dcterms:contributor <https://linked.data.gov.au/org/neii> ;
    dcterms:created "2020-05-18"^^xsd:date ;
    dcterms:creator <https://linked.data.gov.au/org/neii> ;
    dcterms:modified "2020-05-18"^^xsd:date ;
    skos:definition """Total volume of surface water take in each water management area, expressed in megalitres.
Source: Water Regulations 2008 (https://www.legislation.gov.au/Series/F2008L02170) Schedule 3 Part 6."""@en ;
    skos:notation "86" ;
    skos:prefLabel "subcategory 5a water information"@en ;
    skos:related <http://www.neii.gov.au/def/voc/waterprogram/water-regulations-2008-water-information-terms/Category-5-water-information> ;
    skos:topConceptOf <http://www.neii.gov.au/def/voc/waterprogram/water-regulations-2008-water-information-terms/Water-Regulations-2008-water-information-terms> ;
.

<http://www.neii.gov.au/def/voc/waterprogram/water-regulations-2008-water-information-terms/subcategory-5b-water-information>
    a skos:Concept ;
    dcterms:contributor <https://linked.data.gov.au/org/neii> ;
    dcterms:created "2020-05-18"^^xsd:date ;
    dcterms:creator <https://linked.data.gov.au/org/neii> ;
    dcterms:modified "2020-05-18"^^xsd:date ;
    skos:definition """Volume of surface water take for irrigation networks in each water management area, expressed in megalitres.
Source: Water Regulations 2008 (https://www.legislation.gov.au/Series/F2008L02170) Schedule 3 Part 6."""@en ;
    skos:notation "87" ;
    skos:prefLabel "subcategory 5b water information"@en ;
    skos:related <http://www.neii.gov.au/def/voc/waterprogram/water-regulations-2008-water-information-terms/Category-5-water-information> ;
    skos:topConceptOf <http://www.neii.gov.au/def/voc/waterprogram/water-regulations-2008-water-information-terms/Water-Regulations-2008-water-information-terms> ;
.

<http://www.neii.gov.au/def/voc/waterprogram/water-regulations-2008-water-information-terms/subcategory-5c-water-information>
    a skos:Concept ;
    dcterms:contributor <https://linked.data.gov.au/org/neii> ;
    dcterms:created "2020-05-18"^^xsd:date ;
    dcterms:creator <https://linked.data.gov.au/org/neii> ;
    dcterms:modified "2020-05-18"^^xsd:date ;
    skos:definition """Volume of surface water returned from irrigation networks to a watercourse in each water management area, expressed in megalitres.
Source: Water Regulations 2008 (https://www.legislation.gov.au/Series/F2008L02170) Schedule 3 Part 6."""@en ;
    skos:notation "88" ;
    skos:prefLabel "subcategory 5c water information"@en ;
    skos:related <http://www.neii.gov.au/def/voc/waterprogram/water-regulations-2008-water-information-terms/Category-5-water-information> ;
    skos:topConceptOf <http://www.neii.gov.au/def/voc/waterprogram/water-regulations-2008-water-information-terms/Water-Regulations-2008-water-information-terms> ;
.

<http://www.neii.gov.au/def/voc/waterprogram/water-regulations-2008-water-information-terms/subcategory-5d-water-information>
    a skos:Concept ;
    dcterms:contributor <https://linked.data.gov.au/org/neii> ;
    dcterms:created "2020-05-18"^^xsd:date ;
    dcterms:creator <https://linked.data.gov.au/org/neii> ;
    dcterms:modified "2020-05-18"^^xsd:date ;
    skos:definition """Volume of surface water take (excluding take for irrigation networks) in each water management area, expressed in megalitres.
Source: Water Regulations 2008 (https://www.legislation.gov.au/Series/F2008L02170) Schedule 3 Part 6."""@en ;
    skos:notation "89" ;
    skos:prefLabel "subcategory 5d water information"@en ;
    skos:related <http://www.neii.gov.au/def/voc/waterprogram/water-regulations-2008-water-information-terms/Category-5-water-information> ;
    skos:topConceptOf <http://www.neii.gov.au/def/voc/waterprogram/water-regulations-2008-water-information-terms/Water-Regulations-2008-water-information-terms> ;
.

<http://www.neii.gov.au/def/voc/waterprogram/water-regulations-2008-water-information-terms/subcategory-5e-water-information>
    a skos:Concept ;
    dcterms:contributor <https://linked.data.gov.au/org/neii> ;
    dcterms:created "2020-05-18"^^xsd:date ;
    dcterms:creator <https://linked.data.gov.au/org/neii> ;
    dcterms:modified "2020-05-18"^^xsd:date ;
    skos:definition """Volume of water delivered to a surface water resource through inter-basin transfer (excluding transfers relating to water trades) in each water management area, expressed in megalitres.
Source: Water Regulations 2008 (https://www.legislation.gov.au/Series/F2008L02170) Schedule 3 Part 6."""@en ;
    skos:notation "90" ;
    skos:prefLabel "subcategory 5e water information"@en ;
    skos:related <http://www.neii.gov.au/def/voc/waterprogram/water-regulations-2008-water-information-terms/Category-5-water-information> ;
    skos:topConceptOf <http://www.neii.gov.au/def/voc/waterprogram/water-regulations-2008-water-information-terms/Water-Regulations-2008-water-information-terms> ;
.

<http://www.neii.gov.au/def/voc/waterprogram/water-regulations-2008-water-information-terms/subcategory-5f-water-information>
    a skos:Concept ;
    dcterms:contributor <https://linked.data.gov.au/org/neii> ;
    dcterms:created "2020-05-18"^^xsd:date ;
    dcterms:creator <https://linked.data.gov.au/org/neii> ;
    dcterms:modified "2020-05-18"^^xsd:date ;
    skos:definition """Volume of ground water extracted under each ground water licence, expressed in megalitres.
Source: Water Regulations 2008 (https://www.legislation.gov.au/Series/F2008L02170) Schedule 3 Part 6."""@en ;
    skos:notation "91" ;
    skos:prefLabel "subcategory 5f water information"@en ;
    skos:related <http://www.neii.gov.au/def/voc/waterprogram/water-regulations-2008-water-information-terms/Category-5-water-information> ;
    skos:topConceptOf <http://www.neii.gov.au/def/voc/waterprogram/water-regulations-2008-water-information-terms/Water-Regulations-2008-water-information-terms> ;
.

<http://www.neii.gov.au/def/voc/waterprogram/water-regulations-2008-water-information-terms/subcategory-5g-water-information>
    a skos:Concept ;
    dcterms:contributor <https://linked.data.gov.au/org/neii> ;
    dcterms:created "2020-05-18"^^xsd:date ;
    dcterms:creator <https://linked.data.gov.au/org/neii> ;
    dcterms:modified "2020-05-18"^^xsd:date ;
    skos:definition """Volume of ground water extracted under each water management area, otherwise than under a ground water licence, expressed in megalitres.
Source: Water Regulations 2008 (https://www.legislation.gov.au/Series/F2008L02170) Schedule 3 Part 6."""@en ;
    skos:notation "92" ;
    skos:prefLabel "subcategory 5g water information"@en ;
    skos:related <http://www.neii.gov.au/def/voc/waterprogram/water-regulations-2008-water-information-terms/Category-5-water-information> ;
    skos:topConceptOf <http://www.neii.gov.au/def/voc/waterprogram/water-regulations-2008-water-information-terms/Water-Regulations-2008-water-information-terms> ;
.

<http://www.neii.gov.au/def/voc/waterprogram/water-regulations-2008-water-information-terms/subcategory-5h-water-information>
    a skos:Concept ;
    dcterms:contributor <https://linked.data.gov.au/org/neii> ;
    dcterms:created "2020-05-18"^^xsd:date ;
    dcterms:creator <https://linked.data.gov.au/org/neii> ;
    dcterms:modified "2020-05-18"^^xsd:date ;
    skos:definition """Volume of water delivered to a ground water resource for aquifer replenishment in each water management area, expressed in megalitres.
Source: Water Regulations 2008 (https://www.legislation.gov.au/Series/F2008L02170) Schedule 3 Part 6."""@en ;
    skos:notation "93" ;
    skos:prefLabel "subcategory 5h water information"@en ;
    skos:related <http://www.neii.gov.au/def/voc/waterprogram/water-regulations-2008-water-information-terms/Category-5-water-information> ;
    skos:topConceptOf <http://www.neii.gov.au/def/voc/waterprogram/water-regulations-2008-water-information-terms/Water-Regulations-2008-water-information-terms> ;
.

<http://www.neii.gov.au/def/voc/waterprogram/water-regulations-2008-water-information-terms/subcategory-6a-water-information>
    a skos:Concept ;
    dcterms:contributor <https://linked.data.gov.au/org/neii> ;
    dcterms:created "2020-05-18"^^xsd:date ;
    dcterms:creator <https://linked.data.gov.au/org/neii> ;
    dcterms:modified "2020-05-18"^^xsd:date ;
    skos:definition """Water access rights
Source: Water Regulations 2008 (https://www.legislation.gov.au/Series/F2008L02170) Schedule 3 Part 7."""@en ;
    skos:notation "94" ;
    skos:prefLabel "subcategory 6a water information"@en ;
    skos:related <http://www.neii.gov.au/def/voc/waterprogram/water-regulations-2008-water-information-terms/Category-6-water-information> ;
    skos:topConceptOf <http://www.neii.gov.au/def/voc/waterprogram/water-regulations-2008-water-information-terms/Water-Regulations-2008-water-information-terms> ;
.

<http://www.neii.gov.au/def/voc/waterprogram/water-regulations-2008-water-information-terms/subcategory-6b-water-information>
    a skos:Concept ;
    dcterms:contributor <https://linked.data.gov.au/org/neii> ;
    dcterms:created "2020-05-18"^^xsd:date ;
    dcterms:creator <https://linked.data.gov.au/org/neii> ;
    dcterms:modified "2020-05-18"^^xsd:date ;
    skos:definition """Trades or leases of Australian water access entitlements and irrigation rights
Source: Water Regulations 2008 (https://www.legislation.gov.au/Series/F2008L02170) Schedule 3 Part 7."""@en ;
    skos:notation "95" ;
    skos:prefLabel "subcategory 6b water information"@en ;
    skos:related <http://www.neii.gov.au/def/voc/waterprogram/water-regulations-2008-water-information-terms/Category-6-water-information> ;
    skos:topConceptOf <http://www.neii.gov.au/def/voc/waterprogram/water-regulations-2008-water-information-terms/Water-Regulations-2008-water-information-terms> ;
.

<http://www.neii.gov.au/def/voc/waterprogram/water-regulations-2008-water-information-terms/subcategory-6c-water-information>
    a skos:Concept ;
    dcterms:contributor <https://linked.data.gov.au/org/neii> ;
    dcterms:created "2020-05-18"^^xsd:date ;
    dcterms:creator <https://linked.data.gov.au/org/neii> ;
    dcterms:modified "2020-05-18"^^xsd:date ;
    skos:definition """Trades of Australian water allocations
Source: Water Regulations 2008 (https://www.legislation.gov.au/Series/F2008L02170) Schedule 3 Part 7."""@en ;
    skos:notation "96" ;
    skos:prefLabel "subcategory 6c water information"@en ;
    skos:related <http://www.neii.gov.au/def/voc/waterprogram/water-regulations-2008-water-information-terms/Category-6-water-information> ;
    skos:topConceptOf <http://www.neii.gov.au/def/voc/waterprogram/water-regulations-2008-water-information-terms/Water-Regulations-2008-water-information-terms> ;
.

<http://www.neii.gov.au/def/voc/waterprogram/water-regulations-2008-water-information-terms/subcategory-6d-water-information>
    a skos:Concept ;
    dcterms:contributor <https://linked.data.gov.au/org/neii> ;
    dcterms:created "2020-05-18"^^xsd:date ;
    dcterms:creator <https://linked.data.gov.au/org/neii> ;
    dcterms:modified "2020-05-18"^^xsd:date ;
    skos:definition """Formal announcements of Australian water allocations
Source: Water Regulations 2008 (https://www.legislation.gov.au/Series/F2008L02170) Schedule 3 Part 7."""@en ;
    skos:notation "97" ;
    skos:prefLabel "subcategory 6d water information"@en ;
    skos:related <http://www.neii.gov.au/def/voc/waterprogram/water-regulations-2008-water-information-terms/Category-6-water-information> ;
    skos:topConceptOf <http://www.neii.gov.au/def/voc/waterprogram/water-regulations-2008-water-information-terms/Water-Regulations-2008-water-information-terms> ;
.

<http://www.neii.gov.au/def/voc/waterprogram/water-regulations-2008-water-information-terms/subcategory-6e-water-information>
    a skos:Concept ;
    dcterms:contributor <https://linked.data.gov.au/org/neii> ;
    dcterms:created "2020-05-18"^^xsd:date ;
    dcterms:creator <https://linked.data.gov.au/org/neii> ;
    dcterms:modified "2020-05-18"^^xsd:date ;
    skos:definition """Permits to operate or construct a minor storage
Source: Water Regulations 2008 (https://www.legislation.gov.au/Series/F2008L02170) Schedule 3 Part 7."""@en ;
    skos:notation "98" ;
    skos:prefLabel "subcategory 6e water information"@en ;
    skos:related <http://www.neii.gov.au/def/voc/waterprogram/water-regulations-2008-water-information-terms/Category-6-water-information> ;
    skos:topConceptOf <http://www.neii.gov.au/def/voc/waterprogram/water-regulations-2008-water-information-terms/Water-Regulations-2008-water-information-terms> ;
.

<http://www.neii.gov.au/def/voc/waterprogram/water-regulations-2008-water-information-terms/subcategory-6f-water-information>
    a skos:Concept ;
    dcterms:contributor <https://linked.data.gov.au/org/neii> ;
    dcterms:created "2020-05-18"^^xsd:date ;
    dcterms:creator <https://linked.data.gov.au/org/neii> ;
    dcterms:modified "2020-05-18"^^xsd:date ;
    skos:definition """Permits to self extract water from a bore
Source: Water Regulations 2008 (https://www.legislation.gov.au/Series/F2008L02170) Schedule 3 Part 7."""@en ;
    skos:notation "99" ;
    skos:prefLabel "subcategory 6f water information"@en ;
    skos:related <http://www.neii.gov.au/def/voc/waterprogram/water-regulations-2008-water-information-terms/Category-6-water-information> ;
    skos:topConceptOf <http://www.neii.gov.au/def/voc/waterprogram/water-regulations-2008-water-information-terms/Water-Regulations-2008-water-information-terms> ;
.

<http://www.neii.gov.au/def/voc/waterprogram/water-regulations-2008-water-information-terms/subcategory-6g-water-information>
    a skos:Concept ;
    dcterms:contributor <https://linked.data.gov.au/org/neii> ;
    dcterms:created "2020-05-18"^^xsd:date ;
    dcterms:creator <https://linked.data.gov.au/org/neii> ;
    dcterms:modified "2020-05-18"^^xsd:date ;
    skos:definition """Permits to self extract water from a watercourse
Source: Water Regulations 2008 (https://www.legislation.gov.au/Series/F2008L02170) Schedule 3 Part 7."""@en ;
    skos:notation "100" ;
    skos:prefLabel "subcategory 6g water information"@en ;
    skos:related <http://www.neii.gov.au/def/voc/waterprogram/water-regulations-2008-water-information-terms/Category-6-water-information> ;
    skos:topConceptOf <http://www.neii.gov.au/def/voc/waterprogram/water-regulations-2008-water-information-terms/Water-Regulations-2008-water-information-terms> ;
.

<http://www.neii.gov.au/def/voc/waterprogram/water-regulations-2008-water-information-terms/subcategory-7a-water-information>
    a skos:Concept ;
    dcterms:contributor <https://linked.data.gov.au/org/neii> ;
    dcterms:created "2020-05-18"^^xsd:date ;
    dcterms:creator <https://linked.data.gov.au/org/neii> ;
    dcterms:modified "2020-05-18"^^xsd:date ;
    skos:definition """Urban water supply information, provided as volumes and expressed in megalitres, of a kind specified for the purposes of this item in the document titled Urban Water Management Information Requirements (http://www.bom.gov.au/water/regulations/schedules/urbanWater.shtml) (see Regulation 1.06).
Source: Water Regulations 2008 (https://www.legislation.gov.au/Series/F2008L02170) Schedule 3 Part 8."""@en ;
    skos:notation "101" ;
    skos:prefLabel "subcategory 7a water information"@en ;
    skos:related <http://www.neii.gov.au/def/voc/waterprogram/water-regulations-2008-water-information-terms/Category-7-water-information> ;
    skos:topConceptOf <http://www.neii.gov.au/def/voc/waterprogram/water-regulations-2008-water-information-terms/Water-Regulations-2008-water-information-terms> ;
.

<http://www.neii.gov.au/def/voc/waterprogram/water-regulations-2008-water-information-terms/subcategory-7b-water-information>
    a skos:Concept ;
    dcterms:contributor <https://linked.data.gov.au/org/neii> ;
    dcterms:created "2020-05-18"^^xsd:date ;
    dcterms:creator <https://linked.data.gov.au/org/neii> ;
    dcterms:modified "2020-05-18"^^xsd:date ;
    skos:definition """Urban wastewater information, provided as volumes and expressed in megalitres, of a kind specified for the purposes of this item in the document titled Urban Water Management Information Requirements (http://www.bom.gov.au/water/regulations/schedules/urbanWater.shtml) (see Regulation 1.06).
Source: Water Regulations 2008 (https://www.legislation.gov.au/Series/F2008L02170) Schedule 3 Part 8."""@en ;
    skos:notation "102" ;
    skos:prefLabel "subcategory 7b water information"@en ;
    skos:related <http://www.neii.gov.au/def/voc/waterprogram/water-regulations-2008-water-information-terms/Category-7-water-information> ;
    skos:topConceptOf <http://www.neii.gov.au/def/voc/waterprogram/water-regulations-2008-water-information-terms/Water-Regulations-2008-water-information-terms> ;
.

<http://www.neii.gov.au/def/voc/waterprogram/water-regulations-2008-water-information-terms/subcategory-7c-water-information>
    a skos:Concept ;
    dcterms:contributor <https://linked.data.gov.au/org/neii> ;
    dcterms:created "2020-05-18"^^xsd:date ;
    dcterms:creator <https://linked.data.gov.au/org/neii> ;
    dcterms:modified "2020-05-18"^^xsd:date ;
    skos:definition """Urban recycled water information, provided as volumes and expressed in megalitres, of a kind specified for the purposes of this item in the document titled Urban Water Management Information Requirements (http://www.bom.gov.au/water/regulations/schedules/urbanWater.shtml) (see Regulation 1.06).
Source: Water Regulations 2008 (https://www.legislation.gov.au/Series/F2008L02170) Schedule 3 Part 8."""@en ;
    skos:notation "103" ;
    skos:prefLabel "subcategory 7c water information"@en ;
    skos:related <http://www.neii.gov.au/def/voc/waterprogram/water-regulations-2008-water-information-terms/Category-7-water-information> ;
    skos:topConceptOf <http://www.neii.gov.au/def/voc/waterprogram/water-regulations-2008-water-information-terms/Water-Regulations-2008-water-information-terms> ;
.

<http://www.neii.gov.au/def/voc/waterprogram/water-regulations-2008-water-information-terms/subcategory-7d-water-information>
    a skos:Concept ;
    dcterms:contributor <https://linked.data.gov.au/org/neii> ;
    dcterms:created "2020-05-18"^^xsd:date ;
    dcterms:creator <https://linked.data.gov.au/org/neii> ;
    dcterms:modified "2020-05-18"^^xsd:date ;
    skos:definition """Urban stormwater information, provided as volumes and expressed in megalitres, of a kind specified for the purposes of this item in the document titled Urban Water Management Information Requirements (http://www.bom.gov.au/water/regulations/schedules/urbanWater.shtml) (see Regulation 1.06).
Source: Water Regulations 2008 (https://www.legislation.gov.au/Series/F2008L02170) Schedule 3 Part 8."""@en ;
    skos:notation "104" ;
    skos:prefLabel "subcategory 7d water information"@en ;
    skos:related <http://www.neii.gov.au/def/voc/waterprogram/water-regulations-2008-water-information-terms/Category-7-water-information> ;
    skos:topConceptOf <http://www.neii.gov.au/def/voc/waterprogram/water-regulations-2008-water-information-terms/Water-Regulations-2008-water-information-terms> ;
.

<http://www.neii.gov.au/def/voc/waterprogram/water-regulations-2008-water-information-terms/subcategory-8a-water-information>
    a skos:Concept ;
    dcterms:contributor <https://linked.data.gov.au/org/neii> ;
    dcterms:created "2020-05-18"^^xsd:date ;
    dcterms:creator <https://linked.data.gov.au/org/neii> ;
    dcterms:modified "2020-05-18"^^xsd:date ;
    skos:definition """Water use restriction announcements
Source: Water Regulations 2008 (https://www.legislation.gov.au/Series/F2008L02170) Schedule 3 Part 9."""@en ;
    skos:notation "105" ;
    skos:prefLabel "subcategory 8a water information"@en ;
    skos:related <http://www.neii.gov.au/def/voc/waterprogram/water-regulations-2008-water-information-terms/Category-8-water-information> ;
    skos:topConceptOf <http://www.neii.gov.au/def/voc/waterprogram/water-regulations-2008-water-information-terms/Water-Regulations-2008-water-information-terms> ;
.

<http://www.neii.gov.au/def/voc/waterprogram/water-regulations-2008-water-information-terms/subcategory-9a-water-information>
    a skos:Concept ;
    dcterms:contributor <https://linked.data.gov.au/org/neii> ;
    dcterms:created "2020-05-18"^^xsd:date ;
    dcterms:creator <https://linked.data.gov.au/org/neii> ;
    dcterms:modified "2020-05-18"^^xsd:date ;
    skos:definition """Electrical conductivity of surface water above the tidal limit of a watercourse, expressed in microsiemens per centimetre at 25 C.
Source: Water Regulations 2008 (https://www.legislation.gov.au/Series/F2008L02170) Schedule 3 Part 10."""@en ;
    skos:notation "106" ;
    skos:prefLabel "subcategory 9a water information"@en ;
    skos:related <http://www.neii.gov.au/def/voc/waterprogram/water-regulations-2008-water-information-terms/Category-9-water-information> ;
    skos:topConceptOf <http://www.neii.gov.au/def/voc/waterprogram/water-regulations-2008-water-information-terms/Water-Regulations-2008-water-information-terms> ;
.

<http://www.neii.gov.au/def/voc/waterprogram/water-regulations-2008-water-information-terms/subcategory-9b-water-information>
    a skos:Concept ;
    dcterms:contributor <https://linked.data.gov.au/org/neii> ;
    dcterms:created "2020-05-18"^^xsd:date ;
    dcterms:creator <https://linked.data.gov.au/org/neii> ;
    dcterms:modified "2020-05-18"^^xsd:date ;
    skos:definition """Electrical conductivity of ground water, expressed in microsiemens per centimetre at 25 C.
Source: Water Regulations 2008 (https://www.legislation.gov.au/Series/F2008L02170) Schedule 3 Part 10."""@en ;
    skos:notation "107" ;
    skos:prefLabel "subcategory 9b water information"@en ;
    skos:related <http://www.neii.gov.au/def/voc/waterprogram/water-regulations-2008-water-information-terms/Category-9-water-information> ;
    skos:topConceptOf <http://www.neii.gov.au/def/voc/waterprogram/water-regulations-2008-water-information-terms/Water-Regulations-2008-water-information-terms> ;
.

<http://www.neii.gov.au/def/voc/waterprogram/water-regulations-2008-water-information-terms/subcategory-9c-water-information>
    a skos:Concept ;
    dcterms:contributor <https://linked.data.gov.au/org/neii> ;
    dcterms:created "2020-05-18"^^xsd:date ;
    dcterms:creator <https://linked.data.gov.au/org/neii> ;
    dcterms:modified "2020-05-18"^^xsd:date ;
    skos:definition """Total suspended solids concentration of surface water collected above the tidal limit of a watercourse, expressed in milligrams per litre.
Source: Water Regulations 2008 (https://www.legislation.gov.au/Series/F2008L02170) Schedule 3 Part 10."""@en ;
    skos:notation "108" ;
    skos:prefLabel "subcategory 9c water information"@en ;
    skos:related <http://www.neii.gov.au/def/voc/waterprogram/water-regulations-2008-water-information-terms/Category-9-water-information> ;
    skos:topConceptOf <http://www.neii.gov.au/def/voc/waterprogram/water-regulations-2008-water-information-terms/Water-Regulations-2008-water-information-terms> ;
.

<http://www.neii.gov.au/def/voc/waterprogram/water-regulations-2008-water-information-terms/subcategory-9d-water-information>
    a skos:Concept ;
    dcterms:contributor <https://linked.data.gov.au/org/neii> ;
    dcterms:created "2020-05-18"^^xsd:date ;
    dcterms:creator <https://linked.data.gov.au/org/neii> ;
    dcterms:modified "2020-05-18"^^xsd:date ;
    skos:definition """Turbidity of surface water above the tidal limit of a watercourse, expressed in nephelometric turbidity units.
Source: Water Regulations 2008 (https://www.legislation.gov.au/Series/F2008L02170) Schedule 3 Part 10."""@en ;
    skos:notation "109" ;
    skos:prefLabel "subcategory 9d water information"@en ;
    skos:related <http://www.neii.gov.au/def/voc/waterprogram/water-regulations-2008-water-information-terms/Category-9-water-information> ;
    skos:topConceptOf <http://www.neii.gov.au/def/voc/waterprogram/water-regulations-2008-water-information-terms/Water-Regulations-2008-water-information-terms> ;
.

<http://www.neii.gov.au/def/voc/waterprogram/water-regulations-2008-water-information-terms/subcategory-9e-water-information>
    a skos:Concept ;
    dcterms:contributor <https://linked.data.gov.au/org/neii> ;
    dcterms:created "2020-05-18"^^xsd:date ;
    dcterms:creator <https://linked.data.gov.au/org/neii> ;
    dcterms:modified "2020-05-18"^^xsd:date ;
    skos:definition """Total phosphorus concentration of a surface water sample collected above the tidal limit of a watercourse, expressed in milligrams per litre.
Source: Water Regulations 2008 (https://www.legislation.gov.au/Series/F2008L02170) Schedule 3 Part 10."""@en ;
    skos:notation "110" ;
    skos:prefLabel "subcategory 9e water information"@en ;
    skos:related <http://www.neii.gov.au/def/voc/waterprogram/water-regulations-2008-water-information-terms/Category-9-water-information> ;
    skos:topConceptOf <http://www.neii.gov.au/def/voc/waterprogram/water-regulations-2008-water-information-terms/Water-Regulations-2008-water-information-terms> ;
.

<http://www.neii.gov.au/def/voc/waterprogram/water-regulations-2008-water-information-terms/subcategory-9f-water-information>
    a skos:Concept ;
    dcterms:contributor <https://linked.data.gov.au/org/neii> ;
    dcterms:created "2020-05-18"^^xsd:date ;
    dcterms:creator <https://linked.data.gov.au/org/neii> ;
    dcterms:modified "2020-05-18"^^xsd:date ;
    skos:definition """Total nitrogen concentration of a surface water sample collected above the tidal limit of a watercourse, expressed in milligrams per litre.
Source: Water Regulations 2008 (https://www.legislation.gov.au/Series/F2008L02170) Schedule 3 Part 10."""@en ;
    skos:notation "111" ;
    skos:prefLabel "subcategory 9f water information"@en ;
    skos:related <http://www.neii.gov.au/def/voc/waterprogram/water-regulations-2008-water-information-terms/Category-9-water-information> ;
    skos:topConceptOf <http://www.neii.gov.au/def/voc/waterprogram/water-regulations-2008-water-information-terms/Water-Regulations-2008-water-information-terms> ;
.

<http://www.neii.gov.au/def/voc/waterprogram/water-regulations-2008-water-information-terms/subcategory-9g-water-information>
    a skos:Concept ;
    dcterms:contributor <https://linked.data.gov.au/org/neii> ;
    dcterms:created "2020-05-18"^^xsd:date ;
    dcterms:creator <https://linked.data.gov.au/org/neii> ;
    dcterms:modified "2020-05-19"^^xsd:date ;
    skos:definition """pH of surface water collected above the tidal limit of a watercourse
Source: Water Regulations 2008 (https://www.legislation.gov.au/Series/F2008L02170) Schedule 3 Part 10."""@en ;
    skos:notation "112" ;
    skos:prefLabel "subcategory 9g water information"@en ;
    skos:related <http://www.neii.gov.au/def/voc/waterprogram/water-regulations-2008-water-information-terms/Category-9-water-information> ;
    skos:topConceptOf <http://www.neii.gov.au/def/voc/waterprogram/water-regulations-2008-water-information-terms/Water-Regulations-2008-water-information-terms> ;
.

<http://www.neii.gov.au/def/voc/waterprogram/water-regulations-2008-water-information-terms/subcategory-9ga-water-information>
    a skos:Concept ;
    dcterms:contributor <https://linked.data.gov.au/org/neii> ;
    dcterms:created "2020-05-18"^^xsd:date ;
    dcterms:creator <https://linked.data.gov.au/org/neii> ;
    dcterms:modified "2020-05-19"^^xsd:date ;
    skos:definition """pH of ground water
Source: Water Regulations 2008 (https://www.legislation.gov.au/Series/F2008L02170) Schedule 3 Part 10."""@en ;
    skos:notation "113" ;
    skos:prefLabel "subcategory 9ga water information"@en ;
    skos:related <http://www.neii.gov.au/def/voc/waterprogram/water-regulations-2008-water-information-terms/Category-9-water-information> ;
    skos:topConceptOf <http://www.neii.gov.au/def/voc/waterprogram/water-regulations-2008-water-information-terms/Water-Regulations-2008-water-information-terms> ;
.

<http://www.neii.gov.au/def/voc/waterprogram/water-regulations-2008-water-information-terms/subcategory-9h-water-information>
    a skos:Concept ;
    dcterms:contributor <https://linked.data.gov.au/org/neii> ;
    dcterms:created "2020-05-18"^^xsd:date ;
    dcterms:creator <https://linked.data.gov.au/org/neii> ;
    dcterms:modified "2020-05-18"^^xsd:date ;
    skos:definition """Temperature of surface water collected above the tidal limit of a watercourse, expressed in degrees Celsius.
Source: Water Regulations 2008 (https://www.legislation.gov.au/Series/F2008L02170) Schedule 3 Part 10."""@en ;
    skos:notation "114" ;
    skos:prefLabel "subcategory 9h water information"@en ;
    skos:related <http://www.neii.gov.au/def/voc/waterprogram/water-regulations-2008-water-information-terms/Category-9-water-information> ;
    skos:topConceptOf <http://www.neii.gov.au/def/voc/waterprogram/water-regulations-2008-water-information-terms/Water-Regulations-2008-water-information-terms> ;
.

<http://www.neii.gov.au/def/voc/waterprogram/water-regulations-2008-water-information-terms/Category-1-water-information>
    a skos:Concept ;
    dcterms:contributor <https://linked.data.gov.au/org/neii> ;
    dcterms:created "2020-05-18"^^xsd:date ;
    dcterms:creator <https://linked.data.gov.au/org/neii> ;
    dcterms:modified "2020-05-18"^^xsd:date ;
    skos:definition """Surface water resource information
Source: Water Regulations 2008 (https://www.legislation.gov.au/Series/F2008L02170) Schedule 3 Part 2."""@en ;
    skos:notation "8" ;
    skos:prefLabel "Category 1 water information"@en ;
    skos:related
        <http://www.neii.gov.au/def/voc/waterprogram/water-regulations-2008-water-information-terms/subcategory-1a-water-information> ,
        <http://www.neii.gov.au/def/voc/waterprogram/water-regulations-2008-water-information-terms/subcategory-1b-water-information> ;
    skos:topConceptOf <http://www.neii.gov.au/def/voc/waterprogram/water-regulations-2008-water-information-terms/Water-Regulations-2008-water-information-terms> ;
.

<http://www.neii.gov.au/def/voc/waterprogram/water-regulations-2008-water-information-terms/Category-11-water-information>
    a skos:Concept ;
    dcterms:contributor <https://linked.data.gov.au/org/neii> ;
    dcterms:created "2020-05-18"^^xsd:date ;
    dcterms:creator <https://linked.data.gov.au/org/neii> ;
    dcterms:modified "2020-05-18"^^xsd:date ;
    skos:definition """Water information for flood warning purposes
Source: Water Regulations 2008 (https://www.legislation.gov.au/Series/F2008L02170) Schedule 3 Part 11."""@en ;
    skos:notation "17" ;
    skos:prefLabel "Category 11 water information"@en ;
    skos:related
        <http://www.neii.gov.au/def/voc/waterprogram/water-regulations-2008-water-information-terms/subcategory-11a-water-information> ,
        <http://www.neii.gov.au/def/voc/waterprogram/water-regulations-2008-water-information-terms/subcategory-11b-water-information> ,
        <http://www.neii.gov.au/def/voc/waterprogram/water-regulations-2008-water-information-terms/subcategory-11c-water-information> ;
    skos:topConceptOf <http://www.neii.gov.au/def/voc/waterprogram/water-regulations-2008-water-information-terms/Water-Regulations-2008-water-information-terms> ;
.

<http://www.neii.gov.au/def/voc/waterprogram/water-regulations-2008-water-information-terms/Category-2-water-information>
    a skos:Concept ;
    dcterms:contributor <https://linked.data.gov.au/org/neii> ;
    dcterms:created "2020-05-18"^^xsd:date ;
    dcterms:creator <https://linked.data.gov.au/org/neii> ;
    dcterms:modified "2020-05-18"^^xsd:date ;
    skos:definition """Ground water resource information
Source: Water Regulations 2008 (https://www.legislation.gov.au/Series/F2008L02170) Schedule 3 Part 3."""@en ;
    skos:notation "9" ;
    skos:prefLabel "Category 2 water information"@en ;
    skos:related
        <http://www.neii.gov.au/def/voc/waterprogram/water-regulations-2008-water-information-terms/subcategory-2a-water-information> ,
        <http://www.neii.gov.au/def/voc/waterprogram/water-regulations-2008-water-information-terms/subcategory-2b-water-information> ,
        <http://www.neii.gov.au/def/voc/waterprogram/water-regulations-2008-water-information-terms/subcategory-2d-water-information> ,
        <http://www.neii.gov.au/def/voc/waterprogram/water-regulations-2008-water-information-terms/subcategory-2e-water-information> ;
    skos:topConceptOf <http://www.neii.gov.au/def/voc/waterprogram/water-regulations-2008-water-information-terms/Water-Regulations-2008-water-information-terms> ;
.

<http://www.neii.gov.au/def/voc/waterprogram/water-regulations-2008-water-information-terms/Category-7-water-information>
    a skos:Concept ;
    dcterms:contributor <https://linked.data.gov.au/org/neii> ;
    dcterms:created "2020-05-18"^^xsd:date ;
    dcterms:creator <https://linked.data.gov.au/org/neii> ;
    dcterms:modified "2020-05-18"^^xsd:date ;
    skos:definition """Information about urban water management
Source: Water Regulations 2008 (https://www.legislation.gov.au/Series/F2008L02170) Schedule 3 Part 8."""@en ;
    skos:notation "14" ;
    skos:prefLabel "Category 7 water information"@en ;
    skos:related
        <http://www.neii.gov.au/def/voc/waterprogram/water-regulations-2008-water-information-terms/subcategory-7a-water-information> ,
        <http://www.neii.gov.au/def/voc/waterprogram/water-regulations-2008-water-information-terms/subcategory-7b-water-information> ,
        <http://www.neii.gov.au/def/voc/waterprogram/water-regulations-2008-water-information-terms/subcategory-7c-water-information> ,
        <http://www.neii.gov.au/def/voc/waterprogram/water-regulations-2008-water-information-terms/subcategory-7d-water-information> ;
    skos:topConceptOf <http://www.neii.gov.au/def/voc/waterprogram/water-regulations-2008-water-information-terms/Water-Regulations-2008-water-information-terms> ;
.

<http://www.neii.gov.au/def/voc/waterprogram/water-regulations-2008-water-information-terms/Category-3-water-information>
    a skos:Concept ;
    dcterms:contributor <https://linked.data.gov.au/org/neii> ;
    dcterms:created "2020-05-18"^^xsd:date ;
    dcterms:creator <https://linked.data.gov.au/org/neii> ;
    dcterms:modified "2020-05-18"^^xsd:date ;
    skos:definition """Water storage information
Source: Water Regulations 2008 (https://www.legislation.gov.au/Series/F2008L02170) Schedule 3 Part 4."""@en ;
    skos:notation "10" ;
    skos:prefLabel "Category 3 water information"@en ;
    skos:related
        <http://www.neii.gov.au/def/voc/waterprogram/water-regulations-2008-water-information-terms/subcategory-3a-water-information> ,
        <http://www.neii.gov.au/def/voc/waterprogram/water-regulations-2008-water-information-terms/subcategory-3b-water-information> ,
        <http://www.neii.gov.au/def/voc/waterprogram/water-regulations-2008-water-information-terms/subcategory-3c-water-information> ,
        <http://www.neii.gov.au/def/voc/waterprogram/water-regulations-2008-water-information-terms/subcategory-3d-water-information> ,
        <http://www.neii.gov.au/def/voc/waterprogram/water-regulations-2008-water-information-terms/subcategory-3da-water-information> ,
        <http://www.neii.gov.au/def/voc/waterprogram/water-regulations-2008-water-information-terms/subcategory-3e-water-information> ,
        <http://www.neii.gov.au/def/voc/waterprogram/water-regulations-2008-water-information-terms/subcategory-3f-water-information> ;
    skos:topConceptOf <http://www.neii.gov.au/def/voc/waterprogram/water-regulations-2008-water-information-terms/Water-Regulations-2008-water-information-terms> ;
.

<http://www.neii.gov.au/def/voc/waterprogram/water-regulations-2008-water-information-terms/Category-6-water-information>
    a skos:Concept ;
    dcterms:contributor <https://linked.data.gov.au/org/neii> ;
    dcterms:created "2020-05-18"^^xsd:date ;
    dcterms:creator <https://linked.data.gov.au/org/neii> ;
    dcterms:modified "2020-05-18"^^xsd:date ;
    skos:definition """Information about water rights, allocations and trades
Source: Water Regulations 2008 (https://www.legislation.gov.au/Series/F2008L02170) Schedule 3 Part 7."""@en ;
    skos:notation "13" ;
    skos:prefLabel "Category 6 water information"@en ;
    skos:related
        <http://www.neii.gov.au/def/voc/waterprogram/water-regulations-2008-water-information-terms/subcategory-6a-water-information> ,
        <http://www.neii.gov.au/def/voc/waterprogram/water-regulations-2008-water-information-terms/subcategory-6b-water-information> ,
        <http://www.neii.gov.au/def/voc/waterprogram/water-regulations-2008-water-information-terms/subcategory-6c-water-information> ,
        <http://www.neii.gov.au/def/voc/waterprogram/water-regulations-2008-water-information-terms/subcategory-6d-water-information> ,
        <http://www.neii.gov.au/def/voc/waterprogram/water-regulations-2008-water-information-terms/subcategory-6e-water-information> ,
        <http://www.neii.gov.au/def/voc/waterprogram/water-regulations-2008-water-information-terms/subcategory-6f-water-information> ,
        <http://www.neii.gov.au/def/voc/waterprogram/water-regulations-2008-water-information-terms/subcategory-6g-water-information> ;
    skos:topConceptOf <http://www.neii.gov.au/def/voc/waterprogram/water-regulations-2008-water-information-terms/Water-Regulations-2008-water-information-terms> ;
.

<http://www.neii.gov.au/def/voc/waterprogram/water-regulations-2008-water-information-terms/Category-5-water-information>
    a skos:Concept ;
    dcterms:contributor <https://linked.data.gov.au/org/neii> ;
    dcterms:created "2020-05-18"^^xsd:date ;
    dcterms:creator <https://linked.data.gov.au/org/neii> ;
    dcterms:modified "2020-05-18"^^xsd:date ;
    skos:definition """Water use information
Source: Water Regulations 2008 (https://www.legislation.gov.au/Series/F2008L02170) Schedule 3 Part 6."""@en ;
    skos:notation "12" ;
    skos:prefLabel "Category 5 water information"@en ;
    skos:related
        <http://www.neii.gov.au/def/voc/waterprogram/water-regulations-2008-water-information-terms/subcategory-5a-water-information> ,
        <http://www.neii.gov.au/def/voc/waterprogram/water-regulations-2008-water-information-terms/subcategory-5b-water-information> ,
        <http://www.neii.gov.au/def/voc/waterprogram/water-regulations-2008-water-information-terms/subcategory-5c-water-information> ,
        <http://www.neii.gov.au/def/voc/waterprogram/water-regulations-2008-water-information-terms/subcategory-5d-water-information> ,
        <http://www.neii.gov.au/def/voc/waterprogram/water-regulations-2008-water-information-terms/subcategory-5e-water-information> ,
        <http://www.neii.gov.au/def/voc/waterprogram/water-regulations-2008-water-information-terms/subcategory-5f-water-information> ,
        <http://www.neii.gov.au/def/voc/waterprogram/water-regulations-2008-water-information-terms/subcategory-5g-water-information> ,
        <http://www.neii.gov.au/def/voc/waterprogram/water-regulations-2008-water-information-terms/subcategory-5h-water-information> ;
    skos:topConceptOf <http://www.neii.gov.au/def/voc/waterprogram/water-regulations-2008-water-information-terms/Water-Regulations-2008-water-information-terms> ;
.

<http://www.neii.gov.au/def/voc/waterprogram/water-regulations-2008-water-information-terms/Category-9-water-information>
    a skos:Concept ;
    dcterms:contributor <https://linked.data.gov.au/org/neii> ;
    dcterms:created "2020-05-18"^^xsd:date ;
    dcterms:creator <https://linked.data.gov.au/org/neii> ;
    dcterms:modified "2020-05-18"^^xsd:date ;
    skos:definition """Water quality information
Source: Water Regulations 2008 (https://www.legislation.gov.au/Series/F2008L02170) Schedule 3 Part 10."""@en ;
    skos:notation "16" ;
    skos:prefLabel "Category 9 water information"@en ;
    skos:related
        <http://www.neii.gov.au/def/voc/waterprogram/water-regulations-2008-water-information-terms/subcategory-9a-water-information> ,
        <http://www.neii.gov.au/def/voc/waterprogram/water-regulations-2008-water-information-terms/subcategory-9b-water-information> ,
        <http://www.neii.gov.au/def/voc/waterprogram/water-regulations-2008-water-information-terms/subcategory-9c-water-information> ,
        <http://www.neii.gov.au/def/voc/waterprogram/water-regulations-2008-water-information-terms/subcategory-9d-water-information> ,
        <http://www.neii.gov.au/def/voc/waterprogram/water-regulations-2008-water-information-terms/subcategory-9e-water-information> ,
        <http://www.neii.gov.au/def/voc/waterprogram/water-regulations-2008-water-information-terms/subcategory-9f-water-information> ,
        <http://www.neii.gov.au/def/voc/waterprogram/water-regulations-2008-water-information-terms/subcategory-9g-water-information> ,
        <http://www.neii.gov.au/def/voc/waterprogram/water-regulations-2008-water-information-terms/subcategory-9ga-water-information> ,
        <http://www.neii.gov.au/def/voc/waterprogram/water-regulations-2008-water-information-terms/subcategory-9h-water-information> ;
    skos:topConceptOf <http://www.neii.gov.au/def/voc/waterprogram/water-regulations-2008-water-information-terms/Water-Regulations-2008-water-information-terms> ;
.

<http://www.neii.gov.au/def/voc/waterprogram/water-regulations-2008-water-information-terms/Category-4-water-information>
    a skos:Concept ;
    dcterms:contributor <https://linked.data.gov.au/org/neii> ;
    dcterms:created "2020-05-18"^^xsd:date ;
    dcterms:creator <https://linked.data.gov.au/org/neii> ;
    dcterms:modified "2020-05-18"^^xsd:date ;
    skos:definition """Meteorological information
Source: Water Regulations 2008 (https://www.legislation.gov.au/Series/F2008L02170) Schedule 3 Part 5."""@en ;
    skos:notation "11" ;
    skos:prefLabel "Category 4 water information"@en ;
    skos:related
        <http://www.neii.gov.au/def/voc/waterprogram/water-regulations-2008-water-information-terms/subcategory-4a-water-information> ,
        <http://www.neii.gov.au/def/voc/waterprogram/water-regulations-2008-water-information-terms/subcategory-4b-water-information> ,
        <http://www.neii.gov.au/def/voc/waterprogram/water-regulations-2008-water-information-terms/subcategory-4c-water-information> ,
        <http://www.neii.gov.au/def/voc/waterprogram/water-regulations-2008-water-information-terms/subcategory-4d-water-information> ,
        <http://www.neii.gov.au/def/voc/waterprogram/water-regulations-2008-water-information-terms/subcategory-4e-water-information> ,
        <http://www.neii.gov.au/def/voc/waterprogram/water-regulations-2008-water-information-terms/subcategory-4f-water-information> ,
        <http://www.neii.gov.au/def/voc/waterprogram/water-regulations-2008-water-information-terms/subcategory-4g-water-information> ,
        <http://www.neii.gov.au/def/voc/waterprogram/water-regulations-2008-water-information-terms/subcategory-4h-water-information> ,
        <http://www.neii.gov.au/def/voc/waterprogram/water-regulations-2008-water-information-terms/subcategory-4i-water-information> ,
        <http://www.neii.gov.au/def/voc/waterprogram/water-regulations-2008-water-information-terms/subcategory-4j-water-information> ;
    skos:topConceptOf <http://www.neii.gov.au/def/voc/waterprogram/water-regulations-2008-water-information-terms/Water-Regulations-2008-water-information-terms> ;
.

<http://www.neii.gov.au/def/voc/waterprogram/water-regulations-2008-water-information-terms/Water-Regulations-2008-water-information-terms>
    a skos:ConceptScheme ;
    dcterms:created "2020-05-18"^^xsd:date ;
    dcterms:creator <https://linked.data.gov.au/org/neii> ;
    dcterms:issued "2020-06-11" ;
    dcterms:title "Water Regulations 2008 water information terms"@en ;
    owl:versionInfo "Version 1" ;
    skos:hasTopConcept
        <http://www.neii.gov.au/def/voc/waterprogram/water-regulations-2008-water-information-terms/Australian-water-access-entitlement> ,
        <http://www.neii.gov.au/def/voc/waterprogram/water-regulations-2008-water-information-terms/Australian-water-allocation> ,
        <http://www.neii.gov.au/def/voc/waterprogram/water-regulations-2008-water-information-terms/Category> ,
        <http://www.neii.gov.au/def/voc/waterprogram/water-regulations-2008-water-information-terms/Category-1-water-information> ,
        <http://www.neii.gov.au/def/voc/waterprogram/water-regulations-2008-water-information-terms/Category-11-water-information> ,
        <http://www.neii.gov.au/def/voc/waterprogram/water-regulations-2008-water-information-terms/Category-2-water-information> ,
        <http://www.neii.gov.au/def/voc/waterprogram/water-regulations-2008-water-information-terms/Category-3-water-information> ,
        <http://www.neii.gov.au/def/voc/waterprogram/water-regulations-2008-water-information-terms/Category-4-water-information> ,
        <http://www.neii.gov.au/def/voc/waterprogram/water-regulations-2008-water-information-terms/Category-5-water-information> ,
        <http://www.neii.gov.au/def/voc/waterprogram/water-regulations-2008-water-information-terms/Category-6-water-information> ,
        <http://www.neii.gov.au/def/voc/waterprogram/water-regulations-2008-water-information-terms/Category-7-water-information> ,
        <http://www.neii.gov.au/def/voc/waterprogram/water-regulations-2008-water-information-terms/Category-8-water-information> ,
        <http://www.neii.gov.au/def/voc/waterprogram/water-regulations-2008-water-information-terms/Category-9-water-information> ,
        <http://www.neii.gov.au/def/voc/waterprogram/water-regulations-2008-water-information-terms/Category-A-person> ,
        <http://www.neii.gov.au/def/voc/waterprogram/water-regulations-2008-water-information-terms/Category-B-person> ,
        <http://www.neii.gov.au/def/voc/waterprogram/water-regulations-2008-water-information-terms/Category-C-person> ,
        <http://www.neii.gov.au/def/voc/waterprogram/water-regulations-2008-water-information-terms/Category-D-person> ,
        <http://www.neii.gov.au/def/voc/waterprogram/water-regulations-2008-water-information-terms/Category-E-person> ,
        <http://www.neii.gov.au/def/voc/waterprogram/water-regulations-2008-water-information-terms/Category-F-person> ,
        <http://www.neii.gov.au/def/voc/waterprogram/water-regulations-2008-water-information-terms/Category-G-person> ,
        <http://www.neii.gov.au/def/voc/waterprogram/water-regulations-2008-water-information-terms/Category-H-person> ,
        <http://www.neii.gov.au/def/voc/waterprogram/water-regulations-2008-water-information-terms/Category-K-person> ,
        <http://www.neii.gov.au/def/voc/waterprogram/water-regulations-2008-water-information-terms/Category-L-person> ,
        <http://www.neii.gov.au/def/voc/waterprogram/water-regulations-2008-water-information-terms/Category-M-person> ,
        <http://www.neii.gov.au/def/voc/waterprogram/water-regulations-2008-water-information-terms/Irrigation-water-scheme> ,
        <http://www.neii.gov.au/def/voc/waterprogram/water-regulations-2008-water-information-terms/Major-storage> ,
        <http://www.neii.gov.au/def/voc/waterprogram/water-regulations-2008-water-information-terms/Minor-storage> ,
        <http://www.neii.gov.au/def/voc/waterprogram/water-regulations-2008-water-information-terms/State-NGIS-information> ,
        <http://www.neii.gov.au/def/voc/waterprogram/water-regulations-2008-water-information-terms/State-aquifer-framework-information> ,
        <http://www.neii.gov.au/def/voc/waterprogram/water-regulations-2008-water-information-terms/U-code> ,
        <http://www.neii.gov.au/def/voc/waterprogram/water-regulations-2008-water-information-terms/W-indicator> ,
        <http://www.neii.gov.au/def/voc/waterprogram/water-regulations-2008-water-information-terms/bulk-water-charge> ,
        <http://www.neii.gov.au/def/voc/waterprogram/water-regulations-2008-water-information-terms/bulk-water-service> ,
        <http://www.neii.gov.au/def/voc/waterprogram/water-regulations-2008-water-information-terms/bulk-water-supplier> ,
        <http://www.neii.gov.au/def/voc/waterprogram/water-regulations-2008-water-information-terms/calendar-month> ,
        <http://www.neii.gov.au/def/voc/waterprogram/water-regulations-2008-water-information-terms/data-management-system> ,
        <http://www.neii.gov.au/def/voc/waterprogram/water-regulations-2008-water-information-terms/day> ,
        <http://www.neii.gov.au/def/voc/waterprogram/water-regulations-2008-water-information-terms/dewpoint-temperature> ,
        <http://www.neii.gov.au/def/voc/waterprogram/water-regulations-2008-water-information-terms/downward-longwave-exposure> ,
        <http://www.neii.gov.au/def/voc/waterprogram/water-regulations-2008-water-information-terms/downward-longwave-irradiance> ,
        <http://www.neii.gov.au/def/voc/waterprogram/water-regulations-2008-water-information-terms/dry-bulb-air-temperature> ,
        <http://www.neii.gov.au/def/voc/waterprogram/water-regulations-2008-water-information-terms/electrical-conductivity> ,
        <http://www.neii.gov.au/def/voc/waterprogram/water-regulations-2008-water-information-terms/electronic-format> ,
        <http://www.neii.gov.au/def/voc/waterprogram/water-regulations-2008-water-information-terms/exposure> ,
        <http://www.neii.gov.au/def/voc/waterprogram/water-regulations-2008-water-information-terms/global-solar-exposure> ,
        <http://www.neii.gov.au/def/voc/waterprogram/water-regulations-2008-water-information-terms/global-solar-irradiance> ,
        <http://www.neii.gov.au/def/voc/waterprogram/water-regulations-2008-water-information-terms/grace-period> ,
        <http://www.neii.gov.au/def/voc/waterprogram/water-regulations-2008-water-information-terms/groundwater> ,
        <http://www.neii.gov.au/def/voc/waterprogram/water-regulations-2008-water-information-terms/hour> ,
        <http://www.neii.gov.au/def/voc/waterprogram/water-regulations-2008-water-information-terms/irradiance> ,
        <http://www.neii.gov.au/def/voc/waterprogram/water-regulations-2008-water-information-terms/irrigation-network> ,
        <http://www.neii.gov.au/def/voc/waterprogram/water-regulations-2008-water-information-terms/irrigation-right> ,
        <http://www.neii.gov.au/def/voc/waterprogram/water-regulations-2008-water-information-terms/month> ,
        <http://www.neii.gov.au/def/voc/waterprogram/water-regulations-2008-water-information-terms/net-exposure> ,
        <http://www.neii.gov.au/def/voc/waterprogram/water-regulations-2008-water-information-terms/net-global-solar-exposure> ,
        <http://www.neii.gov.au/def/voc/waterprogram/water-regulations-2008-water-information-terms/net-global-solar-irradiance> ,
        <http://www.neii.gov.au/def/voc/waterprogram/water-regulations-2008-water-information-terms/net-irradiance> ,
        <http://www.neii.gov.au/def/voc/waterprogram/water-regulations-2008-water-information-terms/net-longwave-exposure> ,
        <http://www.neii.gov.au/def/voc/waterprogram/water-regulations-2008-water-information-terms/net-longwave-irradiance> ,
        <http://www.neii.gov.au/def/voc/waterprogram/water-regulations-2008-water-information-terms/plant> ,
        <http://www.neii.gov.au/def/voc/waterprogram/water-regulations-2008-water-information-terms/reflected-global-solar-exposure> ,
        <http://www.neii.gov.au/def/voc/waterprogram/water-regulations-2008-water-information-terms/reflected-global-solar-irradiance> ,
        <http://www.neii.gov.au/def/voc/waterprogram/water-regulations-2008-water-information-terms/self-extract> ,
        <http://www.neii.gov.au/def/voc/waterprogram/water-regulations-2008-water-information-terms/subcategory> ,
        <http://www.neii.gov.au/def/voc/waterprogram/water-regulations-2008-water-information-terms/subcategory-11a-water-information> ,
        <http://www.neii.gov.au/def/voc/waterprogram/water-regulations-2008-water-information-terms/subcategory-11b-water-information> ,
        <http://www.neii.gov.au/def/voc/waterprogram/water-regulations-2008-water-information-terms/subcategory-11c-water-information> ,
        <http://www.neii.gov.au/def/voc/waterprogram/water-regulations-2008-water-information-terms/subcategory-1a-water-information> ,
        <http://www.neii.gov.au/def/voc/waterprogram/water-regulations-2008-water-information-terms/subcategory-1b-water-information> ,
        <http://www.neii.gov.au/def/voc/waterprogram/water-regulations-2008-water-information-terms/subcategory-2a-water-information> ,
        <http://www.neii.gov.au/def/voc/waterprogram/water-regulations-2008-water-information-terms/subcategory-2b-water-information> ,
        <http://www.neii.gov.au/def/voc/waterprogram/water-regulations-2008-water-information-terms/subcategory-2d-water-information> ,
        <http://www.neii.gov.au/def/voc/waterprogram/water-regulations-2008-water-information-terms/subcategory-2e-water-information> ,
        <http://www.neii.gov.au/def/voc/waterprogram/water-regulations-2008-water-information-terms/subcategory-3a-water-information> ,
        <http://www.neii.gov.au/def/voc/waterprogram/water-regulations-2008-water-information-terms/subcategory-3b-water-information> ,
        <http://www.neii.gov.au/def/voc/waterprogram/water-regulations-2008-water-information-terms/subcategory-3c-water-information> ,
        <http://www.neii.gov.au/def/voc/waterprogram/water-regulations-2008-water-information-terms/subcategory-3d-water-information> ,
        <http://www.neii.gov.au/def/voc/waterprogram/water-regulations-2008-water-information-terms/subcategory-3da-water-information> ,
        <http://www.neii.gov.au/def/voc/waterprogram/water-regulations-2008-water-information-terms/subcategory-3e-water-information> ,
        <http://www.neii.gov.au/def/voc/waterprogram/water-regulations-2008-water-information-terms/subcategory-3f-water-information> ,
        <http://www.neii.gov.au/def/voc/waterprogram/water-regulations-2008-water-information-terms/subcategory-4a-water-information> ,
        <http://www.neii.gov.au/def/voc/waterprogram/water-regulations-2008-water-information-terms/subcategory-4b-water-information> ,
        <http://www.neii.gov.au/def/voc/waterprogram/water-regulations-2008-water-information-terms/subcategory-4c-water-information> ,
        <http://www.neii.gov.au/def/voc/waterprogram/water-regulations-2008-water-information-terms/subcategory-4d-water-information> ,
        <http://www.neii.gov.au/def/voc/waterprogram/water-regulations-2008-water-information-terms/subcategory-4e-water-information> ,
        <http://www.neii.gov.au/def/voc/waterprogram/water-regulations-2008-water-information-terms/subcategory-4f-water-information> ,
        <http://www.neii.gov.au/def/voc/waterprogram/water-regulations-2008-water-information-terms/subcategory-4g-water-information> ,
        <http://www.neii.gov.au/def/voc/waterprogram/water-regulations-2008-water-information-terms/subcategory-4h-water-information> ,
        <http://www.neii.gov.au/def/voc/waterprogram/water-regulations-2008-water-information-terms/subcategory-4i-water-information> ,
        <http://www.neii.gov.au/def/voc/waterprogram/water-regulations-2008-water-information-terms/subcategory-4j-water-information> ,
        <http://www.neii.gov.au/def/voc/waterprogram/water-regulations-2008-water-information-terms/subcategory-5a-water-information> ,
        <http://www.neii.gov.au/def/voc/waterprogram/water-regulations-2008-water-information-terms/subcategory-5b-water-information> ,
        <http://www.neii.gov.au/def/voc/waterprogram/water-regulations-2008-water-information-terms/subcategory-5c-water-information> ,
        <http://www.neii.gov.au/def/voc/waterprogram/water-regulations-2008-water-information-terms/subcategory-5d-water-information> ,
        <http://www.neii.gov.au/def/voc/waterprogram/water-regulations-2008-water-information-terms/subcategory-5e-water-information> ,
        <http://www.neii.gov.au/def/voc/waterprogram/water-regulations-2008-water-information-terms/subcategory-5f-water-information> ,
        <http://www.neii.gov.au/def/voc/waterprogram/water-regulations-2008-water-information-terms/subcategory-5g-water-information> ,
        <http://www.neii.gov.au/def/voc/waterprogram/water-regulations-2008-water-information-terms/subcategory-5h-water-information> ,
        <http://www.neii.gov.au/def/voc/waterprogram/water-regulations-2008-water-information-terms/subcategory-6a-water-information> ,
        <http://www.neii.gov.au/def/voc/waterprogram/water-regulations-2008-water-information-terms/subcategory-6b-water-information> ,
        <http://www.neii.gov.au/def/voc/waterprogram/water-regulations-2008-water-information-terms/subcategory-6c-water-information> ,
        <http://www.neii.gov.au/def/voc/waterprogram/water-regulations-2008-water-information-terms/subcategory-6d-water-information> ,
        <http://www.neii.gov.au/def/voc/waterprogram/water-regulations-2008-water-information-terms/subcategory-6e-water-information> ,
        <http://www.neii.gov.au/def/voc/waterprogram/water-regulations-2008-water-information-terms/subcategory-6f-water-information> ,
        <http://www.neii.gov.au/def/voc/waterprogram/water-regulations-2008-water-information-terms/subcategory-6g-water-information> ,
        <http://www.neii.gov.au/def/voc/waterprogram/water-regulations-2008-water-information-terms/subcategory-7a-water-information> ,
        <http://www.neii.gov.au/def/voc/waterprogram/water-regulations-2008-water-information-terms/subcategory-7b-water-information> ,
        <http://www.neii.gov.au/def/voc/waterprogram/water-regulations-2008-water-information-terms/subcategory-7c-water-information> ,
        <http://www.neii.gov.au/def/voc/waterprogram/water-regulations-2008-water-information-terms/subcategory-7d-water-information> ,
        <http://www.neii.gov.au/def/voc/waterprogram/water-regulations-2008-water-information-terms/subcategory-8a-water-information> ,
        <http://www.neii.gov.au/def/voc/waterprogram/water-regulations-2008-water-information-terms/subcategory-9a-water-information> ,
        <http://www.neii.gov.au/def/voc/waterprogram/water-regulations-2008-water-information-terms/subcategory-9b-water-information> ,
        <http://www.neii.gov.au/def/voc/waterprogram/water-regulations-2008-water-information-terms/subcategory-9c-water-information> ,
        <http://www.neii.gov.au/def/voc/waterprogram/water-regulations-2008-water-information-terms/subcategory-9d-water-information> ,
        <http://www.neii.gov.au/def/voc/waterprogram/water-regulations-2008-water-information-terms/subcategory-9e-water-information> ,
        <http://www.neii.gov.au/def/voc/waterprogram/water-regulations-2008-water-information-terms/subcategory-9f-water-information> ,
        <http://www.neii.gov.au/def/voc/waterprogram/water-regulations-2008-water-information-terms/subcategory-9g-water-information> ,
        <http://www.neii.gov.au/def/voc/waterprogram/water-regulations-2008-water-information-terms/subcategory-9ga-water-information> ,
        <http://www.neii.gov.au/def/voc/waterprogram/water-regulations-2008-water-information-terms/subcategory-9h-water-information> ,
        <http://www.neii.gov.au/def/voc/waterprogram/water-regulations-2008-water-information-terms/surface-water> ,
        <http://www.neii.gov.au/def/voc/waterprogram/water-regulations-2008-water-information-terms/take> ,
        <http://www.neii.gov.au/def/voc/waterprogram/water-regulations-2008-water-information-terms/tidal-limit> ,
        <http://www.neii.gov.au/def/voc/waterprogram/water-regulations-2008-water-information-terms/total-nitrogen-concentration> ,
        <http://www.neii.gov.au/def/voc/waterprogram/water-regulations-2008-water-information-terms/total-phosphorus-concentration> ,
        <http://www.neii.gov.au/def/voc/waterprogram/water-regulations-2008-water-information-terms/total-suspended-solids> ,
        <http://www.neii.gov.au/def/voc/waterprogram/water-regulations-2008-water-information-terms/transfer-party> ,
        <http://www.neii.gov.au/def/voc/waterprogram/water-regulations-2008-water-information-terms/turbidity> ,
        <http://www.neii.gov.au/def/voc/waterprogram/water-regulations-2008-water-information-terms/upward-longwave-exposure> ,
        <http://www.neii.gov.au/def/voc/waterprogram/water-regulations-2008-water-information-terms/upward-longwave-irradiance> ,
        <http://www.neii.gov.au/def/voc/waterprogram/water-regulations-2008-water-information-terms/urban-recycled-water-information> ,
        <http://www.neii.gov.au/def/voc/waterprogram/water-regulations-2008-water-information-terms/urban-stormwater-information> ,
        <http://www.neii.gov.au/def/voc/waterprogram/water-regulations-2008-water-information-terms/urban-wastewater-information> ,
        <http://www.neii.gov.au/def/voc/waterprogram/water-regulations-2008-water-information-terms/urban-water-supply-information> ,
        <http://www.neii.gov.au/def/voc/waterprogram/water-regulations-2008-water-information-terms/vapour-pressure-deficit> ,
        <http://www.neii.gov.au/def/voc/waterprogram/water-regulations-2008-water-information-terms/wastewater-treatment-plant-WWTP> ,
        <http://www.neii.gov.au/def/voc/waterprogram/water-regulations-2008-water-information-terms/water-connection> ,
        <http://www.neii.gov.au/def/voc/waterprogram/water-regulations-2008-water-information-terms/water-equivalent-precipitation> ,
        <http://www.neii.gov.au/def/voc/waterprogram/water-regulations-2008-water-information-terms/water-information> ,
        <http://www.neii.gov.au/def/voc/waterprogram/water-regulations-2008-water-information-terms/water-management-area> ,
        <http://www.neii.gov.au/def/voc/waterprogram/water-regulations-2008-water-information-terms/water-reclamation-plant-WRP> ,
        <http://www.neii.gov.au/def/voc/waterprogram/water-regulations-2008-water-information-terms/water-storage> ,
        <http://www.neii.gov.au/def/voc/waterprogram/water-regulations-2008-water-information-terms/water-treatment-plant-WTP> ,
        <http://www.neii.gov.au/def/voc/waterprogram/water-regulations-2008-water-information-terms/watercourse> ,
        <http://www.neii.gov.au/def/voc/waterprogram/water-regulations-2008-water-information-terms/web-service> ,
        <http://www.neii.gov.au/def/voc/waterprogram/water-regulations-2008-water-information-terms/week> ,
        <http://www.neii.gov.au/def/voc/waterprogram/water-regulations-2008-water-information-terms/wet-bulb-air-temperature> ,
        <http://www.neii.gov.au/def/voc/waterprogram/water-regulations-2008-water-information-terms/wind-run> ,
        <http://www.neii.gov.au/def/voc/waterprogram/water-regulations-2008-water-information-terms/year> ;
.

<https://linked.data.gov.au/org/neii>
    a
        dcterms:Agent ,
        schema:Organization ;
    foaf:homepage "http://www.bom.gov.au/environment/transition.shtml"^^xsd:anyURI ;
    foaf:name "NEII" ;
.
