PREFIX : <https://linked.data.gov.au/def/australian-network-of-hydrologic-reference-stations-glossary/>
PREFIX cs: <https://linked.data.gov.au/def/australian-network-of-hydrologic-reference-stations-glossary>
PREFIX dcterms: <http://purl.org/dc/terms/>
PREFIX owl: <http://www.w3.org/2002/07/owl#>
PREFIX schema: <https://schema.org/>
PREFIX skos: <http://www.w3.org/2004/02/skos/core#>
PREFIX xsd: <http://www.w3.org/2001/XMLSchema#>

:Annual-Average
    a skos:Concept ;
    dcterms:created "2020-08-27"^^xsd:date ;
    dcterms:creator <https://linked.data.gov.au/org/neii> ;
    skos:definition "Average of the annual total streamflow volumes (within each water year) over the stated period of record."@en ;
    skos:inScheme cs: ;
    skos:prefLabel "Annual Average"@en ;
    skos:topConceptOf cs: ;
.

:Annual-Baseflow
    a skos:Concept ;
    dcterms:created "2020-08-27"^^xsd:date ;
    dcterms:creator <https://linked.data.gov.au/org/neii> ;
    skos:definition "The component of streamflow supplied by groundwater discharge in a water year."@en ;
    skos:inScheme cs: ;
    skos:prefLabel "Annual Baseflow"@en ;
    skos:topConceptOf cs: ;
.

:Annual-Total
    a skos:Concept ;
    dcterms:created "2020-08-27"^^xsd:date ;
    dcterms:creator <https://linked.data.gov.au/org/neii> ;
    skos:definition "Total streamflow volume per water year."@en ;
    skos:inScheme cs: ;
    skos:prefLabel "Annual Total"@en ;
    skos:topConceptOf cs: ;
.

:Anomaly
    a skos:Concept ;
    dcterms:created "2020-08-27"^^xsd:date ;
    dcterms:creator <https://linked.data.gov.au/org/neii> ;
    skos:definition "The deviation of a measurable unit, (e.g., streamflow or precipitation) from the long-term average in each station or region over a specified period."@en ;
    skos:inScheme cs: ;
    skos:prefLabel "Anomaly"@en ;
    skos:topConceptOf cs: ;
.

:Area
    a skos:Concept ;
    dcterms:created "2020-08-27"^^xsd:date ;
    dcterms:creator <https://linked.data.gov.au/org/neii> ;
    skos:definition "The catchment area derived from the Australian Hydrological Geospatial Fabric catchments (including contributing overland flow and internally draining areas)."@en ;
    skos:inScheme cs: ;
    skos:prefLabel "Area"@en ;
    skos:topConceptOf cs: ;
.

:Cease-to-flow
    a skos:Concept ;
    dcterms:created "2020-08-27"^^xsd:date ;
    dcterms:creator <https://linked.data.gov.au/org/neii> ;
    skos:definition "The level at which a stream stops flowing. The lowest point in the low flow control."@en ;
    skos:inScheme cs: ;
    skos:prefLabel "Cease to flow"@en ;
    skos:topConceptOf cs: ;
.

:Daily-Q10
    a skos:Concept ;
    dcterms:created "2020-08-27"^^xsd:date ;
    dcterms:creator <https://linked.data.gov.au/org/neii> ;
    skos:definition "10 Percent of the time, the daily streamflow is below the Q10 value in each water year."@en ;
    skos:inScheme cs: ;
    skos:prefLabel "Daily Q10"@en ;
    skos:topConceptOf cs: ;
.

:Daily-Q50
    a skos:Concept ;
    dcterms:created "2020-08-27"^^xsd:date ;
    dcterms:creator <https://linked.data.gov.au/org/neii> ;
    skos:definition "50 Percent of the time, the daily streamflow is below the Q50 value in each water year."@en ;
    skos:inScheme cs: ;
    skos:prefLabel "Daily Q50"@en ;
    skos:topConceptOf cs: ;
.

:Daily-Q90
    a skos:Concept ;
    dcterms:created "2020-08-27"^^xsd:date ;
    dcterms:creator <https://linked.data.gov.au/org/neii> ;
    skos:definition "90 Percent of the time, the daily streamflow is below the Q90 value in each water year."@en ;
    skos:inScheme cs: ;
    skos:prefLabel "Daily Q90"@en ;
    skos:topConceptOf cs: ;
.

:Event-Analysis
    a skos:Concept ;
    dcterms:created "2020-08-27"^^xsd:date ;
    dcterms:creator <https://linked.data.gov.au/org/neii> ;
    skos:definition "Histograms showing the frequency and magnitude (volume) of events."@en ;
    skos:inScheme cs: ;
    skos:prefLabel "Event Analysis"@en ;
    skos:topConceptOf cs: ;
.

:Flow-Duration-Curve
    a skos:Concept ;
    dcterms:created "2020-08-27"^^xsd:date ;
    dcterms:creator <https://linked.data.gov.au/org/neii> ;
    skos:definition "A curve showing percentage of time streamflow magnitude exceeds certain value."@en ;
    skos:inScheme cs: ;
    skos:prefLabel "Flow Duration Curve"@en ;
    skos:topConceptOf cs: ;
.

:Hydrologic-Reference-Station
    a skos:Concept ;
    dcterms:created "2020-08-27"^^xsd:date ;
    dcterms:creator <https://linked.data.gov.au/org/neii> ;
    skos:definition "A hydrologic reference station is located in an unregulated catchment with minimal land-use change upstream. It has a high-quality long streamflow record with a frequently verified rating table. The gauge has been well maintained. See theStation Selection Guidelinespage (http://www.bom.gov.au/water/hrs/guidelines.shtml) for more information."@en ;
    skos:inScheme cs: ;
    skos:prefLabel "Hydrologic Reference Station"@en ;
    skos:topConceptOf cs: ;
.

:Long-term-streamflow-trend
    a skos:Concept ;
    dcterms:created "2020-08-27"^^xsd:date ;
    dcterms:creator <https://linked.data.gov.au/org/neii> ;
    skos:definition "A unidirectional change in the magnitude of the streamflow variable. The trend may be increasing or decreasing."@en ;
    skos:inScheme cs: ;
    skos:prefLabel "Long-term streamflow trend"@en ;
    skos:topConceptOf cs: ;
.

:Longest-Stream-Length
    a skos:Concept ;
    dcterms:created "2020-08-27"^^xsd:date ;
    dcterms:creator <https://linked.data.gov.au/org/neii> ;
    skos:definition "The length of the longest stream within the catchment of Hydrologic Reference station derived from the contributing streams from the Australian Hydrological Geospatial Fabric MappedStream features."@en ;
    skos:inScheme cs: ;
    skos:prefLabel "Longest Stream Length"@en ;
    skos:topConceptOf cs: ;
.

:Max-Elevation
    a skos:Concept ;
    dcterms:created "2020-08-27"^^xsd:date ;
    dcterms:creator <https://linked.data.gov.au/org/neii> ;
    skos:definition "Maximum elevation within the Australian Hydrological Geospatial Fabric derived catchment boundaries"@en ;
    skos:inScheme cs: ;
    skos:prefLabel "Max Elevation"@en ;
    skos:topConceptOf cs: ;
.

:Min-Elevation
    a skos:Concept ;
    dcterms:created "2020-08-27"^^xsd:date ;
    dcterms:creator <https://linked.data.gov.au/org/neii> ;
    skos:definition "Minimum elevation within the Australian Hydrological Geospatial Fabric derived catchment boundaries"@en ;
    skos:inScheme cs: ;
    skos:prefLabel "Min Elevation"@en ;
    skos:topConceptOf cs: ;
.

:Runoff-Rate
    a skos:Concept ;
    dcterms:created "2020-08-27"^^xsd:date ;
    dcterms:creator <https://linked.data.gov.au/org/neii> ;
    skos:definition "The percentage of rainfall volume that becomes streamflow after losses such as evaporation within the catchment."@en ;
    skos:inScheme cs: ;
    skos:prefLabel "Runoff Rate"@en ;
    skos:topConceptOf cs: ;
.

:WISKI
    a skos:Concept ;
    dcterms:created "2020-08-27"^^xsd:date ;
    dcterms:creator <https://linked.data.gov.au/org/neii> ;
    skos:definition "Water Information System Kisters (WISKI) contains Watercourse level and discharge time-series data and ratings collected from approximately 3500 measurement stations across Australia. This data can be accessed via Water Data Online http://www.bom.gov.au/waterdata/. Except for Victoria, all discharge data are directly uploaded from the water agencies. For Victoria, the rating tables in WISKI are used to compute discharge from the water levels at the time-step provided by the agencies. The discharge data are then accumulated to a daily total at 9am for the previous 24 hours."@en ;
    skos:inScheme cs: ;
    skos:prefLabel "WISKI"@en ;
    skos:topConceptOf cs: ;
.

:Water-Year
    a skos:Concept ;
    dcterms:created "2020-08-27"^^xsd:date ;
    dcterms:creator <https://linked.data.gov.au/org/neii> ;
    skos:definition "The Water Year begins with the month recording minimum average monthly flow over the period of the data. If the beginning month is a month from January to June, the nominal year of the Water Year is the same as the calendar year of the beginning month. For months July to December, the nominal year is the year following the calendar year of the beginning month. For example, a water year starting in July 1997 is nominally Water Year 1998. However, in a few cases it was necessary to modify the definition so that the definition was consistent within each river basin. In Australian Water Information Dictionary (AWID) Water Year is defined as first of July to 30th June."@en ;
    skos:inScheme cs: ;
    skos:prefLabel "Water Year"@en ;
    skos:topConceptOf cs: ;
.

<https://linked.data.gov.au/org/neii>
    a
        dcterms:Agent ,
        schema:Organization ;
    schema:name "National Environmental Information Infrastructure" ;
    schema:url "http://www.bom.gov.au/environment/transition.shtml"^^xsd:anyURI ;
.

cs:
    a skos:ConceptScheme ;
    dcterms:created "2020-08-27"^^xsd:date ;
    dcterms:creator <https://linked.data.gov.au/org/neii> ;
    dcterms:issued "2020-08-27" ;
    dcterms:modified "2024-04-15"^^xsd:date ;
    dcterms:publisher <https://linked.data.gov.au/org/neii> ;
    owl:versionInfo "Version 1" ;
    skos:definition "This glossary defines the key terms used on the Australian Network of Hydrologic Reference Stations portal."@en ;
    skos:hasTopConcept
        :Annual-Average ,
        :Annual-Baseflow ,
        :Annual-Total ,
        :Anomaly ,
        :Area ,
        :Cease-to-flow ,
        :Daily-Q10 ,
        :Daily-Q50 ,
        :Daily-Q90 ,
        :Event-Analysis ,
        :Flow-Duration-Curve ,
        :Hydrologic-Reference-Station ,
        :Long-term-streamflow-trend ,
        :Longest-Stream-Length ,
        :Max-Elevation ,
        :Min-Elevation ,
        :Runoff-Rate ,
        :WISKI ,
        :Water-Year ;
    skos:historyNote "2024-04: IRIs changed from http://www.neii.gov.au/def/voc/EPS/australian-network-of-hydrologic-reference-stations-glossary/Australian-Network-of-Hydrologic-Reference-Stations-glossary for the ConceptScheme and http://www.neii.gov.au/def/voc/EPS/australian-network-of-hydrologic-reference-stations-glossary/ for the Concept namespace to linked.data.gov.au-based IRIs" ;
    skos:prefLabel "Australian Network of Hydrologic Reference Stations glossary"@en ;
.
