PREFIX : <https://linked.data.gov.au/def/Bioregional-Assessment-Programme-Glossary/>
PREFIX cs: <https://linked.data.gov.au/def/Bioregional-Assessment-Programme-Glossary>
PREFIX dcterms: <http://purl.org/dc/terms/>
PREFIX owl: <http://www.w3.org/2002/07/owl#>
PREFIX rdf: <http://www.w3.org/1999/02/22-rdf-syntax-ns#>
PREFIX rdfs: <http://www.w3.org/2000/01/rdf-schema#>
PREFIX schema: <https://schema.org/>
PREFIX skos: <http://www.w3.org/2004/02/skos/core#>
PREFIX xsd: <http://www.w3.org/2001/XMLSchema#>

skos:related
    a
        rdf:Property ,
        rdfs:Resource ;
    rdfs:subPropertyOf skos:related ;
.

:BA-metadata-quality-assurance-process
    a skos:Concept ;
    dcterms:created "2019-04-14"^^xsd:date ;
    dcterms:creator <https://linked.data.gov.au/org/neii> ;
    skos:definition "a mechanism by which the Bioregional Assessment Programme quality assures metadata statements to ensure they are fit for purpose and of sufficient quality to be made publicly available"@en ;
    skos:inScheme cs: ;
    skos:prefLabel "BA metadata quality assurance process"@en ;
    skos:topConceptOf cs: ;
.

:BADMS-compliant-metadata
    a skos:Concept ;
    dcterms:created "2019-04-14"^^xsd:date ;
    dcterms:creator <https://linked.data.gov.au/org/neii> ;
    dcterms:modified "2020-09-28"^^xsd:date ;
    skos:definition "a subset of the mandatory ANZLIC Metadata profile elements that have been selected as the minimum requirement for metadata in the Bioregional Assessment Programme"@en ;
    skos:inScheme cs: ;
    skos:prefLabel "BADMS-compliant metadata"@en ;
    skos:topConceptOf cs: ;
.

:Bioregional-Assessment-Data-Store
    a skos:Concept ;
    dcterms:created "2019-04-14"^^xsd:date ;
    dcterms:creator <https://linked.data.gov.au/org/neii> ;
    dcterms:modified "2020-09-28"^^xsd:date ;
    skos:altLabel "Data Store"@en ;
    skos:definition "the component of the Bioregional Assessment Repository dedicated to storing datasets, maps and products"@en ;
    skos:inScheme cs: ;
    skos:prefLabel "Bioregional Assessment Data Store"@en ;
    skos:topConceptOf cs: ;
.

:Bioregional-Assessment-Metadata-Catalogue
    a skos:Concept ;
    dcterms:created "2019-04-14"^^xsd:date ;
    dcterms:creator <https://linked.data.gov.au/org/neii> ;
    dcterms:modified "2020-09-28"^^xsd:date ;
    skos:altLabel "Metadata Catalogue"@en ;
    skos:definition "the component of the Bioregional Assessment Repository dedicated to storing metadata"@en ;
    skos:inScheme cs: ;
    skos:prefLabel "Bioregional Assessment Metadata Catalogue"@en ;
    skos:topConceptOf cs: ;
.

:Bioregional-Assessment-Repository
    a skos:Concept ;
    dcterms:created "2019-04-14"^^xsd:date ;
    dcterms:creator <https://linked.data.gov.au/org/neii> ;
    dcterms:modified "2020-09-28"^^xsd:date ;
    skos:altLabel "Repository"@en ;
    skos:definition "a collection of systems that together store source and derived datasets, products and maps, accompanying metadata, lineage and supporting material. It consists of the Data Store, Metadata Catalogue and the Repository website. The Repository is not available to the public."@en ;
    skos:inScheme cs: ;
    skos:prefLabel "Bioregional Assessment Repository"@en ;
    skos:topConceptOf cs: ;
.

:Clarence-Moreton-bioregion
    a skos:Concept ;
    dcterms:created "2019-04-14"^^xsd:date ;
    dcterms:creator <https://linked.data.gov.au/org/neii> ;
    skos:definition "The Clarence-Moreton bioregion is located in north-east NSW and south-east Queensland and adjoins the Northern Inland Catchments bioregion. Along with the towns of Casino, Lismore and Grafton, it contains the outskirts of the Queensland cities of Brisbane, Ipswich, Logan and Toowoomba. The bioregion contains large river systems (including the Clarence, Richmond and Logan-Albert rivers) and extensive wetlands, some of which are nationally important. Many of these wetlands are home to water-dependent plants and animals that are listed as rare or threatened under Queensland and Commonwealth legislation. The bioregion contains numerous national parks and forest reserves and includes sites of international importance for bird conservation. A large area of the bioregion is used for dryland farming and plantations and as grazing land for livestock. Irrigated agriculture takes up a comparatively small area. Groundwater is extracted for various uses but most commonly for livestock and agricultural purposes. The largest water reservoir in this bioregion is Lake Wivenhoe on the Brisbane River, which supplies Brisbane and its surrounds. The NSW part of the bioregion has smaller dams located in the upper Richmond river basin."@en ;
    skos:inScheme cs: ;
    skos:prefLabel "Clarence-Moreton bioregion"@en ;
    skos:topConceptOf cs: ;
.

:Element-Conformance-Report
    a skos:Concept ;
    dcterms:created "2019-04-14"^^xsd:date ;
    dcterms:creator <https://linked.data.gov.au/org/neii> ;
    skos:definition "output of the tool that checks that all datasets used to create non-text elements in a technical product such as maps, tables, and graphs, as well as image files associated with these non-text elements, are correctly registered in the Bioregional Assessment Repository."@en ;
    skos:inScheme cs: ;
    skos:prefLabel "Element Conformance Report"@en ;
    skos:topConceptOf cs: ;
.

:Ferrosols
    a skos:Concept ;
    dcterms:created "2019-04-14"^^xsd:date ;
    dcterms:creator <https://linked.data.gov.au/org/neii> ;
    dcterms:modified "2020-09-29"^^xsd:date ;
    skos:definition "Soils other than Vertosols, Hydrosols, and Calcarosols that: i. Have B2 horizons in which the major part has a free iron oxide1 content greater  than 5% Fe in the fine earth fraction (<2 mm), and ii. Do not have  clear or abrupt textural B horizons or a B2 horizon in which at least 0.3m has vertic properties."@en ;
    skos:inScheme cs: ;
    skos:prefLabel "Ferrosols"@en ;
    skos:topConceptOf cs: ;
.

:Geofabric
    a skos:Concept ;
    dcterms:created "2019-04-14"^^xsd:date ;
    dcterms:creator <https://linked.data.gov.au/org/neii> ;
    skos:definition "a nationally consistent series of interrelated spatial datasets defining hierarchically-nested river basins, stream segments, hydrological networks and associated cartography"@en ;
    skos:inScheme cs: ;
    skos:prefLabel "Geofabric"@en ;
    skos:topConceptOf cs: ;
.

:Impact-Modes-and-Effects-Analysis
    a skos:Concept ;
    dcterms:created "2019-04-14"^^xsd:date ;
    dcterms:creator <https://linked.data.gov.au/org/neii> ;
    dcterms:modified "2020-09-29"^^xsd:date ;
    skos:altLabel "IMEA"@en ;
    skos:definition "a systematic hazard identification and prioritisation technique based on Failure Modes and Effects Analysis"@en ;
    skos:inScheme cs: ;
    skos:prefLabel "Impact Modes and Effects Analysis"@en ;
    skos:topConceptOf cs: ;
.

:Joint-Ore-Reserves-Committee-Code
    a skos:Concept ;
    dcterms:created "2019-04-14"^^xsd:date ;
    dcterms:creator <https://linked.data.gov.au/org/neii> ;
    skos:definition "the Australasian professional code of practice that sets minimum standards for the public reporting of mineral exploration results, mineral resources and ore reserves (including coal)"@en ;
    skos:inScheme cs: ;
    skos:prefLabel "Joint Ore Reserves Committee Code"@en ;
    skos:topConceptOf cs: ;
.

:Kurosols
    a skos:Concept ;
    dcterms:created "2019-04-14"^^xsd:date ;
    dcterms:creator <https://linked.data.gov.au/org/neii> ;
    dcterms:modified "2020-09-29"^^xsd:date ;
    skos:definition "Soils other than Hydrosols with a clear or abrupt textural B horizon and in  which the major part of the upper 0.2 m of the B2 horizon (or the major part of the entire B2 horizon if it is less than 0.2 m thick) is strongly acid."@en ;
    skos:inScheme cs: ;
    skos:prefLabel "Kurosols"@en ;
    skos:topConceptOf cs: ;
.

:Markov-chain-Monte-Carlo-methods
    a skos:Concept ;
    dcterms:created "2019-04-14"^^xsd:date ;
    dcterms:creator <https://linked.data.gov.au/org/neii> ;
    dcterms:modified "2020-09-29"^^xsd:date ;
    skos:altLabel
        "MCMC"@en ,
        "Markov chain Monte Carlo sampling"@en ;
    skos:definition "a class of algorithms for sampling from a probability distribution based on constructing a Markov chain that has the desired distribution as its equilibrium distribution. The state of the chain after a number of steps is then used as a sample of the desired distribution. The quality of the sample improves as a function of the number of steps."@en ;
    skos:inScheme cs: ;
    skos:prefLabel "Markov chain Monte Carlo methods"@en ;
    skos:topConceptOf cs: ;
.

:Metadata-Record-Coordinator
    a skos:Concept ;
    dcterms:created "2019-04-14"^^xsd:date ;
    dcterms:creator <https://linked.data.gov.au/org/neii> ;
    skos:definition "the person, usually a Data Coordinator, adding the metadata record and responsible for assigning a metadata record owner"@en ;
    skos:inScheme cs: ;
    skos:prefLabel "Metadata Record Coordinator"@en ;
    skos:topConceptOf cs: ;
.

:Monte-Carlo-simulation
    a skos:Concept ;
    dcterms:created "2019-04-14"^^xsd:date ;
    dcterms:creator <https://linked.data.gov.au/org/neii> ;
    skos:definition "a simulation technique involving random sampling of each probability distribution within the model to produce large number of plausible scenarios. Each probability distribution is sampled in a manner that reproduces the distribution's shape. The distribution of the values calculated for the model outcome therefore reflects the probability of the values that could occur."@en ;
    skos:inScheme cs: ;
    skos:prefLabel "Monte Carlo simulation"@en ;
    skos:topConceptOf cs: ;
.

:R0.2
    a skos:Concept ;
    dcterms:created "2019-04-14"^^xsd:date ;
    dcterms:creator <https://linked.data.gov.au/org/neii> ;
    skos:definition "the peak daily flow in flood events with a return period of 0.2 years as defined from modelled baseline flow in the reference period (1983 to 2012)"@en ;
    skos:inScheme cs: ;
    skos:prefLabel "R0.2"@en ;
    skos:topConceptOf cs: ;
.

:R0.3
    a skos:Concept ;
    dcterms:created "2019-04-14"^^xsd:date ;
    dcterms:creator <https://linked.data.gov.au/org/neii> ;
    skos:definition "the peak daily flow in flood events with a return period of 0.3 years as defined from modelled baseline flow in the reference period (1983 to 2012)"@en ;
    skos:inScheme cs: ;
    skos:prefLabel "R0.3"@en ;
    skos:topConceptOf cs: ;
.

:R2.0
    a skos:Concept ;
    dcterms:created "2019-04-14"^^xsd:date ;
    dcterms:creator <https://linked.data.gov.au/org/neii> ;
    skos:definition "the peak daily flow in flood events with a return period of 2.0 years as defined from modelled baseline flow in the reference period (1983 to 2012)"@en ;
    skos:inScheme cs: ;
    skos:prefLabel "R2.0"@en ;
    skos:topConceptOf cs: ;
.

:R3.0
    a skos:Concept ;
    dcterms:created "2019-04-14"^^xsd:date ;
    dcterms:creator <https://linked.data.gov.au/org/neii> ;
    skos:definition "the peak daily flow in flood events with a return period of 3.0 years as defined from modelled baseline flow in the reference period (1983 to 2012)"@en ;
    skos:inScheme cs: ;
    skos:prefLabel "R3.0"@en ;
    skos:topConceptOf cs: ;
.

:Repository-website
    a skos:Concept ;
    dcterms:created "2019-04-14"^^xsd:date ;
    dcterms:creator <https://linked.data.gov.au/org/neii> ;
    skos:definition "the component of the Bioregional Assessment Repository that is the web-based front-end to access and use its systems. The Repository website is not available to the public."@en ;
    skos:inScheme cs: ;
    skos:prefLabel "Repository website"@en ;
    skos:topConceptOf cs: ;
.

:Rudosols
    a skos:Concept ;
    dcterms:created "2019-04-14"^^xsd:date ;
    dcterms:creator <https://linked.data.gov.au/org/neii> ;
    skos:definition "Soil with negligible (rudimentary) pedologic organisation apart from (a) minimal development of an Al horizon or (b) the presence of less than 10% of B horizon material (including pedogenic carbonate) in fissures in the parent rock or saprolite. The soils are apedal or only weakly structured in the A1 horizon and show no pedological colour changes apart from the darkening of an A1 horizon. There is little or no texture or colour change with depth unless stratified or buried soils are present."@en ;
    skos:inScheme cs: ;
    skos:prefLabel "Rudosols"@en ;
    skos:topConceptOf cs: ;
.

:Sodosols
    a skos:Concept ;
    dcterms:created "2019-04-14"^^xsd:date ;
    dcterms:creator <https://linked.data.gov.au/org/neii> ;
    dcterms:modified "2020-09-29"^^xsd:date ;
    skos:definition "Soils with a clear or abrupt textural B horizon and in which the major part of the upper 0.2m of the B2 horizon (or the major part of the entire B2 horizon if it is less than 0.2m thick) is sodic and not strongly acid. Hydrosols and soils with strongly subplastic upper B2 horizons are excluded."@en ;
    skos:inScheme cs: ;
    skos:prefLabel "Sodosols"@en ;
    skos:topConceptOf cs: ;
.

:Tenosols
    a skos:Concept ;
    dcterms:created "2019-04-14"^^xsd:date ;
    dcterms:creator <https://linked.data.gov.au/org/neii> ;
    dcterms:modified "2020-09-29"^^xsd:date ;
    skos:definition "Soils that do not fit the requirements of any other soil orders and generally with one or more of the following: i. A peaty horizon. ii. A humose, melacic or melanic horizon, or conspicuously bleached A2 horizon, which overlies a calcrete pan, hard unweathered rock or other hard materials; or partially weathered or decomposed rock or saprolite, or unconsolidated mineral materials. iii. A horizons which meet all the conditions for a peaty, humose, melacic or melanic horizon except the depth requirement, and directly overlie a calcrete pan, hard unweathered rock or other hard materials; or partially weathered or decomposed rock or saprolite, or unconsolidated mineral materials. iv. A1 horizons which have more than a weak development of structure and directly overlie a calcrete pan, hard unweathered rock or other hard materials; or partially weathered or decomposed rock or saprolite, or unconsolidated mineral materials. v. An A2 horizon which overlies a calcrete pan, hard unweathered rock or other hard materials; or partially weathered or decomposed rock or saprolite, or unconsolidated mineral materials. vi. Either a tenic B horizon, or a B2 horizon with 15% clay (SL) or less1, or a transitional horizon (C/B) occurring in fissures in the parent rock or saprolite which contains between 10 and 50% of B horizon material (including pedogenic carbonate). vii. A ferric or bauxitic horizon 0.2 m thick. viii. A calcareous horizon 0.2 m thick."@en ;
    skos:inScheme cs: ;
    skos:prefLabel "Tenosols"@en ;
    skos:topConceptOf cs: ;
.

:Vertosols
    a skos:Concept ;
    dcterms:created "2019-04-14"^^xsd:date ;
    dcterms:creator <https://linked.data.gov.au/org/neii> ;
    dcterms:modified "2020-09-29"^^xsd:date ;
    skos:definition "Soils with the following: i. A clay field texture or 35% or more clay throughout the solum except for thin, surface crusty horizons 0.03 m or less thick and ii. When dry, open cracks occur at some time in most years1. These are at least 5 mm wide and extend upward to the surface or to the base of any plough layer, self-mulching horizon, or thin, surface crusty horizon; and iii. Slickensides and/or lenticular peds occur at some depth in the solum. 1 Note that there is no crack frequency criterion as in the Factual Key."@en ;
    skos:inScheme cs: ;
    skos:prefLabel "Vertosols"@en ;
    skos:topConceptOf cs: ;
.

:activity
    a skos:Concept ;
    dcterms:created "2019-04-14"^^xsd:date ;
    dcterms:creator <https://linked.data.gov.au/org/neii> ;
    dcterms:modified "2020-09-28"^^xsd:date ;
    skos:altLabel "activities"@en ;
    skos:definition "for the purposes of Impact Modes and Effects Analysis (IMEA), a planned event associated with a coal seam gas (CSG) operation or coal mine. For example, activities during the production life-cycle stage in a CSG operation include drilling and coring, ground-based geophysics and surface core testing. Activities are grouped into components, which are grouped into life-cycle stages."@en ;
    skos:inScheme cs: ;
    skos:prefLabel "activity"@en ;
    skos:topConceptOf cs: ;
.

:additional-coal-resource-development
    a skos:Concept ;
    dcterms:created "2019-04-14"^^xsd:date ;
    dcterms:creator <https://linked.data.gov.au/org/neii> ;
    dcterms:modified "2020-09-28"^^xsd:date ;
    skos:altLabel "ACRD"@en ;
    skos:definition "all coal mines and coal seam gas (CSG) fields, including expansions of baseline operations, that are expected to begin commercial production after December 2012"@en ;
    skos:inScheme cs: ;
    skos:prefLabel "additional coal resource development"@en ;
    skos:topConceptOf cs: ;
.

:advanced-exploration
    a skos:Concept ;
    dcterms:created "2019-04-14"^^xsd:date ;
    dcterms:creator <https://linked.data.gov.au/org/neii> ;
    dcterms:modified "2020-09-28"^^xsd:date ;
    skos:definition "a stage in the exploration process whereby the particular commodity of interest (such  as coal) is known to exist within the exploration tenement, based on analysis of existing data and information, combined with new data obtained from drilling of boreholes, sampling and analyses of rock types, and other relevant geoscientific studies, etc."@en ;
    skos:inScheme cs: ;
    skos:prefLabel "advanced exploration"@en ;
    skos:topConceptOf cs: ;
.

:amax
    a skos:Concept ;
    dcterms:created "2019-04-14"^^xsd:date ;
    dcterms:creator <https://linked.data.gov.au/org/neii> ;
    skos:definition "maximum raw change"@en ;
    skos:inScheme cs: ;
    skos:prefLabel "amax"@en ;
    skos:topConceptOf cs: ;
.

:analysis-domain-extent
    a skos:Concept ;
    dcterms:created "2019-04-14"^^xsd:date ;
    dcterms:creator <https://linked.data.gov.au/org/neii> ;
    skos:definition "the geographic area used for geoprocessing and data preparation purposes that encompasses the analysis extent plus additional areas sufficient to ensure all relevant data are included for the impact analysis of a bioregional assessment (BA)"@en ;
    skos:inScheme cs: ;
    skos:prefLabel "analysis domain extent"@en ;
    skos:topConceptOf cs: ;
.

:analysis-extent
    a skos:Concept ;
    dcterms:created "2019-04-14"^^xsd:date ;
    dcterms:creator <https://linked.data.gov.au/org/neii> ;
    skos:definition "the geographic area that encompasses all the possible areas that may be reported in the impact analysis of a bioregional assessment (BA), typically including the bioregion or subregion, the preliminary assessment extent (PAE) and the relevant groundwater and surface water model domains"@en ;
    skos:inScheme cs: ;
    skos:prefLabel "analysis extent"@en ;
    skos:topConceptOf cs: ;
.

:analytic-element-model
    a skos:Concept ;
    dcterms:created "2019-04-14"^^xsd:date ;
    dcterms:creator <https://linked.data.gov.au/org/neii> ;
    dcterms:modified "2020-09-28"^^xsd:date ;
    skos:altLabel "AEM"@en ;
    skos:definition "a groundwater model in which the groundwater flow equations are solved based on the representation of internal boundary conditions, points, lines or polygons where constant groundwater level, constant flux or flux dependence on groundwater level is imposed (Bakker, 2013). The resulting groundwater flow equations can be evaluated at arbitrary points in space and time. The solution is therefore independent of a spatial discretisation of the model domain into grids, and a temporal discretisation into time steps, as is necessary for finite element or finite difference groundwater models."@en ;
    skos:inScheme cs: ;
    skos:prefLabel "analytic element model"@en ;
    skos:topConceptOf cs: ;
.

:aquifer
    a skos:Concept ;
    dcterms:created "2019-04-14"^^xsd:date ;
    dcterms:creator <https://linked.data.gov.au/org/neii> ;
    skos:definition "rock or sediment in a formation, group of formations, or part of a formation that is saturated and sufficiently permeable to transmit quantities of water to bores and springs"@en ;
    skos:inScheme cs: ;
    skos:prefLabel "aquifer"@en ;
    skos:topConceptOf cs: ;
.

:aquitard
    a skos:Concept ;
    dcterms:created "2019-04-14"^^xsd:date ;
    dcterms:creator <https://linked.data.gov.au/org/neii> ;
    skos:definition "a saturated geological unit that is less permeable than an aquifer, and incapable of transmitting useful quantities of water. Aquitards often form a confining layer over an artesian aquifer."@en ;
    skos:inScheme cs: ;
    skos:prefLabel "aquitard"@en ;
    skos:topConceptOf cs: ;
.

:artesian-aquifer
    a skos:Concept ;
    dcterms:created "2019-04-14"^^xsd:date ;
    dcterms:creator <https://linked.data.gov.au/org/neii> ;
    skos:definition "an aquifer that has enough natural pressure to allow water in a bore to rise to the ground surface"@en ;
    skos:inScheme cs: ;
    skos:prefLabel "artesian aquifer"@en ;
    skos:topConceptOf cs: ;
.

:asset-identifier
    a skos:Concept ;
    dcterms:created "2019-04-14"^^xsd:date ;
    dcterms:creator <https://linked.data.gov.au/org/neii> ;
    skos:definition "the bioregional assessment (BA) asset identifier (sequential and unique per asset across all assets in the Bioregional Assessment Technical Programme)"@en ;
    skos:inScheme cs: ;
    skos:prefLabel "asset identifier"@en ;
    skos:topConceptOf cs: ;
.

:asset-name
    a skos:Concept ;
    dcterms:created "2019-04-14"^^xsd:date ;
    dcterms:creator <https://linked.data.gov.au/org/neii> ;
    skos:definition "descriptive name given to each asset (assigned according to the asset naming rules explained in submethodology M02 for compiling water-dependent assets(Mount et al., 2014))"@en ;
    skos:inScheme cs: ;
    skos:prefLabel "asset name"@en ;
    skos:topConceptOf cs: ;
.

:basement
    a skos:Concept ;
    dcterms:created "2019-04-14"^^xsd:date ;
    dcterms:creator <https://linked.data.gov.au/org/neii> ;
    skos:definition "the crust below the rocks of interest. In hydrogeology it means non-prospective rocks below accessible groundwater. Commonly refers to igneous and metamorphic rocks which are unconformably overlain by sedimentary beds or cover material, and sometimes used to indicate 'bedrock' (i.e. underlying or encasing palaeovalley sediments)."@en ;
    skos:inScheme cs: ;
    skos:prefLabel "basement"@en ;
    skos:topConceptOf cs: ;
.

:bioregional-assessment
    a skos:Concept ;
    dcterms:created "2019-04-14"^^xsd:date ;
    dcterms:creator <https://linked.data.gov.au/org/neii> ;
    dcterms:modified "2020-09-28"^^xsd:date ;
    skos:altLabel "BA"@en ;
    skos:definition "a scientific analysis of the ecology, hydrology, geology and hydrogeology of a bioregion, with explicit assessment of the potential direct, indirect and cumulative impacts of coal seam gas and coal mining development on water resources. The central purpose of bioregional assessments is to analyse the impacts and risks associated with changes to water-dependent assets that arise in response to current and future pathways of coal seam gas and coal mining development."@en ;
    skos:inScheme cs: ;
    skos:prefLabel "bioregional assessment"@en ;
    skos:topConceptOf cs: ;
.

:brownfield-exploration
    a skos:Concept ;
    dcterms:created "2019-04-14"^^xsd:date ;
    dcterms:creator <https://linked.data.gov.au/org/neii> ;
    skos:definition "exploration activities undertaken in areas close to existing mines or known deposits"@en ;
    skos:inScheme cs: ;
    skos:prefLabel "brownfield exploration"@en ;
    skos:topConceptOf cs: ;
.

:causal-pathway
    a skos:Concept ;
    dcterms:created "2019-04-14"^^xsd:date ;
    dcterms:creator <https://linked.data.gov.au/org/neii> ;
    skos:definition "for the purposes of bioregional assessments, the logical chain of events - either planned or unplanned - that link coal resource development and potential impacts on water resources and water-dependent assets"@en ;
    skos:inScheme cs: ;
    skos:prefLabel "causal pathway"@en ;
    skos:topConceptOf cs: ;
.

:coal-deposit
    a skos:Concept ;
    dcterms:created "2019-04-14"^^xsd:date ;
    dcterms:creator <https://linked.data.gov.au/org/neii> ;
    skos:definition "an early stage exploration development category whereby a coal deposit is known to exist in the tenement, although there is insufficient knowledge of the critical deposit characteristics to determine if it is economic or subeconomic to develop into an operating mine at some stage in the future"@en ;
    skos:inScheme cs: ;
    skos:prefLabel "coal deposit"@en ;
    skos:topConceptOf cs: ;
.

:coal-grade
    a skos:Concept ;
    dcterms:created "2019-04-14"^^xsd:date ;
    dcterms:creator <https://linked.data.gov.au/org/neii> ;
    skos:definition "a coal parameter that refers to the amount of inorganic matter that is mixed with the organic components of the coal. Grade is independent of coal type or rank, such that a high-grade coal has a low percentage of inorganic minerals and thus, a high degree of organic matter."@en ;
    skos:inScheme cs: ;
    skos:prefLabel "coal grade"@en ;
    skos:topConceptOf cs: ;
.

:coalification
    a skos:Concept ;
    dcterms:created "2019-04-14"^^xsd:date ;
    dcterms:creator <https://linked.data.gov.au/org/neii> ;
    skos:definition "the process of forming coal from its constituent precursor organic material, due to its burial and compaction beneath younger rock layers"@en ;
    skos:inScheme cs: ;
    skos:prefLabel "coalification"@en ;
    skos:topConceptOf cs: ;
.

:coking-coal
    a skos:Concept ;
    dcterms:created "2019-04-14"^^xsd:date ;
    dcterms:creator <https://linked.data.gov.au/org/neii> ;
    skos:definition "a type of black coal which is used to make coke, a porous solid compound of carbon and ash used in blast furnaces to make various iron-based products, such as steel"@en ;
    skos:inScheme cs: ;
    skos:prefLabel "coking coal"@en ;
    skos:topConceptOf cs: ;
.

:component
    a skos:Concept ;
    dcterms:created "2019-04-14"^^xsd:date ;
    dcterms:creator <https://linked.data.gov.au/org/neii> ;
    skos:definition "for the purposes of Impact Modes and Effects Analysis (IMEA), a group of activities associated with a coal seam gas (CSG) operation or coal mine. For example, components during the development life-cycle stage of a coal mine include developing the mine infrastructure, the open pit, surface facilities and underground facilities. Components are grouped into life-cycle stages."@en ;
    skos:inScheme cs: ;
    skos:prefLabel "component"@en ;
    skos:topConceptOf cs: ;
.

:conceptual-model
    a skos:Concept ;
    dcterms:created "2019-04-14"^^xsd:date ;
    dcterms:creator <https://linked.data.gov.au/org/neii> ;
    skos:definition "abstraction or simplification of reality"@en ;
    skos:inScheme cs: ;
    skos:prefLabel "conceptual model"@en ;
    skos:topConceptOf cs: ;
.

:confined-aquifer
    a skos:Concept ;
    dcterms:created "2019-04-14"^^xsd:date ;
    dcterms:creator <https://linked.data.gov.au/org/neii> ;
    skos:definition "an aquifer saturated with confining layers of low-permeability rock or sediment both above and below it. It is under pressure so that when the aquifer is penetrated by a bore, the water will rise above the top of the aquifer."@en ;
    skos:inScheme cs: ;
    skos:prefLabel "confined aquifer"@en ;
    skos:topConceptOf cs: ;
.

:connectivity
    a skos:Concept ;
    dcterms:created "2019-04-14"^^xsd:date ;
    dcterms:creator <https://linked.data.gov.au/org/neii> ;
    skos:definition "a descriptive measure of the interaction between water bodies (groundwater and/or surface water)"@en ;
    skos:inScheme cs: ;
    skos:prefLabel "connectivity"@en ;
    skos:topConceptOf cs: ;
.

:consequence
    a skos:Concept ;
    dcterms:created "2019-04-14"^^xsd:date ;
    dcterms:creator <https://linked.data.gov.au/org/neii> ;
    skos:definition "synonym of impact"@en ;
    skos:inScheme cs: ;
    skos:prefLabel "consequence"@en ;
    skos:topConceptOf cs: ;
.

:context
    a skos:Concept ;
    dcterms:created "2019-04-14"^^xsd:date ;
    dcterms:creator <https://linked.data.gov.au/org/neii> ;
    skos:definition "the circumstances that form the setting for an event, statement or idea"@en ;
    skos:inScheme cs: ;
    skos:prefLabel "context"@en ;
    skos:topConceptOf cs: ;
.

:cumulative-impact
    a skos:Concept ;
    dcterms:created "2019-04-14"^^xsd:date ;
    dcterms:creator <https://linked.data.gov.au/org/neii> ;
    skos:definition "for the purposes of bioregional assessments, the total change in water resources and water-dependent assets resulting from coal seam gas and coal mining developments when all past, present and reasonably foreseeable actions that are likely to impact on water resources are considered"@en ;
    skos:inScheme cs: ;
    skos:prefLabel "cumulative impact"@en ;
    skos:topConceptOf cs: ;
.

:current-controls
    a skos:Concept ;
    dcterms:created "2019-04-14"^^xsd:date ;
    dcterms:creator <https://linked.data.gov.au/org/neii> ;
    skos:definition "the methods or actions currently planned, or in place, to detect hazards when they occur or to reduce the likelihood and/or consequences of these hazards should they occur"@en ;
    skos:inScheme cs: ;
    skos:prefLabel "current controls"@en ;
    skos:topConceptOf cs: ;
.

:data-files-owner
    a skos:Concept ;
    dcterms:created "2019-04-14"^^xsd:date ;
    dcterms:creator <https://linked.data.gov.au/org/neii> ;
    skos:definition "the person who is responsible for maintaining the dataset's files"@en ;
    skos:inScheme cs: ;
    skos:prefLabel "data files owner"@en ;
    skos:topConceptOf cs: ;
.

:dataset
    a skos:Concept ;
    dcterms:created "2019-04-14"^^xsd:date ;
    dcterms:creator <https://linked.data.gov.au/org/neii> ;
    skos:definition "a collection of data in files, in databases or delivered by services that comprise a related set of information. Datasets may be spatial (e.g. a shape file or geodatabase or a Web Feature Service) or aspatial (e.g. an Access database, a list of people or a model configuration file)."@en ;
    skos:inScheme cs: ;
    skos:prefLabel "dataset"@en ;
    skos:topConceptOf cs: ;
.

:dataset-granularity
    a skos:Concept ;
    dcterms:created "2019-04-14"^^xsd:date ;
    dcterms:creator <https://linked.data.gov.au/org/neii> ;
    skos:definition "the extent to which data is broken down into datasets. There are no strict guidelines on the granularity of a dataset and common sense should be applied. For example, the spatial  boundaries of wetlands and their attributes across Australia could be a single dataset, but a collection of information about wetlands, vegetation and rainfall may be best stored as three datasets rather than one. Conversely, the wetlands dataset need not be split further into each type of wetland or each region. Data Coordinators may be able to  assist in determining the most useful level of granularity to store datasets."@en ;
    skos:inScheme cs: ;
    skos:prefLabel "dataset granularity"@en ;
    skos:topConceptOf cs: ;
.

:dataset-title
    a skos:Concept ;
    dcterms:created "2019-04-14"^^xsd:date ;
    dcterms:creator <https://linked.data.gov.au/org/neii> ;
    skos:definition "the title given to a dataset. A dataset is a collection of data in files, in databases or delivered by services."@en ;
    skos:inScheme cs: ;
    skos:prefLabel "dataset title"@en ;
    skos:topConceptOf cs: ;
.

:deposit-evaluation
    a skos:Concept ;
    dcterms:created "2019-04-14"^^xsd:date ;
    dcterms:creator <https://linked.data.gov.au/org/neii> ;
    skos:definition "the process of undertaking studies of a known and significant deposit of a particular commodity (e.g. coal), for which it is presently uncertain (due to lack of knowledge of critical resource characteristics) if a commercial mining operation is viable"@en ;
    skos:inScheme cs: ;
    skos:prefLabel "deposit evaluation"@en ;
    skos:topConceptOf cs: ;
.

:depressurisation
    a skos:Concept ;
    dcterms:created "2019-04-14"^^xsd:date ;
    dcterms:creator <https://linked.data.gov.au/org/neii> ;
    skos:definition "in the context of coal seam gas operations, depressurisation is the process whereby the hydrostatic (water) pressure within a coal seam is reduced (through pumping) such that natural gas desorbs from within the coal matrix, enabling the gas (and associated water) to flow to surface"@en ;
    skos:inScheme cs: ;
    skos:prefLabel "depressurisation"@en ;
    skos:topConceptOf cs: ;
.

:derived-dataset
    a skos:Concept ;
    dcterms:created "2019-04-14"^^xsd:date ;
    dcterms:creator <https://linked.data.gov.au/org/neii> ;
    skos:definition "a dataset that has been created by the Bioregional Assessment Programme"@en ;
    skos:inScheme cs: ;
    skos:prefLabel "derived dataset"@en ;
    skos:topConceptOf cs: ;
.

:detection-score
    a skos:Concept ;
    dcterms:created "2019-04-14"^^xsd:date ;
    dcterms:creator <https://linked.data.gov.au/org/neii> ;
    skos:definition "for the purposes of Impact Modes and Effects Analysis (IMEA), the expected time to discover a hazard, scored in such a way that a one-unit increase (or decrease) in score indicates a ten-fold increase (or decrease) in the expected time (measured in days) to discover it"@en ;
    skos:inScheme cs: ;
    skos:prefLabel "detection score"@en ;
    skos:topConceptOf cs: ;
.

:dewatering
    a skos:Concept ;
    dcterms:created "2019-04-14"^^xsd:date ;
    dcterms:creator <https://linked.data.gov.au/org/neii> ;
    skos:definition "the process of controlling groundwater flow within and around mining operations that occur below the watertable. In such operations, mine dewatering plans are important to provide more efficient work conditions, improve stability and safety, and enhance economic viability of operations. There are various dewatering methods, such as direct pumping of water from within a mine, installation of dewatering wells around the mine perimeter, and pit slope drains."@en ;
    skos:inScheme cs: ;
    skos:prefLabel "dewatering"@en ;
    skos:topConceptOf cs: ;
.

:direct-impact
    a skos:Concept ;
    dcterms:created "2019-04-14"^^xsd:date ;
    dcterms:creator <https://linked.data.gov.au/org/neii> ;
    skos:definition "for the purposes of bioregional assessments, a change in water resources and water-dependent assets resulting from coal seam gas and coal mining developments without intervening agents or pathways"@en ;
    skos:inScheme cs: ;
    skos:prefLabel "direct impact"@en ;
    skos:topConceptOf cs: ;
.

:discharge
    a skos:Concept ;
    dcterms:created "2019-04-14"^^xsd:date ;
    dcterms:creator <https://linked.data.gov.au/org/neii> ;
    skos:definition "water that moves from a groundwater body to the ground surface or surface water body (e.g. a river or lake)"@en ;
    skos:inScheme cs: ;
    skos:prefLabel "discharge"@en ;
    skos:topConceptOf cs: ;
.

:diversion
    a skos:Concept ;
    dcterms:created "2019-04-14"^^xsd:date ;
    dcterms:creator <https://linked.data.gov.au/org/neii> ;
    skos:definition "see extraction"@en ;
    skos:inScheme cs: ;
    skos:prefLabel "diversion"@en ;
    skos:topConceptOf cs: ;
.

:ecosystem
    a skos:Concept ;
    dcterms:created "2019-04-14"^^xsd:date ;
    dcterms:creator <https://linked.data.gov.au/org/neii> ;
    skos:definition "a dynamic complex of plant, animal, and micro-organism communities and their non-living environment interacting as a functional unit. Note: ecosystems include those that are human-influenced such as rural and urban ecosystems."@en ;
    skos:inScheme cs: ;
    skos:prefLabel "ecosystem"@en ;
    skos:topConceptOf cs: ;
.

:ecosystem-function
    a skos:Concept ;
    dcterms:created "2019-04-14"^^xsd:date ;
    dcterms:creator <https://linked.data.gov.au/org/neii> ;
    skos:definition "the biological, geochemical and physical processes and components that take place or occur within an ecosystem. It refers to the structural components of an ecosystem (e.g. vegetation, water, soil, atmosphere and biota) and how they interact with each other, within ecosystems and across ecosystems."@en ;
    skos:inScheme cs: ;
    skos:prefLabel "ecosystem function"@en ;
    skos:topConceptOf cs: ;
.

:ephemeral-stream
    a skos:Concept ;
    dcterms:created "2019-04-14"^^xsd:date ;
    dcterms:creator <https://linked.data.gov.au/org/neii> ;
    skos:definition "a stream that flows only briefly during and following a period of rainfall, and has no baseflow component"@en ;
    skos:inScheme cs: ;
    skos:prefLabel "ephemeral stream"@en ;
    skos:topConceptOf cs: ;
.

:extraction
    a skos:Concept ;
    dcterms:created "2019-04-14"^^xsd:date ;
    dcterms:creator <https://linked.data.gov.au/org/neii> ;
    skos:definition "the removal of water for use from waterways or aquifers (including storages) by pumping or gravity channels"@en ;
    skos:inScheme cs: ;
    skos:prefLabel "extraction"@en ;
    skos:topConceptOf cs: ;
.

:fairway
    a skos:Concept ;
    dcterms:created "2019-04-14"^^xsd:date ;
    dcterms:creator <https://linked.data.gov.au/org/neii> ;
    skos:definition "a term used in geology to describe a regional trend along which a particular geological feature is likely to occur, such as a hydrocarbon fairway. Understanding and predicting fairways can help geologists explore for various types of resources, such as minerals, oil and gas."@en ;
    skos:inScheme cs: ;
    skos:prefLabel "fairway"@en ;
    skos:topConceptOf cs: ;
.

:fecundity
    a skos:Concept ;
    dcterms:created "2019-04-14"^^xsd:date ;
    dcterms:creator <https://linked.data.gov.au/org/neii> ;
    dcterms:modified "2020-09-29"^^xsd:date ;
    skos:definition "The reproductive capacity of an organism, i.e. the number of eggs that develop in a mated female over a specified period. It is usually calculated at the stage when this number is readily observable (i.e. in oviparous animals when eggs are laid and in viviparous animals when young are born), although strictly speaking it applies from the time that fertilization occurs. Sometimes the term 'fertility' is applied only to the production of fertilized eggs (ova), while 'fecundity' is used for the production of offspring, so excluding those embryos which fail to develop."@en ;
    skos:inScheme cs: ;
    skos:prefLabel "fecundity"@en ;
    skos:topConceptOf cs: ;
.

:focal-analysis-extent
    a skos:Concept ;
    dcterms:created "2019-04-14"^^xsd:date ;
    dcterms:creator <https://linked.data.gov.au/org/neii> ;
    skos:definition "a geographic area that encompasses the modelled areas relevant for the impact analysis of a bioregional assessment (BA), including groundwater, surface water and receptor impact models"@en ;
    skos:inScheme cs: ;
    skos:prefLabel "focal analysis extent"@en ;
    skos:topConceptOf cs: ;
.

:foreland-basin
    a skos:Concept ;
    dcterms:created "2019-04-14"^^xsd:date ;
    dcterms:creator <https://linked.data.gov.au/org/neii> ;
    skos:definition "a type of sedimentary basin formed adjacent to thrust belts and fault-bounded uplifts, and typically infilled with very thick accumulations of sedimentary rocks"@en ;
    skos:inScheme cs: ;
    skos:prefLabel "foreland basin"@en ;
    skos:topConceptOf cs: ;
.

:formation
    a skos:Concept ;
    dcterms:created "2019-04-14"^^xsd:date ;
    dcterms:creator <https://linked.data.gov.au/org/neii> ;
    skos:definition "rock layers that have common physical characteristics (lithology) deposited during a specific period of geological time"@en ;
    skos:inScheme cs: ;
    skos:prefLabel "formation"@en ;
    skos:topConceptOf cs: ;
.

:fractile
    a skos:Concept ;
    dcterms:created "2019-04-14"^^xsd:date ;
    dcterms:creator <https://linked.data.gov.au/org/neii> ;
    skos:definition "the value of a distribution below which some fraction of the sample lies. For example, the 0.95-fractile is the value below which there is a probability of 0.95 occurrence (or equivalently, 95% of the values lie below the 0.95-fractile)."@en ;
    skos:inScheme cs: ;
    skos:prefLabel "fractile"@en ;
    skos:topConceptOf cs: ;
.

:geological-formation
    a skos:Concept ;
    dcterms:created "2019-04-14"^^xsd:date ;
    dcterms:creator <https://linked.data.gov.au/org/neii> ;
    skos:definition "stratigraphic unit with distinct rock types, which is able to mapped at surface or in the subsurface, and which formed at a specific period of geological time"@en ;
    skos:inScheme cs: ;
    skos:prefLabel "geological formation"@en ;
    skos:topConceptOf cs: ;
.

:globally-unique-identifier
    a skos:Concept ;
    dcterms:created "2019-04-14"^^xsd:date ;
    dcterms:creator <https://linked.data.gov.au/org/neii> ;
    skos:definition "for bioregional assessment (BA) purposes, a 'globally unique identifier' (GUID) is an identifier assigned to each dataset in the Bioregional Assessment Data Store (Data Store). GUIDs are a specific implementation of the computer science universally unique ID (UUID) standard. When combined with the web address of the Data Store, a BA GUID forms a BA dataset universal resource identifier (URI) which can be used in web browsers and elsewhere to look up a dataset's metadata."@en ;
    skos:inScheme cs: ;
    skos:prefLabel "globally unique identifier"@en ;
    skos:topConceptOf cs: ;
.

:goaf
    a skos:Concept ;
    dcterms:created "2019-04-14"^^xsd:date ;
    dcterms:creator <https://linked.data.gov.au/org/neii> ;
    skos:definition "That part of a mine from which the coal has been partially or wholly removed; the waste left in old workings."@en ;
    skos:inScheme cs: ;
    skos:prefLabel "goaf"@en ;
    skos:topConceptOf cs: ;
.

:grass-roots-exploration
    a skos:Concept ;
    dcterms:created "2019-04-14"^^xsd:date ;
    dcterms:creator <https://linked.data.gov.au/org/neii> ;
    skos:definition "initial exploration activities in regional greenfield areas at the outset it is unknown if resources for a particular commodity exist within the tenement"@en ;
    skos:inScheme cs: ;
    skos:prefLabel "grass roots exploration"@en ;
    skos:topConceptOf cs: ;
.

:groundwater
    a skos:Concept ;
    dcterms:created "2019-04-14"^^xsd:date ;
    dcterms:creator <https://linked.data.gov.au/org/neii> ;
    skos:definition "water occurring naturally below ground level (whether stored in or flowing through aquifers or within low-permeability aquitards), or water occurring at a place below ground that has been pumped, diverted or released to that place for storage there. This does not include water held in underground tanks, pipes or other works."@en ;
    skos:inScheme cs: ;
    skos:prefLabel "groundwater"@en ;
    skos:topConceptOf cs: ;
.

:groundwater-dependent-ecosystem
    a skos:Concept ;
    dcterms:created "2019-04-14"^^xsd:date ;
    dcterms:creator <https://linked.data.gov.au/org/neii> ;
    dcterms:modified "2020-09-29"^^xsd:date ;
    skos:altLabel "GDE"@en ;
    skos:definition "ecosystems that rely on groundwater - typically the natural discharge of groundwater - for their existence and health"@en ;
    skos:inScheme cs: ;
    skos:prefLabel "groundwater-dependent ecosystem"@en ;
    skos:topConceptOf cs: ;
.

:groundwater-recharge
    a skos:Concept ;
    dcterms:created "2019-04-14"^^xsd:date ;
    dcterms:creator <https://linked.data.gov.au/org/neii> ;
    skos:definition "replenishment of groundwater by natural infiltration of surface water (precipitation, runoff), or artificially via infiltration lakes or injection"@en ;
    skos:inScheme cs: ;
    skos:prefLabel "groundwater recharge"@en ;
    skos:topConceptOf cs: ;
.

:groundwater-system
    a skos:Concept ;
    dcterms:created "2019-04-14"^^xsd:date ;
    dcterms:creator <https://linked.data.gov.au/org/neii> ;
    skos:definition "see water system"@en ;
    skos:inScheme cs: ;
    skos:prefLabel "groundwater system"@en ;
    skos:topConceptOf cs: ;
.

:hazard
    a skos:Concept ;
    dcterms:created "2019-04-14"^^xsd:date ;
    dcterms:creator <https://linked.data.gov.au/org/neii> ;
    skos:definition "an event, or chain of events, that might result in an effect (change in the quality and/or quantity of surface water or groundwater)"@en ;
    skos:inScheme cs: ;
    skos:prefLabel "hazard"@en ;
    skos:topConceptOf cs: ;
.

:hazard-priority-number
    a skos:Concept ;
    dcterms:created "2019-04-14"^^xsd:date ;
    dcterms:creator <https://linked.data.gov.au/org/neii> ;
    dcterms:modified "2020-09-29"^^xsd:date ;
    skos:definition "for the purposes of Impact Modes and Effects Analysis (IMEA), one of two ranking systems that indicate the relative importance of a hazard. It is the sum of severity score, likelihood score and detection score."@en ;
    skos:inScheme cs: ;
    skos:prefLabel "hazard priority number"@en ;
    skos:topConceptOf cs: ;
.

:hazard-score
    a skos:Concept ;
    dcterms:created "2019-04-14"^^xsd:date ;
    dcterms:creator <https://linked.data.gov.au/org/neii> ;
    skos:definition "for the purposes of Impact Modes and Effects Analysis (IMEA), one of two ranking systems that indicate the relative importance of a hazard. It is the sum of the severity score and likelihood score."@en ;
    skos:inScheme cs: ;
    skos:prefLabel "hazard score"@en ;
    skos:topConceptOf cs: ;
.

:hydrogeology
    a skos:Concept ;
    dcterms:created "2019-04-14"^^xsd:date ;
    dcterms:creator <https://linked.data.gov.au/org/neii> ;
    skos:definition "the study of groundwater, including flow in aquifers, groundwater resource evaluation, and the chemistry of interactions between water and rock"@en ;
    skos:inScheme cs: ;
    skos:prefLabel "hydrogeology"@en ;
    skos:topConceptOf cs: ;
.

:impact-cause
    a skos:Concept ;
    dcterms:created "2019-04-14"^^xsd:date ;
    dcterms:creator <https://linked.data.gov.au/org/neii> ;
    skos:definition "an activity (or aspect of an activity) that initiates a hazardous chain of events"@en ;
    skos:inScheme cs: ;
    skos:prefLabel "impact cause"@en ;
    skos:topConceptOf cs: ;
.

:impact-mode
    a skos:Concept ;
    dcterms:created "2019-04-14"^^xsd:date ;
    dcterms:creator <https://linked.data.gov.au/org/neii> ;
    skos:definition "the manner in which a hazardous chain of events (initiated by an impact cause) could result in an effect (change in the quality and/or quantity of surface water or groundwater). There might be multiple impact modes for each activity or chain of events."@en ;
    skos:inScheme cs: ;
    skos:prefLabel "impact mode"@en ;
    skos:topConceptOf cs: ;
.

:indirect-impact
    a skos:Concept ;
    dcterms:created "2019-04-14"^^xsd:date ;
    dcterms:creator <https://linked.data.gov.au/org/neii> ;
    skos:definition "for the purposes of bioregional assessments, a change in water resources and water-dependent assets resulting from coal seam gas and coal mining developments with one or more intervening agents or pathways"@en ;
    skos:inScheme cs: ;
    skos:prefLabel "indirect impact"@en ;
    skos:topConceptOf cs: ;
.

:inertinite
    a skos:Concept ;
    dcterms:created "2019-04-14"^^xsd:date ;
    dcterms:creator <https://linked.data.gov.au/org/neii> ;
    skos:definition "one of the main maceral groups for humic coal, which are those coals formed predominantly from woody or sedge/reed plant remains. Humic coals tend to form in moist, aerobic zones within a mire, through the process of peatification. Inertinite has a varied origin, including fire, biochemical or microbial, and oxidation origins. Specific macerals of the inertinite group inlcude fusinite, funginite, secretinite, and micrinite (to name a few)"@en ;
    skos:inScheme cs: ;
    skos:prefLabel "inertinite"@en ;
    skos:topConceptOf cs: ;
.

:inflow
    a skos:Concept ;
    dcterms:created "2019-04-14"^^xsd:date ;
    dcterms:creator <https://linked.data.gov.au/org/neii> ;
    skos:definition "surface water runoff and deep drainage to groundwater (groundwater recharge) and transfers into the water system (both surface water and groundwater) for a defined area"@en ;
    skos:inScheme cs: ;
    skos:prefLabel "inflow"@en ;
    skos:topConceptOf cs: ;
.

:life-cycle-stage
    a skos:Concept ;
    dcterms:created "2019-04-14"^^xsd:date ;
    dcterms:creator <https://linked.data.gov.au/org/neii> ;
    skos:definition "one of five stages of operations in coal resource development considered as part of the Impact Modes and Effects Analysis (IMEA). For coal seam gas (CSG) operations these are exploration and appraisal, construction, production, work-over and decommissioning. For coal mines these are exploration and appraisal, development, production, closure and rehabilitation. Each life-cycle stage is further divided into components, which are further divided into activities."@en ;
    skos:inScheme cs: ;
    skos:prefLabel "life-cycle stage"@en ;
    skos:topConceptOf cs: ;
.

:likelihood
    a skos:Concept ;
    dcterms:created "2019-04-14"^^xsd:date ;
    dcterms:creator <https://linked.data.gov.au/org/neii> ;
    skos:definition "probability that something might happen"@en ;
    skos:inScheme cs: ;
    skos:prefLabel "likelihood"@en ;
    skos:topConceptOf cs: ;
.

:likelihood-score
    a skos:Concept ;
    dcterms:created "2019-04-14"^^xsd:date ;
    dcterms:creator <https://linked.data.gov.au/org/neii> ;
    skos:definition "for the purposes of Impact Modes and Effects Analysis (IMEA), the annual probability of a hazard occurring, which is scored so that a one-unit increase (or decrease) in score indicates a ten-fold increase (or decrease) in the probability of occurrence"@en ;
    skos:inScheme cs: ;
    skos:prefLabel "likelihood score"@en ;
    skos:topConceptOf cs: ;
.

:list-date
    a skos:Concept ;
    dcterms:created "2019-04-14"^^xsd:date ;
    dcterms:creator <https://linked.data.gov.au/org/neii> ;
    skos:definition "the date the element was added to the element list"@en ;
    skos:inScheme cs: ;
    skos:prefLabel "list date"@en ;
    skos:topConceptOf cs: ;
.

:lithic
    a skos:Concept ;
    dcterms:created "2019-04-14"^^xsd:date ;
    dcterms:creator <https://linked.data.gov.au/org/neii> ;
    skos:definition "sediment or sedimentary rock that contains a significant proportion of detrital rock fragments (10 to 50%) derived by erosion from older, pre-existing rock outcrop"@en ;
    skos:inScheme cs: ;
    skos:prefLabel "lithic"@en ;
    skos:topConceptOf cs: ;
.

:marine-transgression
    a skos:Concept ;
    dcterms:created "2019-04-14"^^xsd:date ;
    dcterms:creator <https://linked.data.gov.au/org/neii> ;
    skos:definition "the landward spreading of the sea over a large area within relatively short space of geological time (a few million years or less). The reverse of transgression is regression."@en ;
    skos:inScheme cs: ;
    skos:prefLabel "marine transgression"@en ;
    skos:topConceptOf cs: ;
.

:material
    a skos:Concept ;
    dcterms:created "2019-04-14"^^xsd:date ;
    dcterms:creator <https://linked.data.gov.au/org/neii> ;
    skos:definition "pertinent or relevant"@en ;
    skos:inScheme cs: ;
    skos:prefLabel "material"@en ;
    skos:topConceptOf cs: ;
.

:metadata-author
    a skos:Concept ;
    dcterms:created "2019-04-14"^^xsd:date ;
    dcterms:creator <https://linked.data.gov.au/org/neii> ;
    skos:definition "the person who writes metadata to Bioregional Assessment quality standards"@en ;
    skos:inScheme cs: ;
    skos:prefLabel "metadata author"@en ;
    skos:topConceptOf cs: ;
.

:metadata-record-owner
    a skos:Concept ;
    dcterms:created "2019-04-14"^^xsd:date ;
    dcterms:creator <https://linked.data.gov.au/org/neii> ;
    skos:definition "the person responsible for filling out a registered dataset's metadata record in the Bioregional Assessment Metadata Catalogue. This person is assigned by the Metadata Record Coordinator."@en ;
    skos:inScheme cs: ;
    skos:prefLabel "metadata record owner"@en ;
    skos:topConceptOf cs: ;
.

:metasedimentary-rock
    a skos:Concept ;
    dcterms:created "2019-04-14"^^xsd:date ;
    dcterms:creator <https://linked.data.gov.au/org/neii> ;
    skos:definition "sedimentary rock altered by metamorphism, typically modifying one or more aspect of the primary texture, chemistry, or mineralogy. Commonly, original sedimentary features (such as bedding) may be preserved"@en ;
    skos:inScheme cs: ;
    skos:prefLabel "metasedimentary rock"@en ;
    skos:topConceptOf cs: ;
.

:model-chain
    a skos:Concept ;
    dcterms:created "2019-04-14"^^xsd:date ;
    dcterms:creator <https://linked.data.gov.au/org/neii> ;
    skos:definition "a series of linked models where the output of one model becomes an input to another"@en ;
    skos:inScheme cs: ;
    skos:prefLabel "model chain"@en ;
    skos:topConceptOf cs: ;
.

:model-domain-extent
    a skos:Concept ;
    dcterms:created "2019-04-14"^^xsd:date ;
    dcterms:creator <https://linked.data.gov.au/org/neii> ;
    skos:definition "the geographic area that encompasses a model or models, such as the groundwater and surface water models used for the impact analysis of a bioregional assessment(BA)"@en ;
    skos:inScheme cs: ;
    skos:prefLabel "model domain extent"@en ;
    skos:topConceptOf cs: ;
.

:model-emulator
    a skos:Concept ;
    dcterms:created "2019-04-14"^^xsd:date ;
    dcterms:creator <https://linked.data.gov.au/org/neii> ;
    skos:definition "a computationally efficient statistical approximation of a process model that mimics the effect of parameter values on a model prediction. In uncertainty analysis a slow, complex process model is replaced by an emulator, which, for a given parameter combination, will provide a prediction that is very close to the prediction that would be obtained by running the process model."@en ;
    skos:inScheme cs: ;
    skos:prefLabel "model emulator"@en ;
    skos:topConceptOf cs: ;
.

:model-node
    a skos:Concept ;
    dcterms:created "2019-04-14"^^xsd:date ;
    dcterms:creator <https://linked.data.gov.au/org/neii> ;
    skos:definition "a point in the landscape where hydrological changes (and their uncertainty) are assessed. Hydrological changes at points other than model nodes are obtained by interpolation."@en ;
    skos:inScheme cs: ;
    skos:prefLabel "model node"@en ;
    skos:topConceptOf cs: ;
.

:model-spin-up-period
    a skos:Concept ;
    dcterms:created "2019-04-14"^^xsd:date ;
    dcterms:creator <https://linked.data.gov.au/org/neii> ;
    skos:definition "a period of time in which the model is allowed to run prior to the period for which predictions are required. A spin-up period allows the initial values of any model stores (such as the soil water stores) before the prediction period begins."@en ;
    skos:inScheme cs: ;
    skos:prefLabel "model spin-up period"@en ;
    skos:topConceptOf cs: ;
.

:overbank-flow
    a skos:Concept ;
    dcterms:created "2019-04-14"^^xsd:date ;
    dcterms:creator <https://linked.data.gov.au/org/neii> ;
    skos:definition "flood condition where water flows beyond and sub-parallel to the main channel of a river, but within the bounding floodplain"@en ;
    skos:inScheme cs: ;
    skos:prefLabel "overbank flow"@en ;
    skos:topConceptOf cs: ;
.

:overbench-flow
    a skos:Concept ;
    dcterms:created "2019-04-14"^^xsd:date ;
    dcterms:creator <https://linked.data.gov.au/org/neii> ;
    skos:definition "high-flow condition where a river channel is partially or completely filled for a period of weeks to months. All habitats within the river channel will be wet including boulders, logs and lateral benches, and the entire length of the channel is connected with relatively deep water, allowing movement of biota freely along the river."@en ;
    skos:inScheme cs: ;
    skos:prefLabel "overbench flow"@en ;
    skos:topConceptOf cs: ;
.

:percentile
    a skos:Concept ;
    dcterms:created "2019-04-14"^^xsd:date ;
    dcterms:creator <https://linked.data.gov.au/org/neii> ;
    skos:definition "a specific type of quantile where the range of a distribution or set of runs is divided into 100 contiguous intervals, each with probability 0.01. An individual percentile may be used to indicate the value below which a given percentage or proportion of observations in a group of observations fall. For example, the 95th percentile is the value below which 95% of the observations may be found."@en ;
    skos:inScheme cs: ;
    skos:prefLabel "percentile"@en ;
    skos:topConceptOf cs: ;
.

:permeability
    a skos:Concept ;
    dcterms:created "2019-04-14"^^xsd:date ;
    dcterms:creator <https://linked.data.gov.au/org/neii> ;
    skos:definition "the measure of the ability of a rock, soil or sediment to yield or transmit a fluid. The magnitude of permeability depends largely on the porosity and the interconnectivity of pores and spaces in the ground."@en ;
    skos:inScheme cs: ;
    skos:prefLabel "permeability"@en ;
    skos:topConceptOf cs: ;
.

:piezometric-surface
    a skos:Concept ;
    dcterms:created "2019-04-14"^^xsd:date ;
    dcterms:creator <https://linked.data.gov.au/org/neii> ;
    skos:definition "a theoretical surface representing the pressure of groundwater in an aquifer. It is defined by the level that water is measured in the bore that penetrates the aquifer."@en ;
    skos:inScheme cs: ;
    skos:prefLabel "piezometric surface"@en ;
    skos:topConceptOf cs: ;
.

:plugged-and-abandoned
    a skos:Concept ;
    dcterms:created "2019-04-14"^^xsd:date ;
    dcterms:creator <https://linked.data.gov.au/org/neii> ;
    skos:definition "refers to a well that, after it has been deemed unproductive, and the surface casing, wellhead and other equipment are removed, is plugged with cement to prevent fluid migration and is sealed below the surface. Consequently, the well is permanently closed, and the surrounding land is reclaimed and rehabilitated."@en ;
    skos:inScheme cs: ;
    skos:prefLabel "plugged and abandoned"@en ;
    skos:topConceptOf cs: ;
.

:pmax
    a skos:Concept ;
    dcterms:created "2019-04-14"^^xsd:date ;
    dcterms:creator <https://linked.data.gov.au/org/neii> ;
    skos:definition "maximum percent change"@en ;
    skos:inScheme cs: ;
    skos:prefLabel "pmax"@en ;
    skos:topConceptOf cs: ;
.

:porosity
    a skos:Concept ;
    dcterms:created "2019-04-14"^^xsd:date ;
    dcterms:creator <https://linked.data.gov.au/org/neii> ;
    skos:definition "the proportion of the volume of rock consisting of pores, usually expressed as a percentage of the total rock or soil mass"@en ;
    skos:inScheme cs: ;
    skos:prefLabel "porosity"@en ;
    skos:topConceptOf cs: ;
.

:probability-distribution
    a skos:Concept ;
    dcterms:created "2019-04-14"^^xsd:date ;
    dcterms:creator <https://linked.data.gov.au/org/neii> ;
    skos:definition "the probability distribution of a random variable specifies the chance that the variable takes a value in any subset of the real numbers. It allows statements such as 'There is a probability of x that the variable is between a and b'."@en ;
    skos:inScheme cs: ;
    skos:prefLabel "probability distribution"@en ;
    skos:topConceptOf cs: ;
.

:quantile
    a skos:Concept ;
    dcterms:created "2019-04-14"^^xsd:date ;
    dcterms:creator <https://linked.data.gov.au/org/neii> ;
    skos:definition "a set of values of a variate that divide the range of a probability distribution into contiguous intervals with equal probabilities (e.g. 20 intervals with probability 0.05, or 100 intervals with probability 0.01). Within bioregional assessments, probability distributions are approximated using a number of runs or realisations."@en ;
    skos:inScheme cs: ;
    skos:prefLabel "quantile"@en ;
    skos:topConceptOf cs: ;
.

:receptor
    a skos:Concept ;
    dcterms:created "2019-04-14"^^xsd:date ;
    dcterms:creator <https://linked.data.gov.au/org/neii> ;
    skos:definition "a point in the landscape where water-related impacts on assets are assessed"@en ;
    skos:inScheme cs: ;
    skos:prefLabel "receptor"@en ;
    skos:topConceptOf cs: ;
.

:receptor-impact-variable
    a skos:Concept ;
    dcterms:created "2019-04-14"^^xsd:date ;
    dcterms:creator <https://linked.data.gov.au/org/neii> ;
    dcterms:modified "2020-09-29"^^xsd:date ;
    skos:definition "a characteristic of the system that, according to the conceptual modelling, potentially changes due to changes in hydrological response variables (for example, condition of the breeding habitat for a given species, or biomass of river red gums)"@en ;
    skos:inScheme cs: ;
    skos:prefLabel "receptor impact variable"@en ;
    skos:topConceptOf cs: ;
.

:receptor-register
    a skos:Concept ;
    dcterms:created "2019-04-14"^^xsd:date ;
    dcterms:creator <https://linked.data.gov.au/org/neii> ;
    skos:definition "a simple and authoritative list of receptors in a specific bioregional assessment"@en ;
    skos:inScheme cs: ;
    skos:prefLabel "receptor register"@en ;
    skos:topConceptOf cs: ;
.

:recharge
    a skos:Concept ;
    dcterms:created "2019-04-14"^^xsd:date ;
    dcterms:creator <https://linked.data.gov.au/org/neii> ;
    skos:definition "see groundwater recharge"@en ;
    skos:inScheme cs: ;
    skos:prefLabel "recharge"@en ;
    skos:topConceptOf cs: ;
.

:regional-watertable
    a skos:Concept ;
    dcterms:created "2019-04-14"^^xsd:date ;
    dcterms:creator <https://linked.data.gov.au/org/neii> ;
    skos:definition "the upper groundwater level within the unconfined, near-surface aquifer (not perched), where pore water pressure is equal to atmospheric pressure. For bioregional assessment (BA) purposes, the regional watertable is developed by combining, at the subregion or bioregion scale, the watertable from all the near-surface geological units (or layers) in which it occurs, so that impacts to water-dependent assets and ecosystems can be assessed. As the regional watertable is not a contiguous geological layer, water may not move freely through it."@en ;
    skos:inScheme cs: ;
    skos:prefLabel "regional-watertable"@en ;
    skos:topConceptOf cs: ;
.

:repeatability
    a skos:Concept ;
    dcterms:created "2019-04-14"^^xsd:date ;
    dcterms:creator <https://linked.data.gov.au/org/neii> ;
    skos:definition "the extent to which materially consistent results are obtained when Assessment teams redo part or all of a bioregional assessment using the same methods, models, data, software and computer systems. Some domains use 'replicability' interchangeably with 'repeatability'."@en ;
    skos:inScheme cs: ;
    skos:prefLabel "repeatability"@en ;
    skos:topConceptOf cs: ;
.

:reproducibility
    a skos:Concept ;
    dcterms:created "2019-04-14"^^xsd:date ;
    dcterms:creator <https://linked.data.gov.au/org/neii> ;
    skos:definition "the extent to which materially consistent results are obtained when experts outside of the Assessment teams redo part or all of a bioregional assessment using the same methods, models, data and software, but different computer systems"@en ;
    skos:inScheme cs: ;
    skos:prefLabel "reproducibility"@en ;
    skos:topConceptOf cs: ;
.

:response-variables
    a skos:Concept ;
    dcterms:created "2019-04-14"^^xsd:date ;
    dcterms:creator <https://linked.data.gov.au/org/neii> ;
    skos:definition "variables that relate parameters, state variables and/or fluxes in groundwater and surface water models with impacts on receptors. Response variables also link receptors with subsequent advice on monitoring programs."@en ;
    skos:inScheme cs: ;
    skos:prefLabel "response variables"@en ;
    skos:topConceptOf cs: ;
.

:return-period
    a skos:Concept ;
    dcterms:created "2019-04-14"^^xsd:date ;
    dcterms:creator <https://linked.data.gov.au/org/neii> ;
    skos:definition "An event has a return period (or recurrence interval) of T years if its magnitude is equalled or exceeded once on average every T years. The reciprocal of the return period is the exceedance probability of the event, that is, the probability that the event is equalled or exceeded in any one year. For example, a flood with a return period of 10 years has a 0.1 or 10% chance of being exceeded in any one year and a flood with a return period of 50 years has a 0.02 or 2% chance of being exceeded in any one year. The actual number of years between floods of any given size varies a lot because of climatic variability."@en ;
    skos:inScheme cs: ;
    skos:prefLabel "return period"@en ;
    skos:topConceptOf cs: ;
.

:riparian
    a skos:Concept ;
    dcterms:created "2019-04-14"^^xsd:date ;
    dcterms:creator <https://linked.data.gov.au/org/neii> ;
    skos:definition "An area or zone within or along the banks of a stream or adjacent to a watercourse or wetland; relating to a riverbank and its environment, particularly to the vegetation."@en ;
    skos:inScheme cs: ;
    skos:prefLabel "riparian"@en ;
    skos:topConceptOf cs: ;
.

:risk
    a skos:Concept ;
    dcterms:created "2019-04-14"^^xsd:date ;
    dcterms:creator <https://linked.data.gov.au/org/neii> ;
    skos:definition "the effect of uncertainty on objectives"@en ;
    skos:inScheme cs: ;
    skos:prefLabel "risk"@en ;
    skos:topConceptOf cs: ;
.

:riverbed-conductance
    a skos:Concept ;
    dcterms:created "2019-04-14"^^xsd:date ;
    dcterms:creator <https://linked.data.gov.au/org/neii> ;
    skos:definition "a parameter used in the river package of MODFLOW. It is defined as the result of the product of hydraulic conductivity of the riverbed materials and the area (width times the length) of the river in the cell, divided by the vertical thickness of the riverbed materials."@en ;
    skos:inScheme cs: ;
    skos:prefLabel "riverbed conductance"@en ;
    skos:topConceptOf cs: ;
.

:rune-of-mine-coal
    a skos:Concept ;
    dcterms:created "2019-04-14"^^xsd:date ;
    dcterms:creator <https://linked.data.gov.au/org/neii> ;
    dcterms:modified "2020-09-29"^^xsd:date ;
    skos:altLabel
        "ROM"@en ,
        "run-of-mine"@en ;
    skos:definition "refers to coal extracted from a mining operation and delivered to a coal handling and preparation plant (CHPP), prior to any further processing stages that may be required. The ROM coal is essentially the raw material from the mine that feeds the CHPP and, in addition to coal, may also include minor non-coal rocks and minerals."@en ;
    skos:inScheme cs: ;
    skos:prefLabel "rune-of-mine coal"@en ;
    skos:topConceptOf cs: ;
.

:runoff
    a skos:Concept ;
    dcterms:created "2019-04-14"^^xsd:date ;
    dcterms:creator <https://linked.data.gov.au/org/neii> ;
    skos:definition "rainfall that does not infiltrate the ground or evaporate to the atmosphere. This water flows down a slope and enters surface water systems."@en ;
    skos:inScheme cs: ;
    skos:prefLabel "runoff'"@en ;
    skos:topConceptOf cs: ;
.

:saturated-zone
    a skos:Concept ;
    dcterms:created "2019-04-14"^^xsd:date ;
    dcterms:creator <https://linked.data.gov.au/org/neii> ;
    skos:definition "the part of the ground in which all the voids in the rocks or soil are filled with water. The watertable is the top of the saturated zone in an unconfined aquifer."@en ;
    skos:inScheme cs: ;
    skos:prefLabel "saturated zone"@en ;
    skos:topConceptOf cs: ;
.

:scalar-value
    a skos:Concept ;
    dcterms:created "2019-04-14"^^xsd:date ;
    dcterms:creator <https://linked.data.gov.au/org/neii> ;
    skos:definition "a single real number that describes a measurable quantity, such as temperature, length or groundwater level"@en ;
    skos:inScheme cs: ;
    skos:prefLabel "scalar value"@en ;
    skos:topConceptOf cs: ;
.

:sensitivity
    a skos:Concept ;
    dcterms:created "2019-04-14"^^xsd:date ;
    dcterms:creator <https://linked.data.gov.au/org/neii> ;
    skos:definition "the degree to which the output of a model (numerical or otherwise) responds to uncertainty in a model input"@en ;
    skos:inScheme cs: ;
    skos:prefLabel "sensitivity"@en ;
    skos:topConceptOf cs: ;
.

:severity
    a skos:Concept ;
    dcterms:created "2019-04-14"^^xsd:date ;
    dcterms:creator <https://linked.data.gov.au/org/neii> ;
    skos:definition "magnitude of an impact"@en ;
    skos:inScheme cs: ;
    skos:prefLabel "severity"@en ;
    skos:topConceptOf cs: ;
.

:severity-score
    a skos:Concept ;
    dcterms:created "2019-04-14"^^xsd:date ;
    dcterms:creator <https://linked.data.gov.au/org/neii> ;
    skos:definition "for the purposes of Impact Modes and Effects Analysis (IMEA), the magnitude of the impact resulting from a hazard, which is scored so that an increase (or decrease) in score indicates an increase (or decrease) in the magnitude of the impact"@en ;
    skos:inScheme cs: ;
    skos:prefLabel "severity score"@en ;
    skos:topConceptOf cs: ;
.

:sleeper-licence
    a skos:Concept ;
    dcterms:created "2019-04-14"^^xsd:date ;
    dcterms:creator <https://linked.data.gov.au/org/neii> ;
    skos:definition "a licence that uses none (or little) of its allocation or entitlement over the course of the water year but has the potential to be used"@en ;
    skos:inScheme cs: ;
    skos:prefLabel "sleeper licence"@en ;
    skos:topConceptOf cs: ;
.

:source-dataset
    a skos:Concept ;
    dcterms:created "2019-04-14"^^xsd:date ;
    dcterms:creator <https://linked.data.gov.au/org/neii> ;
    skos:definition "a pre-existing dataset sourced from outside the Bioregional Assessment Programme (including from Programme partner organisations) or a dataset created by the Programme based on analyses conducted by the Programme for use in the bioregional assessments (BAs)"@en ;
    skos:inScheme cs: ;
    skos:prefLabel "source dataset"@en ;
    skos:topConceptOf cs: ;
.

:spring
    a skos:Concept ;
    dcterms:created "2019-04-14"^^xsd:date ;
    dcterms:creator <https://linked.data.gov.au/org/neii> ;
    skos:definition "a naturally occurring discharge of groundwater flowing out of the ground, often forming a small stream or pool of water. Typically, it represents the point at which the watertable intersects ground level."@en ;
    skos:inScheme cs: ;
    skos:prefLabel "spring"@en ;
    skos:topConceptOf cs: ;
.

:stationary-system
    a skos:Concept ;
    dcterms:created "2019-04-14"^^xsd:date ;
    dcterms:creator <https://linked.data.gov.au/org/neii> ;
    skos:definition "a system in which the hydrological regime or other conditions do not vary through time"@en ;
    skos:inScheme cs: ;
    skos:prefLabel "stationary system"@en ;
    skos:topConceptOf cs: ;
.

:stratigraphy
    a skos:Concept ;
    dcterms:created "2019-04-14"^^xsd:date ;
    dcterms:creator <https://linked.data.gov.au/org/neii> ;
    skos:definition "stratified (layered) rocks"@en ;
    skos:inScheme cs: ;
    skos:prefLabel "stratigraphy"@en ;
    skos:topConceptOf cs: ;
.

:stressor
    a skos:Concept ;
    dcterms:created "2019-04-14"^^xsd:date ;
    dcterms:creator <https://linked.data.gov.au/org/neii> ;
    skos:definition "chemical or biological agent, environmental condition or external stimulus that might contribute to an impact mode"@en ;
    skos:inScheme cs: ;
    skos:prefLabel "stressor"@en ;
    skos:topConceptOf cs: ;
.

:subcrop
    a skos:Concept ;
    dcterms:created "2019-04-14"^^xsd:date ;
    dcterms:creator <https://linked.data.gov.au/org/neii> ;
    skos:definition "1 - A subsurface outcrop, e.g. where a formation intersects a subsurface plane such as an unconformity. 2 - In mining, any near-surface development of a rock or orebody, usually beneath superficial material."@en ;
    skos:inScheme cs: ;
    skos:prefLabel "subcrop"@en ;
    skos:topConceptOf cs: ;
.

:subregion
    a skos:Concept ;
    dcterms:created "2019-04-14"^^xsd:date ;
    dcterms:creator <https://linked.data.gov.au/org/neii> ;
    dcterms:modified "2020-09-29"^^xsd:date ;
    skos:definition "an identified area wholly contained within a bioregion that enables convenient presentation of outputs of a bioregional assessment (BA)"@en ;
    skos:inScheme cs: ;
    skos:prefLabel "subregion"@en ;
    skos:topConceptOf cs: ;
.

:subsidence
    a skos:Concept ;
    dcterms:created "2019-04-14"^^xsd:date ;
    dcterms:creator <https://linked.data.gov.au/org/neii> ;
    skos:definition "localised lowering of the land surface. It occurs when underground voids or cavities collapse, or when soil or geological formations (including coal seams, sandstone and other sedimentary strata) compact due to reduction in moisture content and pressure within the ground."@en ;
    skos:inScheme cs: ;
    skos:prefLabel "subsidence"@en ;
    skos:topConceptOf cs: ;
.

:surface-water
    a skos:Concept ;
    dcterms:created "2019-04-14"^^xsd:date ;
    dcterms:creator <https://linked.data.gov.au/org/neii> ;
    skos:definition "water that flows over land and in watercourses or artificial channels and can be captured, stored and supplemented from dams and reservoirs"@en ;
    skos:inScheme cs: ;
    skos:prefLabel "surface water"@en ;
    skos:topConceptOf cs: ;
.

:sustainable-yield
    a skos:Concept ;
    dcterms:created "2019-04-14"^^xsd:date ;
    dcterms:creator <https://linked.data.gov.au/org/neii> ;
    skos:definition "the level of water extraction from a particular system that, if exceeded, would compromise the productive base of the water resource and important environmental assets or ecosystem functions"@en ;
    skos:inScheme cs: ;
    skos:prefLabel "sustainable yield"@en ;
    skos:topConceptOf cs: ;
.

:tenement
    a skos:Concept ;
    dcterms:created "2019-04-14"^^xsd:date ;
    dcterms:creator <https://linked.data.gov.au/org/neii> ;
    skos:definition "a defined area of land granted by a relevant government authority under prescribed legislative conditions to permit various activities associated with the exploration, development and mining of a specific mineral or energy resource, such as coal. Administration and granting of tenements is usually undertaken by state and territory governments, with various types related to the expected level and style of exploration and mining. Tenements are important mechanisms to maintain standards and safeguards relating to environmental factors and other land uses, including native title."@en ;
    skos:inScheme cs: ;
    skos:prefLabel "tenement"@en ;
    skos:topConceptOf cs: ;
.

:transmissivity
    a skos:Concept ;
    dcterms:created "2019-04-14"^^xsd:date ;
    dcterms:creator <https://linked.data.gov.au/org/neii> ;
    skos:definition "A parameter indicating the ease of groundwater flow through a metre width of aquifer section (taken perpendicular to the direction of flow)."@en ;
    skos:inScheme cs: ;
    skos:prefLabel "transmissivity"@en ;
    skos:topConceptOf cs: ;
.

:transparency
    a skos:Concept ;
    dcterms:created "2019-04-14"^^xsd:date ;
    dcterms:creator <https://linked.data.gov.au/org/neii> ;
    skos:definition "a key requirement for the Bioregional Assessment Programme, achieved by providing the methods and unencumbered models, data and software to the public so that experts outside of the Assessment team can understand how a bioregional assessment was undertaken and update it using different models, data or software"@en ;
    skos:inScheme cs: ;
    skos:prefLabel "transparency"@en ;
    skos:topConceptOf cs: ;
.

:uncertainty
    a skos:Concept ;
    dcterms:created "2019-04-14"^^xsd:date ;
    dcterms:creator <https://linked.data.gov.au/org/neii> ;
    dcterms:modified "2020-09-29"^^xsd:date ;
    skos:altLabel "uncertainties"@en ;
    skos:definition "the state, even partial, of deficiency of information related to understanding or knowledge of an event, its consequence, or likelihood. For the purposes of bioregional assessments, uncertainty includes: the variation caused by natural fluctuations or heterogeneity; the incomplete knowledge or understanding of the system under consideration; and the simplification or abstraction of the system in the conceptual and numerical models."@en ;
    skos:inScheme cs: ;
    skos:prefLabel "uncertainty"@en ;
    skos:topConceptOf cs: ;
.

:unconfined-aquifer
    a skos:Concept ;
    dcterms:created "2019-04-14"^^xsd:date ;
    dcterms:creator <https://linked.data.gov.au/org/neii> ;
    skos:definition "an aquifer whose upper water surface (watertable) is at atmospheric pressure and does not have a confining layer of low-permeability rock or sediment above it"@en ;
    skos:inScheme cs: ;
    skos:prefLabel "unconfined aquifer"@en ;
    skos:topConceptOf cs: ;
.

:unsaturated-zone
    a skos:Concept ;
    dcterms:created "2019-04-14"^^xsd:date ;
    dcterms:creator <https://linked.data.gov.au/org/neii> ;
    skos:definition "the zone in soils and rocks occurring above the watertable, where there is some air within the pore spaces"@en ;
    skos:inScheme cs: ;
    skos:prefLabel "unsaturated zone"@en ;
    skos:topConceptOf cs: ;
.

:very-likely
    a skos:Concept ;
    dcterms:created "2019-04-14"^^xsd:date ;
    dcterms:creator <https://linked.data.gov.au/org/neii> ;
    dcterms:modified "2020-09-29"^^xsd:date ;
    skos:definition "greater than 95% chance"@en ;
    skos:inScheme cs: ;
    skos:prefLabel "very likely"@en ;
    skos:topConceptOf cs: ;
.

:very-unlikely
    a skos:Concept ;
    dcterms:created "2019-04-14"^^xsd:date ;
    dcterms:creator <https://linked.data.gov.au/org/neii> ;
    dcterms:modified "2020-09-29"^^xsd:date ;
    skos:definition "less than 5% chance"@en ;
    skos:inScheme cs: ;
    skos:prefLabel "very unlikely"@en ;
    skos:topConceptOf cs: ;
.

:water-allocation
    a skos:Concept ;
    dcterms:created "2019-04-14"^^xsd:date ;
    dcterms:creator <https://linked.data.gov.au/org/neii> ;
    skos:definition "the specific volume of water allocated to water access entitlements in a given season, defined according to rules established in the relevant water plan"@en ;
    skos:inScheme cs: ;
    skos:prefLabel "water allocation"@en ;
    skos:topConceptOf cs: ;
.

:water-dependent-asset-register
    a skos:Concept ;
    dcterms:created "2019-04-14"^^xsd:date ;
    dcterms:creator <https://linked.data.gov.au/org/neii> ;
    skos:definition "a simple and authoritative listing of the assets within the preliminary assessment extent (PAE) that are potentially subject to water-related impacts"@en ;
    skos:inScheme cs: ;
    skos:prefLabel "water-dependent asset register"@en ;
    skos:topConceptOf cs: ;
.

:water-make
    a skos:Concept ;
    dcterms:created "2019-04-14"^^xsd:date ;
    dcterms:creator <https://linked.data.gov.au/org/neii> ;
    skos:definition "the groundwater extracted for dewatering mines"@en ;
    skos:inScheme cs: ;
    skos:prefLabel "water make"@en ;
    skos:topConceptOf cs: ;
.

:water-use
    a skos:Concept ;
    dcterms:created "2019-04-14"^^xsd:date ;
    dcterms:creator <https://linked.data.gov.au/org/neii> ;
    skos:definition "the volume of water diverted from a stream, extracted from groundwater, or transferred to another area for use. It is not representative of 'on-farm' or 'town' use; rather it represents the volume taken from the environment."@en ;
    skos:inScheme cs: ;
    skos:prefLabel "water use"@en ;
    skos:topConceptOf cs: ;
.

:watertable
    a skos:Concept ;
    dcterms:created "2019-04-14"^^xsd:date ;
    dcterms:creator <https://linked.data.gov.au/org/neii> ;
    skos:definition "the upper surface of a body of groundwater occurring in an unconfined aquifer. At the watertable, pore water pressure equals atmospheric pressure."@en ;
    skos:inScheme cs: ;
    skos:prefLabel "watertable"@en ;
    skos:topConceptOf cs: ;
.

<https://linked.data.gov.au/org/bap>
    a dcterms:Agent ;
    schema:name "Bioregional Assessment Programme" ;
.

:Central-West-subregion
    a skos:Concept ;
    dcterms:created "2019-04-14"^^xsd:date ;
    dcterms:creator <https://linked.data.gov.au/org/neii> ;
    dcterms:modified "2020-09-28"^^xsd:date ;
    skos:broader :Northern-Inland-Catchments-bioregion ;
    skos:definition "The main rivers in the Central West subregion are the Macquarie, Castlereagh and Bogan rivers of the Murray-Darling Basin. The subregion extends from the plains around Dubbo across the low-lying plains of the Macquarie and Castlereagh river systems north-west to the Barwon River floodplains. The main cities and towns for the subregion are Dubbo, Coonabarabran, Coonamble, Gilgandra and Nyngan. Most of the land in the subregion is used for agriculture (grazing and cropping). The subregion contains seasonal, semi-permanent and permanent wetlands and lagoons, including the Macquarie Marshes which is an internationally recognised and protected wetland. The subregion is home to a number of water-dependent ecological communities, and plant and animal species which are listed as endangered or critically endangered under NSW and Commonwealth legislation."@en ;
    skos:inScheme cs: ;
    skos:prefLabel "Central West subregion"@en ;
    skos:topConceptOf cs: ;
.

:Cooper-subregion
    a skos:Concept ;
    dcterms:created "2019-04-14"^^xsd:date ;
    dcterms:creator <https://linked.data.gov.au/org/neii> ;
    dcterms:modified "2020-09-29"^^xsd:date ;
    skos:broader :Lake-Eyre-Basin-bioregion ;
    skos:definition "The Cooper subregion spans south-west Queensland and north-east SA. It is part of the Lake Eyre Basin bioregion and adjoins the Galilee subregion in the north-east. Localities in this sparsely populated subregion include Innamincka, Cameron Corner and Moomba. Land is mainly used for cattle grazing of native and semi-natural pasture. The vegetation in this subregion is characterised by sparse shrubs, hummock grasses and scattered grassland. Groundwater is primarily used for livestock watering and by petroleum and conventional gas extraction industries. All of the rivers and lakes in this subregion are seasonal. Major streams include the Cooper Creek and the Thomson, Barcoo and Bulloo rivers. Significant nature conservation areas in this subregion encompass a number of protected areas and wetlands, including the internationally recognised Coongie Lakes and Lake Pinaroo. The Cooper subregion is home to a diverse range of plants and animals, including many that are listed as rare or threatened under Commonwealth and state government legislation."@en ;
    skos:inScheme cs: ;
    skos:prefLabel "Cooper subregion"@en ;
    skos:topConceptOf cs: ;
.

:EventsR0.2
    a skos:Concept ;
    dcterms:created "2019-04-14"^^xsd:date ;
    dcterms:creator <https://linked.data.gov.au/org/neii> ;
    dcterms:modified "2020-09-29"^^xsd:date ;
    skos:broader :hydrological-response-variable ;
    skos:definition "the mean annual number of events with a peak daily flow exceeding the threshold (the peak daily flow in flood events with a return period of 0.2 years as defined from modelled baseline flow in the reference period (1983 to 2012)). This metric is designed to be approximately representative of the number of overbench flow events in future 30-year periods. This is typically reported as the maximum change due to additional coal resource development."@en ;
    skos:inScheme cs: ;
    skos:prefLabel "EventsR0.2"@en ;
    skos:topConceptOf cs: ;
.

:EventsR0.3
    a skos:Concept ;
    dcterms:created "2019-04-14"^^xsd:date ;
    dcterms:creator <https://linked.data.gov.au/org/neii> ;
    dcterms:modified "2020-09-29"^^xsd:date ;
    skos:broader :hydrological-response-variable ;
    skos:definition "the mean annual number of events with a peak daily flow exceeding the threshold (the peak daily flow in flood events with a return period of 0.3 years as defined from modelled baseline flow in the reference period (1983 to 2012)). This metric is designed to be approximately representative of the number of overbench flow events in future 30-year periods. This is typically reported as the maximum change due to additional coal resource development."@en ;
    skos:inScheme cs: ;
    skos:prefLabel "EventsR0.3"@en ;
    skos:topConceptOf cs: ;
.

:EventsR2.0
    a skos:Concept ;
    dcterms:created "2019-04-14"^^xsd:date ;
    dcterms:creator <https://linked.data.gov.au/org/neii> ;
    dcterms:modified "2020-09-29"^^xsd:date ;
    skos:broader :hydrological-response-variable ;
    skos:definition "the mean annual number of events with a peak daily flow exceeding the threshold (the peak daily flow in flood events with a return period of 2.0 years as defined from modelled baseline flow in the reference period (1983 to 2012)). This metric is designed to be approximately representative of the number of overbank flow events in future 30-year periods. This is typically reported as the maximum change due to additional coal resource development."@en ;
    skos:inScheme cs: ;
    skos:prefLabel "EventsR2.0"@en ;
    skos:topConceptOf cs: ;
.

:EventsR3.0
    a skos:Concept ;
    dcterms:created "2019-04-14"^^xsd:date ;
    dcterms:creator <https://linked.data.gov.au/org/neii> ;
    dcterms:modified "2020-09-29"^^xsd:date ;
    skos:broader :hydrological-response-variable ;
    skos:definition "the mean annual number of events with a peak daily flow exceeding the threshold (the peak daily flow in flood events with a return period of 3.0 years as defined from modelled baseline flow in the reference period (1983 to 2012)). This metric is designed to be approximately representative of the number of overbank flow events in future 30-year periods. This is typically reported as the maximum change due to additional coal resource development."@en ;
    skos:inScheme cs: ;
    skos:prefLabel "EventsR3.0"@en ;
    skos:topConceptOf cs: ;
.

:Galilee-subregion
    a skos:Concept ;
    dcterms:created "2019-04-14"^^xsd:date ;
    dcterms:creator <https://linked.data.gov.au/org/neii> ;
    dcterms:modified "2020-09-29"^^xsd:date ;
    skos:broader :Lake-Eyre-Basin-bioregion ;
    skos:definition "The Galilee subregion is part of the Lake Eyre Basin bioregion and is entirely within Queensland. It extends westwards across the Great Dividing Range and into the Lake Eyre drainage basin. The subregion is sparsely populated, with most people living in towns and localities including Charleville, Barcaldine, Blackall and Hughenden. The subregion encompasses the headwaters of several major waterways including the Cooper Creek and the Diamantina, Belyando, Cape, Thomson, Barcoo, Flinders, Bulloo, and Warrego rivers. In addition to the river systems, the subregion has numerous wetlands, springs, waterholes and lakes, including the nationally important lakes Buchanan and Galilee. Some of these are home to diverse and unique plants and animals, many of which are listed as rare or threatened under Queensland and Commonwealth legislation. Native vegetation consists largely of grasslands in the west and open eucalyptus woodlands in the east. Cattle and sheep grazing on native pasture is the main land use and groundwater is of great importance."@en ;
    skos:inScheme cs: ;
    skos:prefLabel "Galilee subregion"@en ;
    skos:topConceptOf cs: ;
.

:Gloucester-subregion
    a skos:Concept ;
    dcterms:created "2019-04-14"^^xsd:date ;
    dcterms:creator <https://linked.data.gov.au/org/neii> ;
    dcterms:modified "2020-09-29"^^xsd:date ;
    skos:broader :Northern-Sydney-Basin-bioregion ;
    skos:definition "The Gloucester subregion covers an area of about 348 km². The Gloucester subregion is defined by the geological Gloucester Basin. It is located just north of the Hunter Valley in NSW, approximately 85 km north-north-east of Newcastle and relative to regional centres is 60 km south-west of Taree and 55 km west of Forster."@en ;
    skos:inScheme cs: ;
    skos:prefLabel "Gloucester subregion"@en ;
    skos:topConceptOf cs: ;
.

:Gwydir-subregion
    a skos:Concept ;
    dcterms:created "2019-04-14"^^xsd:date ;
    dcterms:creator <https://linked.data.gov.au/org/neii> ;
    dcterms:modified "2020-09-29"^^xsd:date ;
    skos:broader :Northern-Inland-Catchments-bioregion ;
    skos:definition "The Gwydir subregion includes parts of the northern Murray-Darling Basin in northern New South Wales and southern Queensland. The main rivers draining the subregion are the Gwydir and Macintyre-Barwon rivers. The subregion extends westward from the lower slopes of the New England Tablelands onto the low-lying riverine plains of the Barwon-Darling river system. Moree is the largest town in the subregion. Most of the land in the subregion is used for grazing and cropping. Groundwater is heavily used for irrigation of summer crops such as cotton. The subregion contains seasonal, semi-permanent and permanent wetlands and lagoons. This includes the Gwydir Wetlands, which is an internationally recognised and protected wetland. The subregion is home to a number of endangered water-dependent ecological communities, animals and plants which are protected under Commonwealth and New South Wales legislation."@en ;
    skos:inScheme cs: ;
    skos:prefLabel "Gwydir subregion"@en ;
    skos:topConceptOf cs: ;
.

:Hunter-subregion
    a skos:Concept ;
    dcterms:created "2019-04-14"^^xsd:date ;
    dcterms:creator <https://linked.data.gov.au/org/neii> ;
    dcterms:modified "2020-09-29"^^xsd:date ;
    skos:broader :Northern-Sydney-Basin-bioregion ;
    skos:definition "Along the coast, the Hunter subregion extends north from the northern edge of Broken Bay on the New South Wales Central Coast to just north of Newcastle. The subregion is bordered in the west and north-west by the Great Dividing Range and in the north by the towns of Scone and Muswellbrook. The Hunter River is the major river in the subregion, rising in the Barrington Tops and Liverpool Ranges and draining south-west to Lake Glenbawn before heading east where it enters the Tasman Sea at Newcastle. The subregion also includes smaller catchments along the central coast, including the Macquarie and Tuggerah lakes catchments."@en ;
    skos:inScheme cs: ;
    skos:prefLabel "Hunter subregion"@en ;
    skos:topConceptOf cs: ;
.

:LME
    a skos:Concept ;
    dcterms:created "2019-04-14"^^xsd:date ;
    dcterms:creator <https://linked.data.gov.au/org/neii> ;
    dcterms:modified "2020-09-29"^^xsd:date ;
    skos:broader :hydrological-response-variable ;
    skos:definition "the maximum length of spells (in days per year) with low flow, averaged over a 30-year period. This is typically reported as the maximum change due to additional coal resource development."@en ;
    skos:inScheme cs: ;
    skos:prefLabel "LME"@en ;
    skos:topConceptOf cs: ;
.

:Maranoa-Balonne-Condamine-subregion
    a skos:Concept ;
    dcterms:created "2019-04-14"^^xsd:date ;
    dcterms:creator <https://linked.data.gov.au/org/neii> ;
    dcterms:modified "2020-09-29"^^xsd:date ;
    skos:broader :Northern-Inland-Catchments-bioregion ;
    skos:definition "The Maranoa-Balonne-Condamine subregion is mainly within the Queensland part of the Murray-Darling Basin, with a small area in New South Wales. It includes the headwaters of the Condamine River and the Maranoa River as well as the floodplains of the Upper Darling Plains. The main cities and towns are Toowoomba, Warwick, Dalby, Chinchilla, Roma, St George and Goondiwindi. Most of the land is used for agriculture. Groundwater use varies across the subregion, but is commonly extracted for stock and domestic purposes, as well as for town water supply, agriculture and coal seam gas production. Wetlands in the subregion include seasonal, semi-permanent and permanent wetlands and lagoons. Some of these wetlands are nationally significant. The Culgoa River Floodplains and the Narran Lakes system are downstream of the subregion. The northern part of the Narran Lakes system is an internationally recognised and protected wetland. Two significant cultural sites are also downstream of the subregion and could be impacted by activities in the subregion. The subregion is home to a number of water-dependent ecological communities, animals and plants which are listed as threatened under Queensland and Commonwealth legislation."@en ;
    skos:inScheme cs: ;
    skos:prefLabel "Maranoa-Balonne-Condamine subregion"@en ;
    skos:topConceptOf cs: ;
.

:Namoi-subregion
    a skos:Concept ;
    dcterms:created "2019-04-14"^^xsd:date ;
    dcterms:creator <https://linked.data.gov.au/org/neii> ;
    dcterms:modified "2020-09-29"^^xsd:date ;
    skos:broader :Northern-Inland-Catchments-bioregion ;
    skos:definition "The Namoi subregion is located within the Murray-Darling Basin in central New South Wales. The subregion lies within the Namoi river basin, which includes the Namoi, Peel and Manilla rivers. However, the subregion being assessed is smaller than the Namoi river basin because the eastern part of the river basin does not overlie a coal-bearing geological basin. The largest towns in the subregion are Gunnedah, Narrabri and Walgett. The main surface water resource of the Namoi subregion is the Namoi River. There are three large dams that supply water to the subregion, of which Keepit Dam is the main water storage.  More than half of the water released from Keepit Dam and river inflow may be extracted for use for agriculture, towns and households. Of this, the great majority is used for agricultural irrigation. The landscape has been considerably altered since European settlement for agriculture. Significant volumes of groundwater are also used for agriculture (cropping). Across the subregion there are a number of water-dependent ecological communities, and plant and animal species that are listed as threatened under either Commonwealth or New South Wales legislation. The subregion also contains Lake Goran, a wetland of national importance, and sites of international importance for bird conservation."@en ;
    skos:inScheme cs: ;
    skos:prefLabel "Namoi subregion"@en ;
    skos:topConceptOf cs: ;
.

:P01
    a skos:Concept ;
    dcterms:created "2019-04-14"^^xsd:date ;
    dcterms:creator <https://linked.data.gov.au/org/neii> ;
    dcterms:modified "2020-09-29"^^xsd:date ;
    skos:broader :hydrological-response-variable ;
    skos:definition "the daily flow rate at the 1st percentile (ML/day). This is typically reported as the maximum change due to additional coal resource development over the 90-year period (from 2013 to 2102)."@en ;
    skos:inScheme cs: ;
    skos:prefLabel "P01"@en ;
    skos:topConceptOf cs: ;
.

:P99
    a skos:Concept ;
    dcterms:created "2019-04-14"^^xsd:date ;
    dcterms:creator <https://linked.data.gov.au/org/neii> ;
    dcterms:modified "2020-09-29"^^xsd:date ;
    skos:broader :hydrological-response-variable ;
    skos:definition "the daily flow rate at the 99th percentile (ML/day). This is typically reported as the maximum change due to additional coal resource development over the 90-year period (from 2013 to 2102)."@en ;
    skos:inScheme cs: ;
    skos:prefLabel "P99"@en ;
    skos:topConceptOf cs: ;
.

:QBFI
    a skos:Concept ;
    dcterms:created "2019-04-14"^^xsd:date ;
    dcterms:creator <https://linked.data.gov.au/org/neii> ;
    dcterms:modified "2020-09-29"^^xsd:date ;
    skos:broader :hydrological-response-variable ;
    skos:definition "ratio of total baseflow generation to total streamflow generation, averaged over a 30-year period. This is typically reported as the maximum change due to additional coal resource development."@en ;
    skos:inScheme cs: ;
    skos:prefLabel "QBFI"@en ;
    skos:topConceptOf cs: ;
.

:Yrs2tmaxRef
    a skos:Concept ;
    dcterms:created "2019-04-14"^^xsd:date ;
    dcterms:creator <https://linked.data.gov.au/org/neii> ;
    dcterms:modified "2020-09-29"^^xsd:date ;
    skos:definition "the difference between tmaxRef and the assessment year that is relevant for the prediction (2012, 2042 or 2102)"@en ;
    skos:inScheme cs: ;
    skos:prefLabel "Yrs2tmaxRef"@en ;
    skos:related :tmaxRef ;
    skos:topConceptOf cs: ;
.

:ZMA
    a skos:Concept ;
    dcterms:created "2019-04-14"^^xsd:date ;
    dcterms:creator <https://linked.data.gov.au/org/neii> ;
    dcterms:modified "2020-09-29"^^xsd:date ;
    skos:broader :hydrological-response-variable ;
    skos:definition "the maximum length of spells (in days per year) with zero flow over a 30-year period. This is typically reported as the maximum change due to additional coal resource development."@en ;
    skos:inScheme cs: ;
    skos:prefLabel "ZMA"@en ;
    skos:topConceptOf cs: ;
.

:ZME
    a skos:Concept ;
    dcterms:created "2019-04-14"^^xsd:date ;
    dcterms:creator <https://linked.data.gov.au/org/neii> ;
    dcterms:modified "2020-09-29"^^xsd:date ;
    skos:broader :hydrological-response-variable ;
    skos:definition "the maximum length of spells (in days per year) with zero flow, averaged over a 30-year period. This is typically reported as the maximum change due to additional coal resource development."@en ;
    skos:inScheme cs: ;
    skos:prefLabel "ZME"@en ;
    skos:topConceptOf cs: ;
.

:annual-flow
    a skos:Concept ;
    dcterms:created "2019-04-14"^^xsd:date ;
    dcterms:creator <https://linked.data.gov.au/org/neii> ;
    dcterms:modified "2020-09-28"^^xsd:date ;
    skos:altLabel "AF"@en ;
    skos:broader :hydrological-response-variable ;
    skos:definition "the volume of water that discharges past a specific point in a stream in a year, commonly measured in GL/year. This is typically reported as the maximum change due to additional coal resource development over the 90-year period (from 2013 to 2102)."@en ;
    skos:inScheme cs: ;
    skos:prefLabel "annual flow"@en ;
    skos:topConceptOf cs: ;
.

:asset-element
    a skos:Concept ;
    dcterms:created "2019-04-14"^^xsd:date ;
    dcterms:creator <https://linked.data.gov.au/org/neii> ;
    dcterms:modified "2020-09-28"^^xsd:date ;
    skos:definition "individual spatial features - points, lines and polygons - that describe an asset spatially"@en ;
    skos:inScheme cs: ;
    skos:prefLabel "asset element"@en ;
    skos:relatedMatch :asset ;
    skos:topConceptOf cs: ;
.

:at-minimal-risk-of-ecological-and-hydrological-changes
    a skos:Concept ;
    dcterms:created "2019-04-14"^^xsd:date ;
    dcterms:creator <https://linked.data.gov.au/org/neii> ;
    dcterms:modified "2020-09-29"^^xsd:date ;
    skos:definition "assessment units that overlap a landscape class are considered 'at minimal risk of ecological and hydrological changes' relative to other assessment units if modelled hydrological changes result in ecological changes that do not exceed the lower thresholds of risk. These bioregion-specific thresholds are based on expert opinion and are defined using receptor impact variables. Categorisation assists the rule-out process and in identifying where further local-scale assessment is warranted."@en ;
    skos:inScheme cs: ;
    skos:prefLabel "at minimal risk of ecological and hydrological changes"@en ;
    skos:related :assessment-unit ;
    skos:topConceptOf cs: ;
.

:at-some-risk-of-ecological-and-hydrological-changes
    a skos:Concept ;
    dcterms:created "2019-04-14"^^xsd:date ;
    dcterms:creator <https://linked.data.gov.au/org/neii> ;
    dcterms:modified "2020-09-29"^^xsd:date ;
    skos:definition "assessment units that overlap a landscape class are considered 'at some risk of ecological and hydrological changes' relative to other assessment units if modelled hydrological changes result in ecological changes that exceed the lower thresholds of risk but do not exceed the upper thresholds of risk. These bioregion-specific thresholds are based on expert opinion and are defined using receptor impact variables. Categorisation assists the rule-out process and in identifying where further local-scale assessment is warranted."@en ;
    skos:inScheme cs: ;
    skos:prefLabel "at some risk of ecological and hydrological changes"@en ;
    skos:related :assessment-unit ;
    skos:topConceptOf cs: ;
.

:baseflow-index
    a skos:Concept ;
    dcterms:created "2019-04-14"^^xsd:date ;
    dcterms:creator <https://linked.data.gov.au/org/neii> ;
    dcterms:modified "2020-09-28"^^xsd:date ;
    skos:definition "the ratio of baseflow to total streamflow over a long period of time (years)"@en ;
    skos:inScheme cs: ;
    skos:prefLabel "baseflow index"@en ;
    skos:related :baseflow ;
    skos:topConceptOf cs: ;
.

:bioregion
    a skos:Concept ;
    dcterms:created "2019-04-14"^^xsd:date ;
    dcterms:creator <https://linked.data.gov.au/org/neii> ;
    dcterms:modified "2020-09-29"^^xsd:date ;
    skos:definition "a geographic land area within which coal seam gas (CSG) and/or coal mining developments are taking place, or could take place, and for which bioregional assessments (BAs) are conducted"@en ;
    skos:inScheme cs: ;
    skos:prefLabel "bioregion"@en ;
    skos:related :Lake-Eyre-Basin-bioregion ;
    skos:topConceptOf cs: ;
.

:bore
    a skos:Concept ;
    dcterms:created "2019-04-14"^^xsd:date ;
    dcterms:creator <https://linked.data.gov.au/org/neii> ;
    dcterms:modified "2020-09-29"^^xsd:date ;
    skos:altLabel "borehole"@en ;
    skos:definition "a narrow, artificially constructed hole or cavity used to intercept, collect or store water from an aquifer, or to passively observe or collect groundwater information. Also known as a borehole or piezometer."@en ;
    skos:inScheme cs: ;
    skos:prefLabel "bore"@en ;
    skos:related :well ;
    skos:topConceptOf cs: ;
.

:dmax
    a skos:Concept ;
    dcterms:created "2019-04-14"^^xsd:date ;
    dcterms:creator <https://linked.data.gov.au/org/neii> ;
    dcterms:modified "2020-09-29"^^xsd:date ;
    skos:broader :hydrological-response-variable ;
    skos:definition "maximum difference in drawdown, obtained by choosing the maximum of the time series of differences between two futures. For example, to calculate the difference in drawdown between the coal resource development pathway (CRDP) and baseline, use the equations dmax = max (dCRDP(t) - dbaseline(t)) where d is drawdown, or dmax = max (hbaseline(t) - hCRDP(t)) where h is groundwater level and t is time."@en ;
    skos:inScheme cs: ;
    skos:prefLabel "dmax"@en ;
    skos:topConceptOf cs: ;
.

:dmaxRef
    a skos:Concept ;
    dcterms:created "2019-04-14"^^xsd:date ;
    dcterms:creator <https://linked.data.gov.au/org/neii> ;
    dcterms:modified "2020-09-29"^^xsd:date ;
    skos:broader :hydrological-response-variable ;
    skos:definition "maximum difference in drawdown under the baseline future or under the coal resource development pathway future relative to the reference period (1983 to 2012). This is typically reported as the maximum change due to additional coal resource development."@en ;
    skos:inScheme cs: ;
    skos:prefLabel "dmaxRef"@en ;
    skos:topConceptOf cs: ;
.

:ecosystem-asset
    a skos:Concept ;
    dcterms:created "2019-04-14"^^xsd:date ;
    dcterms:creator <https://linked.data.gov.au/org/neii> ;
    dcterms:modified "2020-09-29"^^xsd:date ;
    skos:definition "an ecosystem that may provide benefits to humanity. It is a spatial area comprising a combination of biotic and abiotic components and other elements which function together."@en ;
    skos:inScheme cs: ;
    skos:prefLabel "ecosystem asset"@en ;
    skos:related :landscape-class ;
    skos:topConceptOf cs: ;
.

:effect
    a skos:Concept ;
    dcterms:created "2019-04-14"^^xsd:date ;
    dcterms:creator <https://linked.data.gov.au/org/neii> ;
    dcterms:modified "2020-09-29"^^xsd:date ;
    skos:definition "for the purposes of Impact Modes and Effects Analysis (IMEA), change in the quantity and/or quality of surface water or groundwater. An effect is a specific type of an impact (any change resulting from prior events)."@en ;
    skos:inScheme cs: ;
    skos:prefLabel "effect"@en ;
    skos:related :impact ;
    skos:topConceptOf cs: ;
.

:groundwater-zone-of-potential-hydrological-change
    a skos:Concept ;
    dcterms:created "2019-04-14"^^xsd:date ;
    dcterms:creator <https://linked.data.gov.au/org/neii> ;
    dcterms:modified "2020-09-29"^^xsd:date ;
    skos:altLabel "GW zone"@en ;
    skos:broader :zone-of-potential-hydrological-change ;
    skos:definition "outside this extent, groundwater drawdown (and hence potential impacts) is very unlikely (less than 5% chance). It is the area with a greater than 5% chance of exceeding 0.2 m of drawdown due to additional coal resource development in the relevant aquifers."@en ;
    skos:inScheme cs: ;
    skos:prefLabel "groundwater zone of potential hydrological change"@en ;
    skos:topConceptOf cs: ;
.

:high-flow-days
    a skos:Concept ;
    dcterms:created "2019-04-14"^^xsd:date ;
    dcterms:creator <https://linked.data.gov.au/org/neii> ;
    dcterms:modified "2020-09-29"^^xsd:date ;
    skos:altLabel "FD"@en ;
    skos:broader :hydrological-response-variable ;
    skos:definition "the number of high-flow days per year. This is typically reported as the maximum change due to additional coal resource development over the 90-year period (from 2013 to 2102). The threshold for high-flow days is the 90th percentile from the simulated 90-year period. In some early products, this was referred to as 'flood days'."@en ;
    skos:inScheme cs: ;
    skos:prefLabel "high-flow days"@en ;
    skos:topConceptOf cs: ;
.

:impact
    a skos:Concept ;
    dcterms:created "2019-04-14"^^xsd:date ;
    dcterms:creator <https://linked.data.gov.au/org/neii> ;
    dcterms:modified "2020-09-29"^^xsd:date ;
    skos:definition "a change resulting from prior events, at any stage in a chain of events or a causal pathway. An impact might be equivalent to an effect (change in the quality and/or quantity of surface water or groundwater), or it might be a change resulting from those effects (for example, ecological changes that result from hydrological changes)."@en ;
    skos:inScheme cs: ;
    skos:prefLabel "impact"@en ;
    skos:related :effect ;
    skos:topConceptOf cs: ;
.

:interquartile-range
    a skos:Concept ;
    dcterms:created "2019-04-14"^^xsd:date ;
    dcterms:creator <https://linked.data.gov.au/org/neii> ;
    dcterms:modified "2020-09-29"^^xsd:date ;
    skos:altLabel "IQR"@en ;
    skos:broader :hydrological-response-variable ;
    skos:definition "the interquartile range in daily flow (ML/day); that is, the difference between the daily flow rate at the 75th percentile and at the 25th percentile. This is typically reported as the maximum change due to additional coal resource development over the 90-year period (from 2013 to 2102)."@en ;
    skos:inScheme cs: ;
    skos:prefLabel "interquartile range"@en ;
    skos:topConceptOf cs: ;
.

:landscape-group
    a skos:Concept ;
    dcterms:created "2019-04-14"^^xsd:date ;
    dcterms:creator <https://linked.data.gov.au/org/neii> ;
    dcterms:modified "2020-09-29"^^xsd:date ;
    skos:definition "for the purposes of bioregional assessments (BAs), a set of landscape classes grouped together based on common ecohydrological characteristics that are relevant for analysis purposes"@en ;
    skos:inScheme cs: ;
    skos:prefLabel "landscape group"@en ;
    skos:related :landscape-class ;
    skos:topConceptOf cs: ;
.

:length-of-low-flow-spell
    a skos:Concept ;
    dcterms:created "2019-04-14"^^xsd:date ;
    dcterms:creator <https://linked.data.gov.au/org/neii> ;
    dcterms:modified "2020-09-29"^^xsd:date ;
    skos:altLabel "LLFS"@en ;
    skos:broader :hydrological-response-variable ;
    skos:definition "the length (days) of the longest low-flow spell each year. This is typically reported as the maximum change due to additional coal resource development over the 90-year period (from 2013 to 2102)."@en ;
    skos:inScheme cs: ;
    skos:prefLabel "length of low-flow spell"@en ;
    skos:topConceptOf cs: ;
.

:low-flow-days
    a skos:Concept ;
    dcterms:created "2019-04-14"^^xsd:date ;
    dcterms:creator <https://linked.data.gov.au/org/neii> ;
    dcterms:modified "2020-09-29"^^xsd:date ;
    skos:altLabel "LFD"@en ;
    skos:broader :hydrological-response-variable ;
    skos:definition "the number of low-flow days per year. This is typically reported as the maximum change due to additional coal resource development over the 90-year period (from 2013 to 2102). The threshold for low-flow days is the 10th percentile from the simulated 90-year period."@en ;
    skos:inScheme cs: ;
    skos:prefLabel "low-flow days"@en ;
    skos:topConceptOf cs: ;
.

:low-flow-days-averaged-over-30-years
    a skos:Concept ;
    dcterms:created "2019-04-14"^^xsd:date ;
    dcterms:creator <https://linked.data.gov.au/org/neii> ;
    dcterms:modified "2020-09-29"^^xsd:date ;
    skos:altLabel "LQD"@en ;
    skos:broader :hydrological-response-variable ;
    skos:definition "the number of days per year with low flow (<10 ML/day), averaged over a 30-year period. This is typically reported as the maximum change due to additional coal resource development."@en ;
    skos:inScheme cs: ;
    skos:prefLabel "low-flow days (averaged over 30 years)"@en ;
    skos:topConceptOf cs: ;
.

:low-flow-spells
    a skos:Concept ;
    dcterms:created "2019-04-14"^^xsd:date ;
    dcterms:creator <https://linked.data.gov.au/org/neii> ;
    dcterms:modified "2020-09-29"^^xsd:date ;
    skos:broader :hydrological-response-variable ;
    skos:definition "the number of low-flow spells per year. This is typically reported as the maximum change due to additional coal resource development over the 90-year period (from 2013 to 2102). A spell is defined as a period of contiguous days of flow below the 10th percentile threshold."@en ;
    skos:inScheme cs: ;
    skos:prefLabel "low-flow spells"@en ;
    skos:topConceptOf cs: ;
.

:mine-exclusion-zone
    a skos:Concept ;
    dcterms:created "2019-04-14"^^xsd:date ;
    dcterms:creator <https://linked.data.gov.au/org/neii> ;
    dcterms:modified "2020-09-29"^^xsd:date ;
    skos:definition "areas in the zone of potential hydrological change that are within or near open-cut mine pits or underground mine workings, and where (i) modelled drawdowns are highly uncertain due to the very steep hydraulic gradients at the mine pit interface; (ii) changes in the drawdown are inevitable where the mine pit intersects the regional watertable; (iii) other factors, such as physical removal of a wetland or creek, may have a larger impact on a landscape class than the predicted decrease in groundwater level; and (iv) impacts are predominantly site-scale, assumed to be adequately addressed through existing development approval processes, and hence not the primary focus of bioregional assessments. The modelled estimates of drawdown in the mine exclusion zone are considered unreliable for use in the receptor impact modelling."@en ;
    skos:inScheme cs: ;
    skos:prefLabel "mine exclusion zone"@en ;
    skos:related :drawdown ;
    skos:topConceptOf cs: ;
.

:mine-pit-exclusion-zone
    a skos:Concept ;
    dcterms:created "2019-04-14"^^xsd:date ;
    dcterms:creator <https://linked.data.gov.au/org/neii> ;
    dcterms:modified "2020-09-29"^^xsd:date ;
    skos:definition "areas in the zone of potential hydrological change that are within or near open-cut mine pits, and where (i) modelled drawdowns are highly uncertain due to the very steep hydraulic gradients at the mine pit interface; (ii) changes in the drawdown are inevitable where the mine pit intersects the regional watertable; (iii) other factors, such as physical removal of a wetland or creek, may have a larger impact on a landscape class than the predicted decrease in groundwater level; and (iv) impacts are predominantly site-scale, assumed to be adequately addressed through existing development approval processes, and hence not the primary focus of bioregional assessments. The modelled estimates of drawdown in the mine pit exclusion zone are considered unreliable for use in the receptor impact modelling."@en ;
    skos:inScheme cs: ;
    skos:prefLabel "mine pit exclusion zone"@en ;
    skos:related :drawdown ;
    skos:topConceptOf cs: ;
.

:surface-water-zone-of-potential-hydrological-change
    a skos:Concept ;
    dcterms:created "2019-04-14"^^xsd:date ;
    dcterms:creator <https://linked.data.gov.au/org/neii> ;
    dcterms:modified "2020-09-29"^^xsd:date ;
    skos:altLabel "SW zone"@en ;
    skos:broader :zone-of-potential-hydrological-change ;
    skos:definition "outside this extent, changes in surface water hydrological response variables due to additional coal resource development (and hence potential impacts) are very unlikely (less than 5% chance). The area contains those river reaches where a change in any one of nine surface water hydrological response variables exceeds the specified thresholds. For the four flux-based hydrological response variables (annual flow (AF), daily flow rate at the 99th percentile (P99), interquartile range (IQR) and daily flow rate at the 1st percentile (P01)), the threshold is a 5% chance of a 1% change in the variable. That is, if 5% or more of model runs show a maximum change in results under coal resource development pathway (CRDP) of 1% relative to baseline. For four of the frequency-based hydrological response variables (high-flow days (FD), low-flow days (LFD), length of longest low-flow spell (LLFS) and zero-flow days (ZFD)), the threshold is a 5% chance of a change of 3 days per year. For the final frequency-based hydrological response variable (low-flow spells (LFS)), the threshold is a 5% chance of a change of 2 spells per year."@en ;
    skos:inScheme cs: ;
    skos:prefLabel "surface water zone of potential hydrological change"@en ;
    skos:topConceptOf cs: ;
.

:tmax
    a skos:Concept ;
    dcterms:created "2019-04-14"^^xsd:date ;
    dcterms:creator <https://linked.data.gov.au/org/neii> ;
    dcterms:modified "2020-09-29"^^xsd:date ;
    skos:broader :hydrological-response-variable ;
    skos:definition "year of maximum change"@en ;
    skos:inScheme cs: ;
    skos:prefLabel "tmax"@en ;
    skos:topConceptOf cs: ;
.

:water-dependent-asset
    a skos:Concept ;
    dcterms:created "2019-04-14"^^xsd:date ;
    dcterms:creator <https://linked.data.gov.au/org/neii> ;
    dcterms:modified "2020-09-29"^^xsd:date ;
    skos:definition "an asset potentially impacted, either positively or negatively, by changes in the groundwater and/or surface water regime due to coal resource development"@en ;
    skos:inScheme cs: ;
    skos:prefLabel "water-dependent asset"@en ;
    skos:related :receptor-impact-model ;
    skos:topConceptOf cs: ;
.

:water-system
    a skos:Concept ;
    dcterms:created "2019-04-14"^^xsd:date ;
    dcterms:creator <https://linked.data.gov.au/org/neii> ;
    dcterms:modified "2020-09-28"^^xsd:date ;
    skos:definition "a system that is hydrologically connected and described at the level desired for management purposes (e.g. subcatchment, catchment, basin or drainage division, or groundwater management unit, subaquifer, aquifer, groundwater basin)"@en ;
    skos:inScheme cs: ;
    skos:prefLabel "water system"@en ;
    skos:related :baseflow ;
    skos:topConceptOf cs: ;
.

:well
    a skos:Concept ;
    dcterms:created "2019-04-14"^^xsd:date ;
    dcterms:creator <https://linked.data.gov.au/org/neii> ;
    dcterms:modified "2020-09-29"^^xsd:date ;
    skos:definition "typically a narrow diameter hole drilled into the earth for the purposes of exploring, evaluating or recovering various natural resources, such as hydrocarbons (oil and gas) or water. As part of the drilling and construction process the well can be encased by materials such as steel and cement, or it may be uncased. Wells are sometimes known as a 'wellbore'."@en ;
    skos:inScheme cs: ;
    skos:prefLabel "well"@en ;
    skos:related :bore ;
    skos:topConceptOf cs: ;
.

:zero-flow-days
    a skos:Concept ;
    dcterms:created "2019-04-14"^^xsd:date ;
    dcterms:creator <https://linked.data.gov.au/org/neii> ;
    dcterms:modified "2020-09-29"^^xsd:date ;
    skos:altLabel "ZFD"@en ;
    skos:broader :hydrological-response-variable ;
    skos:definition "the number of zero-flow days per year. This is typically reported as the maximum change due to additional coal resource development over the 90-year period (from 2013 to 2102)."@en ;
    skos:inScheme cs: ;
    skos:prefLabel "zero-flow days"@en ;
    skos:topConceptOf cs: ;
.

:zero-flow-days-averaged-over-30-years
    a skos:Concept ;
    dcterms:created "2019-04-14"^^xsd:date ;
    dcterms:creator <https://linked.data.gov.au/org/neii> ;
    dcterms:modified "2020-09-29"^^xsd:date ;
    skos:altLabel "ZQD"@en ;
    skos:broader :hydrological-response-variable ;
    skos:definition "the number of zero-flow days per year, averaged over a 30-year period. This is typically reported as the maximum change due to additional coal resource development."@en ;
    skos:inScheme cs: ;
    skos:prefLabel "zero-flow days (averaged over 30 years)"@en ;
    skos:topConceptOf cs: ;
.

:Northern-Sydney-Basin-bioregion
    a skos:Concept ;
    dcterms:created "2019-04-14"^^xsd:date ;
    dcterms:creator <https://linked.data.gov.au/org/neii> ;
    dcterms:modified "2020-09-29"^^xsd:date ;
    skos:definition "The Northern Sydney Basin bioregion is located south-east of the Great Dividing Range and is entirely within NSW. It adjoins the Northern Inland Catchments bioregion in the north-west. This bioregion contains two subregions: the Gloucester and Hunter subregions, within the Hunter Central Rivers natural resource management region."@en ;
    skos:inScheme cs: ;
    skos:narrower
        :Gloucester-subregion ,
        :Hunter-subregion ;
    skos:prefLabel "Northern Sydney Basin bioregion"@en ;
    skos:topConceptOf cs: ;
.

:additional-drawdown
    a skos:Concept ;
    dcterms:created "2019-04-14"^^xsd:date ;
    dcterms:creator <https://linked.data.gov.au/org/neii> ;
    dcterms:modified "2020-09-29"^^xsd:date ;
    skos:altLabel "drawdown due to additional coal resource development"@en ;
    skos:definition "the maximum difference in drawdown (dmax) between the coal resource development pathway (CRDP) and baseline, due to additional coal resource development"@en ;
    skos:inScheme cs: ;
    skos:prefLabel "additional drawdown"@en ;
    skos:related
        :baseline-coal-resource-development ,
        :coal-resource-development-pathway ;
    skos:topConceptOf cs: ;
.

:assessment-extent
    a skos:Concept ;
    dcterms:created "2019-04-14"^^xsd:date ;
    dcterms:creator <https://linked.data.gov.au/org/neii> ;
    dcterms:modified "2020-09-29"^^xsd:date ;
    skos:definition "the geographic area associated with a subregion or bioregion in which the potential water-related impact of coal resource development on assets is assessed. The assessment extent is created by revising the preliminary assessment extent on the basis of information from Component 1: Contextual information and Component 2: Model-data analysis."@en ;
    skos:inScheme cs: ;
    skos:prefLabel "assessment extent"@en ;
    skos:related :preliminary-assessment-extent ;
    skos:relatedMatch :preliminary-assessment-extent ;
    skos:topConceptOf cs: ;
.

:asset
    a skos:Concept ;
    dcterms:created "2019-04-14"^^xsd:date ;
    dcterms:creator <https://linked.data.gov.au/org/neii> ;
    dcterms:modified "2020-09-29"^^xsd:date ;
    skos:definition "an entity that has value to the community and, for bioregional assessment purposes, is associated with a subregion or bioregion. Technically, an asset is a store of value and may be managed and/or used to maintain and/or produce further value. Each asset will have many values associated with it and they can be measured from a range of perspectives; for example, the values of a wetland can be measured from ecological, sociocultural and economic perspectives."@en ;
    skos:inScheme cs: ;
    skos:prefLabel "asset"@en ;
    skos:related :more-at-risk-of-hydrological-changes ;
    skos:relatedMatch :asset-element ;
    skos:topConceptOf cs: ;
.

:baseflow
    a skos:Concept ;
    dcterms:created "2019-04-14"^^xsd:date ;
    dcterms:creator <https://linked.data.gov.au/org/neii> ;
    dcterms:modified "2020-09-28"^^xsd:date ;
    skos:definition "the portion of streamflow that comes from shallow and deep subsurface flow, and is an important part of the groundwater system"@en ;
    skos:inScheme cs: ;
    skos:prefLabel "baseflow"@en ;
    skos:related
        :baseflow-index ,
        :water-system ;
    skos:topConceptOf cs: ;
.

:baseline-drawdown
    a skos:Concept ;
    dcterms:created "2019-04-14"^^xsd:date ;
    dcterms:creator <https://linked.data.gov.au/org/neii> ;
    dcterms:modified "2020-09-29"^^xsd:date ;
    skos:altLabel "drawdown under the baseline"@en ;
    skos:definition "the maximum difference in drawdown (dmax) under the baseline relative to no coal resource development"@en ;
    skos:inScheme cs: ;
    skos:prefLabel "baseline drawdown"@en ;
    skos:related
        :baseline-coal-resource-development ,
        :coal-resource-development-pathway ;
    skos:topConceptOf cs: ;
.

:more-at-risk-of-ecological-and-hydrological-changes
    a skos:Concept ;
    dcterms:created "2019-04-14"^^xsd:date ;
    dcterms:creator <https://linked.data.gov.au/org/neii> ;
    dcterms:modified "2020-09-29"^^xsd:date ;
    skos:definition "assessment units that overlap a landscape class are considered 'more at risk of ecological and hydrological changes' relative to other assessment units if modelled hydrological changes result in ecological changes that exceed the upper thresholds of risk. These bioregion-specific thresholds are based on expert opinion and are defined using receptor impact variables. Categorisation assists the rule-out process and in identifying where further local-scale assessment is warranted."@en ;
    skos:inScheme cs: ;
    skos:prefLabel "more at risk of ecological and hydrological changes"@en ;
    skos:related
        :assessment-unit ,
        :landscape-class ;
    skos:topConceptOf cs: ;
.

:preliminary-assessment-extent
    a skos:Concept ;
    dcterms:created "2019-04-14"^^xsd:date ;
    dcterms:creator <https://linked.data.gov.au/org/neii> ;
    dcterms:modified "2020-09-29"^^xsd:date ;
    skos:altLabel "PAE"@en ;
    skos:definition "the geographic area associated with a subregion or bioregion in which the potential water-related impact of coal resource development on assets is assessed. The PAE is estimated at the beginning of a bioregional assessment, and is updated to the 'assessment extent' on the basis of information from Component 1: Contextual information and Component 2: Model-data analysis."@en ;
    skos:inScheme cs: ;
    skos:prefLabel "preliminary assessment extent"@en ;
    skos:related :assessment-extent ;
    skos:relatedMatch :assessment-extent ;
    skos:topConceptOf cs: ;
.

:tmaxRef
    a skos:Concept ;
    dcterms:created "2019-04-14"^^xsd:date ;
    dcterms:creator <https://linked.data.gov.au/org/neii> ;
    dcterms:modified "2020-09-29"^^xsd:date ;
    skos:broader :hydrological-response-variable ;
    skos:definition "the year that the maximum difference in drawdown relative to the reference period (1983 to 2012) (dmaxRef) occurs"@en ;
    skos:inScheme cs: ;
    skos:prefLabel "tmaxRef"@en ;
    skos:related :Yrs2tmaxRef ;
    skos:topConceptOf cs: ;
.

:zone-of-potential-hydrological-change
    a skos:Concept ;
    dcterms:created "2019-04-14"^^xsd:date ;
    dcterms:creator <https://linked.data.gov.au/org/neii> ;
    dcterms:modified "2020-09-29"^^xsd:date ;
    skos:definition "outside this extent, hydrological changes (and hence potential impacts) are very unlikely (less than 5% chance). Each bioregional assessment defines the zone of potential hydrological change using probabilities of exceeding thresholds for relevant hydrological response variables. The zone of potential hydrological change is the union of the groundwater zone of potential hydrological change (the area with a greater than 5% chance of exceeding 0.2 m of drawdown due to additional coal resource development in the relevant aquifers) and the surface water zone of potential hydrological change (the area with a greater than 5% chance of exceeding changes in relevant surface water hydrological response variables due to additional coal resource development)."@en ;
    skos:inScheme cs: ;
    skos:narrower
        :groundwater-zone-of-potential-hydrological-change ,
        :surface-water-zone-of-potential-hydrological-change ;
    skos:prefLabel "zone of potential hydrological change"@en ;
    skos:topConceptOf cs: ;
.

:Lake-Eyre-Basin-bioregion
    a skos:Concept ;
    dcterms:created "2019-04-14"^^xsd:date ;
    dcterms:creator <https://linked.data.gov.au/org/neii> ;
    dcterms:modified "2020-09-29"^^xsd:date ;
    skos:definition "The Lake Eyre Basin bioregion covers an area of about 1.31 million square kilometres of central and north-eastern Australia, which is almost one-sixth of the country. It extends across parts of Queensland, SA, NSW and the NT and incorporates the whole of the Lake Eyre drainage basin. The bioregion was selected for assessment because of the likelihood of coal seam gas and coal mining development and the potential for water-dependent impacts on the environment and other industries that use water such as agriculture."@en ;
    skos:inScheme cs: ;
    skos:narrower
        :Cooper-subregion ,
        :Galilee-subregion ;
    skos:prefLabel "Lake Eyre Basin bioregion"@en ;
    skos:related :bioregion ;
    skos:topConceptOf cs: ;
.

:baseline-coal-resource-development
    a skos:Concept ;
    dcterms:created "2019-04-14"^^xsd:date ;
    dcterms:creator <https://linked.data.gov.au/org/neii> ;
    dcterms:modified "2020-09-29"^^xsd:date ;
    skos:altLabel "baseline"@en ;
    skos:definition "a future that includes all coal mines and coal seam gas (CSG) fields that are commercially producing as of December 2012"@en ;
    skos:inScheme cs: ;
    skos:prefLabel "baseline coal resource development"@en ;
    skos:related
        :additional-drawdown ,
        :baseline-drawdown ,
        :drawdown ;
    skos:topConceptOf cs: ;
.

:coal-resource-development-pathway
    a skos:Concept ;
    dcterms:created "2019-04-14"^^xsd:date ;
    dcterms:creator <https://linked.data.gov.au/org/neii> ;
    dcterms:modified "2020-09-29"^^xsd:date ;
    skos:altLabel "CRDP"@en ;
    skos:definition "a future that includes all coal mines and coal seam gas (CSG) fields that are in the baseline as well as those that are expected to begin commercial production after December 2012"@en ;
    skos:inScheme cs: ;
    skos:prefLabel "coal resource development pathway"@en ;
    skos:related
        :additional-drawdown ,
        :baseline-drawdown ,
        :drawdown ;
    skos:topConceptOf cs: ;
.

:more-at-risk-of-hydrological-changes
    a skos:Concept ;
    dcterms:created "2019-04-14"^^xsd:date ;
    dcterms:creator <https://linked.data.gov.au/org/neii> ;
    dcterms:modified "2020-09-29"^^xsd:date ;
    skos:definition "assessment units that overlap an asset are considered 'more at risk of hydrological changes' relative to other assessment units if modelled hydrological changes exceed bioregion-specific thresholds of risk. These thresholds are based on expert opinion and are defined using hydrological response variables. Categorisation assists the rule-out process and identifying where further local-scale assessment is warranted."@en ;
    skos:inScheme cs: ;
    skos:prefLabel "more at risk of hydrological changes"@en ;
    skos:related
        :assessment-unit ,
        :asset ,
        :hydrological-response-variable ;
    skos:topConceptOf cs: ;
.

:receptor-impact-model
    a skos:Concept ;
    dcterms:created "2019-04-14"^^xsd:date ;
    dcterms:creator <https://linked.data.gov.au/org/neii> ;
    dcterms:modified "2020-09-29"^^xsd:date ;
    skos:definition "a function that translates hydrological changes into the distribution or range of potential ecosystem outcomes that may arise from those changes. Within bioregional assessments, hydrological changes are described by hydrological response variables, ecosystem outcomes are described by receptor impact variables, and a receptor impact model determines the relationship between a particular receptor impact variable and one or more hydrological response variables. Receptor impact models are relevant to specific landscape classes, and play a crucial role in quantifying potential impacts for ecological water-dependent assets that are within the landscape class. In the broader scientific literature receptor impact models are often known as 'ecological response functions'."@en ;
    skos:inScheme cs: ;
    skos:prefLabel "receptor impact model"@en ;
    skos:related
        :hydrological-response-variable ,
        :landscape-class ,
        :water-dependent-asset ;
    skos:topConceptOf cs: ;
.

:Northern-Inland-Catchments-bioregion
    a skos:Concept ;
    dcterms:created "2019-04-14"^^xsd:date ;
    dcterms:creator <https://linked.data.gov.au/org/neii> ;
    dcterms:modified "2020-09-29"^^xsd:date ;
    skos:definition "The Northern Inland Catchments bioregion is located west of the Great Dividing Range in eastern Australia and includes parts of the northern Murray-Darling Basin in northern New South Wales and southern Queensland. The Northern Inland Catchments bioregion adjoins the Clarence-Moreton bioregion in the north-east, and the Northern Sydney Basin bioregion in the south. The bioregion was selected for assessment because of the likely coal seam gas and coal mining development and the potential for water dependent impacts on the environment and other water-using industries such as agriculture. The Northern Inland Catchments bioregion includes four subregions: the Maranoa-Balonne-Condamine, Gwydir, Namoi and Central West subregions. The subregion boundaries follow river basin boundaries, but only include areas that have the types of rocks known to contain coal and coal seam gas. Some water resources outside the Northern Inland Catchments bioregion that may potentially be impacted as a result of coal and coal seam gas development in the Northern Inland Catchments bioregion will also be considered in the assessment."@en ;
    skos:inScheme cs: ;
    skos:narrower
        :Central-West-subregion ,
        :Gwydir-subregion ,
        :Maranoa-Balonne-Condamine-subregion ,
        :Namoi-subregion ;
    skos:prefLabel "Northern Inland Catchments bioregion"@en ;
    skos:topConceptOf cs: ;
.

:assessment-unit
    a skos:Concept ;
    dcterms:created "2019-04-14"^^xsd:date ;
    dcterms:creator <https://linked.data.gov.au/org/neii> ;
    dcterms:modified "2020-09-29"^^xsd:date ;
    skos:definition "for the purposes of impact analysis, a geographic area that is used to partition the entire assessment extent into square polygons that do not overlap. The spatial resolution of the assessment units is closely related to that of the bioregional assessment groundwater modelling and is, typically, 1 x 1 km. Each assessment unit has a unique identifier. The partitioned data can be combined and recombined into any aggregation supported by the conceptual modelling, causal pathways and model data."@en ;
    skos:inScheme cs: ;
    skos:prefLabel "assessment unit"@en ;
    skos:related
        :at-minimal-risk-of-ecological-and-hydrological-changes ,
        :at-some-risk-of-ecological-and-hydrological-changes ,
        :more-at-risk-of-ecological-and-hydrological-changes ,
        :more-at-risk-of-hydrological-changes ;
    skos:topConceptOf cs: ;
.

:drawdown
    a skos:Concept ;
    dcterms:created "2019-04-14"^^xsd:date ;
    dcterms:creator <https://linked.data.gov.au/org/neii> ;
    dcterms:modified "2020-09-29"^^xsd:date ;
    skos:definition "a lowering of the groundwater level (caused, for example, by pumping). In the bioregional assessment (BA) context this is reported as the difference in groundwater level between two potential futures considered in BAs: baseline coal resource development (baseline) and the coal resource development pathway (CRDP). The difference in drawdown between CRDP and baseline is due to the additional coal resource development (ACRD). Drawdown under the baseline is relative to drawdown with no coal resource development; likewise, drawdown under the CRDP is relative to drawdown with no coal resource development."@en ;
    skos:inScheme cs: ;
    skos:prefLabel "drawdown"@en ;
    skos:related
        :baseline-coal-resource-development ,
        :coal-resource-development-pathway ,
        :mine-exclusion-zone ,
        :mine-pit-exclusion-zone ;
    skos:topConceptOf cs: ;
.

:landscape-class
    a skos:Concept ;
    dcterms:created "2019-04-14"^^xsd:date ;
    dcterms:creator <https://linked.data.gov.au/org/neii> ;
    dcterms:modified "2020-09-29"^^xsd:date ;
    skos:definition "for bioregional assessment (BA) purposes, an ecosystem with characteristics that are expected to respond similarly to changes in groundwater and/or surface water due to coal resource development. Note that there is expected to be less heterogeneity in the response within a landscape class than between landscape classes. They are present on the landscape across the entire BA subregion or bioregion and their spatial coverage is exhaustive and non-overlapping. Conceptually, landscape classes can be considered as types of ecosystem assets."@en ;
    skos:inScheme cs: ;
    skos:prefLabel "landscape class"@en ;
    skos:related
        :ecosystem-asset ,
        :landscape-group ,
        :more-at-risk-of-ecological-and-hydrological-changes ,
        :receptor-impact-model ;
    skos:topConceptOf cs: ;
.

:hydrological-response-variable
    a skos:Concept ;
    dcterms:created "2019-04-14"^^xsd:date ;
    dcterms:creator <https://linked.data.gov.au/org/neii> ;
    dcterms:modified "2020-09-29"^^xsd:date ;
    skos:definition "a hydrological characteristic of the system that potentially changes due to coal resource development (for example, drawdown or the annual flow volume)"@en ;
    skos:inScheme cs: ;
    skos:narrower
        :EventsR0.2 ,
        :EventsR0.3 ,
        :EventsR2.0 ,
        :EventsR3.0 ,
        :LME ,
        :P01 ,
        :P99 ,
        :QBFI ,
        :ZMA ,
        :ZME ,
        :annual-flow ,
        :dmax ,
        :dmaxRef ,
        :high-flow-days ,
        :interquartile-range ,
        :length-of-low-flow-spell ,
        :low-flow-days ,
        :low-flow-days-averaged-over-30-years ,
        :low-flow-spells ,
        :tmax ,
        :tmaxRef ,
        :zero-flow-days ,
        :zero-flow-days-averaged-over-30-years ;
    skos:prefLabel "hydrological response variable"@en ;
    skos:related
        :more-at-risk-of-hydrological-changes ,
        :receptor-impact-model ;
    skos:topConceptOf cs: ;
.

<https://linked.data.gov.au/org/neii>
    a
        dcterms:Agent ,
        schema:Organization ;
    schema:name "National Environmental Information Infrastructure" ;
    schema:url "http://www.bom.gov.au/environment/transition.shtml"^^xsd:anyURI ;
.

cs:
    a skos:ConceptScheme ;
    dcterms:created "2019-04-12"^^xsd:date ;
    dcterms:creator <https://linked.data.gov.au/org/neii> ;
    dcterms:issued "2019-04-15" ;
    dcterms:modified "2024-04-15"^^xsd:date ;
    dcterms:publisher <https://linked.data.gov.au/org/bap> ;
    dcterms:subject "Bioregional Assessment Programme"@en ;
    owl:deprecated true ;
    owl:versionInfo "Version 1" ;
    skos:definition "Terms and definitions used in technical products in the Bioregional Assessment Programme, a collaboration between the Australian Government Department of the Environment and Energy, the Bureau of Meteorology, CSIRO and Geoscience Australia. See http://www.bioregionalassessment.gov.au for more information about the Programme. "@en ;
    skos:hasTopConcept
        :BA-metadata-quality-assurance-process ,
        :BADMS-compliant-metadata ,
        :Bioregional-Assessment-Data-Store ,
        :Bioregional-Assessment-Metadata-Catalogue ,
        :Bioregional-Assessment-Repository ,
        :Central-West-subregion ,
        :Clarence-Moreton-bioregion ,
        :Cooper-subregion ,
        :Element-Conformance-Report ,
        :EventsR0.2 ,
        :EventsR0.3 ,
        :EventsR2.0 ,
        :EventsR3.0 ,
        :Ferrosols ,
        :Galilee-subregion ,
        :Geofabric ,
        :Gloucester-subregion ,
        :Gwydir-subregion ,
        :Hunter-subregion ,
        :Impact-Modes-and-Effects-Analysis ,
        :Joint-Ore-Reserves-Committee-Code ,
        :Kurosols ,
        :LME ,
        :Lake-Eyre-Basin-bioregion ,
        :Maranoa-Balonne-Condamine-subregion ,
        :Markov-chain-Monte-Carlo-methods ,
        :Metadata-Record-Coordinator ,
        :Monte-Carlo-simulation ,
        :Namoi-subregion ,
        :Northern-Inland-Catchments-bioregion ,
        :Northern-Sydney-Basin-bioregion ,
        :P01 ,
        :P99 ,
        :QBFI ,
        :R0.2 ,
        :R0.3 ,
        :R2.0 ,
        :R3.0 ,
        :Repository-website ,
        :Rudosols ,
        :Sodosols ,
        :Tenosols ,
        :Vertosols ,
        :Yrs2tmaxRef ,
        :ZMA ,
        :ZME ,
        :activity ,
        :additional-coal-resource-development ,
        :additional-drawdown ,
        :advanced-exploration ,
        :amax ,
        :analysis-domain-extent ,
        :analysis-extent ,
        :analytic-element-model ,
        :annual-flow ,
        :aquifer ,
        :aquitard ,
        :artesian-aquifer ,
        :assessment-extent ,
        :assessment-unit ,
        :asset ,
        :asset-element ,
        :asset-identifier ,
        :asset-name ,
        :at-minimal-risk-of-ecological-and-hydrological-changes ,
        :at-some-risk-of-ecological-and-hydrological-changes ,
        :baseflow ,
        :baseflow-index ,
        :baseline-coal-resource-development ,
        :baseline-drawdown ,
        :basement ,
        :bioregion ,
        :bioregional-assessment ,
        :bore ,
        :brownfield-exploration ,
        :causal-pathway ,
        :coal-deposit ,
        :coal-grade ,
        :coal-resource-development-pathway ,
        :coalification ,
        :coking-coal ,
        :component ,
        :conceptual-model ,
        :confined-aquifer ,
        :connectivity ,
        :consequence ,
        :context ,
        :cumulative-impact ,
        :current-controls ,
        :data-files-owner ,
        :dataset ,
        :dataset-granularity ,
        :dataset-title ,
        :deposit-evaluation ,
        :depressurisation ,
        :derived-dataset ,
        :detection-score ,
        :dewatering ,
        :direct-impact ,
        :discharge ,
        :diversion ,
        :dmax ,
        :dmaxRef ,
        :drawdown ,
        :ecosystem ,
        :ecosystem-asset ,
        :ecosystem-function ,
        :effect ,
        :ephemeral-stream ,
        :extraction ,
        :fairway ,
        :fecundity ,
        :focal-analysis-extent ,
        :foreland-basin ,
        :formation ,
        :fractile ,
        :geological-formation ,
        :globally-unique-identifier ,
        :goaf ,
        :grass-roots-exploration ,
        :groundwater ,
        :groundwater-dependent-ecosystem ,
        :groundwater-recharge ,
        :groundwater-system ,
        :groundwater-zone-of-potential-hydrological-change ,
        :hazard ,
        :hazard-priority-number ,
        :hazard-score ,
        :high-flow-days ,
        :hydrogeology ,
        :hydrological-response-variable ,
        :impact ,
        :impact-cause ,
        :impact-mode ,
        :indirect-impact ,
        :inertinite ,
        :inflow ,
        :interquartile-range ,
        :landscape-class ,
        :landscape-group ,
        :length-of-low-flow-spell ,
        :life-cycle-stage ,
        :likelihood ,
        :likelihood-score ,
        :list-date ,
        :lithic ,
        :low-flow-days ,
        :low-flow-days-averaged-over-30-years ,
        :low-flow-spells ,
        :marine-transgression ,
        :material ,
        :metadata-author ,
        :metadata-record-owner ,
        :metasedimentary-rock ,
        :mine-exclusion-zone ,
        :mine-pit-exclusion-zone ,
        :model-chain ,
        :model-domain-extent ,
        :model-emulator ,
        :model-node ,
        :model-spin-up-period ,
        :more-at-risk-of-ecological-and-hydrological-changes ,
        :more-at-risk-of-hydrological-changes ,
        :overbank-flow ,
        :overbench-flow ,
        :percentile ,
        :permeability ,
        :piezometric-surface ,
        :plugged-and-abandoned ,
        :pmax ,
        :porosity ,
        :preliminary-assessment-extent ,
        :probability-distribution ,
        :quantile ,
        :receptor ,
        :receptor-impact-model ,
        :receptor-impact-variable ,
        :receptor-register ,
        :recharge ,
        :regional-watertable ,
        :repeatability ,
        :reproducibility ,
        :response-variables ,
        :return-period ,
        :riparian ,
        :risk ,
        :riverbed-conductance ,
        :rune-of-mine-coal ,
        :runoff ,
        :saturated-zone ,
        :scalar-value ,
        :sensitivity ,
        :severity ,
        :severity-score ,
        :sleeper-licence ,
        :source-dataset ,
        :spring ,
        :stationary-system ,
        :stratigraphy ,
        :stressor ,
        :subcrop ,
        :subregion ,
        :subsidence ,
        :surface-water ,
        :surface-water-zone-of-potential-hydrological-change ,
        :sustainable-yield ,
        :tenement ,
        :tmax ,
        :tmaxRef ,
        :transmissivity ,
        :transparency ,
        :uncertainty ,
        :unconfined-aquifer ,
        :unsaturated-zone ,
        :very-likely ,
        :very-unlikely ,
        :water-allocation ,
        :water-dependent-asset ,
        :water-dependent-asset-register ,
        :water-make ,
        :water-system ,
        :water-use ,
        :watertable ,
        :well ,
        :zero-flow-days ,
        :zero-flow-days-averaged-over-30-years ,
        :zone-of-potential-hydrological-change ;
    skos:historyNote "2024-04: IRIs changed from http://www.neii.gov.au/def/voc/NEII/Bioregional-Assessment-Programme-Glossary/Bioregional-Assessment-Programme-Glossary for the ConceptScheme and http://www.neii.gov.au/def/voc/NEII/Bioregional-Assessment-Programme-Glossary/ for the Concept namespace to linked.data.gov.au-based IRIs" ;
    skos:prefLabel "Bioregional Assessment Programme Glossary"@en ;
.
